\documentclass[letterpaper,12pt,fleqn]{article}
\usepackage{matharticle}
\pagestyle{empty}
\renewcommand{\d}{\delta}
\newcommand{\e}{\epsilon}
\newcommand{\limz}{\lim_{z\to z_0}}
\newcommand{\limxy}{\lim_{(x,y)\to (x_0,y_0)}}
\begin{document}
\section*{Continuity}

\begin{definition}
  To say that $f(z)$ is \emph{continuous} at a point $z_0$ means:
  \[\forall\,\e>0,\exists\,\d>0,0<\abs{z-z_0}<\d\implies\abs{f(z)-f(z_0)}<\e\]
  In other words:
  \[\limz{f(z)}=f(z_0)\]
  To say that $f(z)$ is continuous in a region $R$ means
  $\forall\,z\in R,f(z)$ is continuous at $z$.
\end{definition}

\begin{theorem}
  Let $f(z)=u+iv$ and $z_0=x_0+iy_0$: \\
  $f(z)$ is continuous at $z_0\iff u$ and $v$ are continuous at $(x_0,y_0)$
\end{theorem}

\begin{theproof}
  \listbreak
  \begin{description}
  \item $\implies$ Assume $f(z)$ is continuous at $z_0$

    Let $u(x_0,y_0)=u_0$ and $v(x_0,y_0)=v_0$ \\
    $\limz f(z)=f(z_0)=u(x_0,y_0)+iv(x_0,y_0)=u_0+iv_0$ \\
    $\limz f(z)=\limxy u(x,y)+i\limxy v(x,y)$ \\
    $\limxy u(x,y)+i\limxy v(x,y)=u_0+iv_0$ \\
    $\limxy u(x,y)=u_0$ and $\limxy v(x,y)=v_0$ \\
    $\therefore u$ and $v$ are continuous at $(x_0,y_0)$

  \item $\impliedby$ Assume $u$ and $v$ are continuous at $(x_0,y_0)$

    Let $u(x_0,y_0)=u_0$ and $v(x_0,y_0)=v_0$ \\
    Let $\limxy u(x,y)=u_0$ and $\limxy v(x,y)=v_0$ \\
    $\limz f(z)=\limxy u(x,y)+i\lim v(x,y)=u_0+iv_0=f(z_0$) \\
    $\therefore f(z)$ is continuous at $z_0$
  \end{description}
\end{theproof}

The following theorem also follows directly from the limit laws:

\begin{theorem}
  Assume $f(z)$ and $g(z)$ are continuous at a point $z_0$:
  \begin{enumerate}
  \item $\abs{f(z)}$ is continuous at $z_0$
  \item $-f(z)$ is continuous at $z_0$
  \item $f(z)+g(z)$ is continuous at $z_0$
  \item $f(z)-g(z)$ is continuous at $z_0$
  \item $f(z)g(z)$ is continuous at $z_0$
  \item $f(z_0)\ne0\implies\frac{1}{f(z)}$ is continuous at $z_0$
  \item $g(z_0)\ne0\implies\frac{f(z)}{g(z)}$ is continuous at $z_0$
  \end{enumerate}
\end{theorem}

\begin{theorem}
  $f(z)$ and $g(z)$ continuous at $z_0\implies (f\circ g)(z)$ continuous at
  $z_0$.
\end{theorem}

\begin{theproof}
  Assume $f(z)$ and $g(z)$ are continuous at $z_0$ \\
  Assume $\e>0$ \\
  $\exists\,\d_1>0,0<\abs{z-z_0}<\d_1\implies\abs{f(z)-f(z_0)}<\e$ \\
  $\exists\,\d_2>0,0<\abs{f(z)-f(z_0)}<\d_2\implies
  \abs{g[f(z)]-g[f(z_0)]}<\e$ \\
  Let $\d=\min\{\d_1,\d_2\}$ \\
  Assume $0<\abs{z-z_0}<\d$ \\
  $\abs{f(z)-f(z_0)}<\e$ \\
  $\abs{g[f(z)]-g[f(z_0)]}<\e$
\end{theproof}

\begin{theorem}
  Let $f(z)$ be continuous at $z_0$ and $f(z_0)\ne0$:
  \[\exists\,\e>0,\forall\,z\in N_{\e}(z_0),f(z)\ne 0\]
\end{theorem}

\begin{theproof}
  Let $\e=\frac{\abs{f(z_0)}}{2}>0$ \\
  $\exists\,\d>0,0<\abs{z-z_0}<\d\implies\abs{f(z)-f(z_0)}<
  \frac{\abs{f(z_0)}}{2}$ \\
  ABC: $\exists\,z^*,0<\abs{z^*-z_0}<\d$ and $f(z^*)=0$ \\
  $\abs{f(z^*)-f(z_0)}=\abs{f(z_0)}<\frac{\abs{f(z_0)}}{2}$ \\
  But $f(z_0)\ne0$ \\
  Contradiction! \\
  $\therefore f(z^*)\ne0$
\end{theproof}

\begin{theorem}
  Let $R$ be a closed and bounded region: \\
  $f(z)$ continuous on
  $R\implies\exists\,M>0,\forall\,z\in R,\abs{f(z)}\le M$. \\
  Furthermore, equality occurs for at least one $z\in R$.
\end{theorem}
\newpage
\begin{theproof}
  Assume $f(z)$ is continuous on $R$ \\
  Let $f(z)=u+iv$ \\
  $u$ and $v$ are bounded and continuous in $R$ \\
  $\sqrt{u^2+v^2}\in\R$ is bounded and continuous and achieves some maximum
  value $M$ in $R$ \\
  But $\abs{f(z)}=\sqrt{u^2+v^2}$ \\
  $\therefore \forall\,z\in R,\abs{f(z)}\le M$, with equality somewhere in $R$.
\end{theproof}

\end{document}
