\documentclass[letterpaper,12pt,fleqn]{article}
\usepackage{matharticle}
\pagestyle{empty}
\renewcommand{\l}{\lambda}
\newcommand{\m}{\mu}
\renewcommand{\o}{\sigma}
\twocolumn
\begin{document}

\subsubsection*{Derivatives}

\begin{gather*}
  f'(x)=\lim_{h\to0}\frac{f(x+h)-f(x)}{h} \\
  \frac{d}{dx}\left[c\right]=0 \\
  \frac{d}{dx}\left[x^c\right]=cx^{c-1} \\
  \frac{d}{dx}\left[cf(x)\right]=cf'(x) \\
  \frac{d}{dx}\left[f(x)\pm g(x)\right]=f'(x)\pm g'(x) \\
  \frac{d}{dx}\left[f(x)g(x)\right]=f(x)g'(x)+f'(x)g(x) \\
  \frac{d}{dx}\left[\frac{f(x)}{g(x)}\right]=\frac{g(x)f'(x)-g'(x)f(x)}{[g(x)]^2} \\
  \frac{d}{dx}\left[f(u(x))\right]=f'(u)u'(x) \\
  \frac{d}{dx}\left[\frac{1}{x}\right]=-\frac{1}{x^2} \\
  \frac{d}{dx}\left[e^x\right]=e^x \\
  \frac{d}{dx}\left[e^{u(x)}\right]=e^{u(x)}u'(x) \\
  \frac{d}{dx}\left[a^x\right]=a^x\ln(a) \\
  \frac{d}{dx}\left[a^{u(x)}\right]=a^{u(x)}u'(x)\ln(a) \\
  \frac{d}{dx}\left[\ln(x)\right]=\frac{1}{x} \\
  \frac{d}{dx}\left[\ln(u(x))\right]=\frac{u'(x)}{u(x)} \\
  \frac{d}{dx}\left[\log_a(x)\right]=\frac{1}{\ln(a)}\cdot\frac{1}{x} \\
  \frac{d}{dx}\left[\log_a(u(x))\right]=\frac{1}{\ln(a)}\cdot\frac{u'(x)}{u(x)}
\end{gather*}

\subsection*{Probability}

\[p(x)=\frac{1}{\o\sqrt{2\pi}}e^{\frac{-(x-\m)^2}{2\o^2}}\]
68--95--99.7 rule

\subsubsection*{First/Second Derivative Tests}

\begin{tabular}{|l|l|l|}
  \hline
  & \(<0\) & \(>0\) \\
  \hline
  \(f'(x)\) & decreasing & increasing \\
  \hline
  \(f''(x)\) & concave down & concave up \\
  \hline
\end{tabular}

\subsection*{Business}

\begin{gather*}
  C(n)=F+n(p)V \\
  R(n)=pn(p) \\
  P(n)=R(n)-C(n)
\end{gather*}

\subsubsection*{Lagrange Multiplier}

\begin{gather*}
f_x=\l g_x \\
f_y=\l g_y \\
\vdots \\
g(x,y,\ldots)=0
\end{gather*}

\subsubsection*{Interest}

\begin{tabular}{ll}
  Compound Interest & \(A=P\left(1+\frac{r}{n}\right)^{nt}\) \\
  Population Growth & \(P(t)=P(0)e^{rt}\) \\
  Radioactive Decay & \(m(t)=m(0)e^{-\frac{t\ln(2)}{h_0}}\)
\end{tabular}

\subsubsection*{Logarithms}

\begin{gather*}
  \ln(1)=0 \\
  \ln(e)=1 \\
  e^{\ln(x)}=x \\
  \ln(e^x)=x \\
  e^x=e^y\iff x=y \\
  \ln(x)=\ln(y)\iff x=y \\
  \ln(xy)=\ln(x)+\ln(y) \\
  \ln\left(\frac{x}{y}\right)=\ln(x)-\ln(y) \\
  \ln\left(x^y\right)=y\ln(x)
\end{gather*}

\subsection*{Indefinite Integrals}

\begin{gather*}
  \int kdx=kx+C \\
  \int x^kdx=\frac{x^{k+1}}{k+1} \\
  \int kf(x)dx=k\int f(x)dx \\
  \int\left[f(x)\pm g(x)\right]dx=\int f(x)dx\pm\int g(x)dx \\
  \int e^xdx=e^x+C \\
  \int\left[u'(x)e^{u(x)}\right]dx=e^{u(x)}+C \\
  \int\frac{dx}{x}=\ln\abs{x}+C \\
  \int\frac{u'(x)}{u(x)}dx=\ln\abs{u(x)}+C
\end{gather*}

\subsection*{Numerical Integration}

\begin{gather*}
  \int_a^b f(x)dx\approx\left(\frac{b-a}{2n}\right)\left[f(x_0)+2f(x_1)+\cdots+2f(x_{n-1})+f(x_n)\right] \\
  \int_a^b f(x)dx\approx\left(\frac{b-a}{3n}\right)
  \left[f(x_0)+4f(x_1)+2f(x_2)+\cdots+2f(x_{n-2})+4f(x_{n-1})+f(x_n)\right]
\end{gather*}

\subsection*{Even/Odd}

\begin{gather*}
  E+E=E \\
  O+O=O \\
  E\cdot E=E \\
  O\cdot O=E \\
  E\cdot O=O
\end{gather*}

\subsection*{Definite Integrals}

\begin{gather*}
  \int_a^bf(x)dx=F(b)-F(a) \\
  \int_a^b kf(x)dx=k\int_a^b f(x)dx \\
  \int_a^b\left[f(x)\pm g(x)\right]dx=\int_a^b f(x)dx\pm\int_a^b g(x)dx \\
  \int_a^b f(x)dx=\int_a^c f(x)dx+\int_c^b f(x)dx \\
  \int_a^a f(x)dx = 0 \\
  \int_a^b f(x)dx = -\int_b^a f(x)dx \\
  \int_{-a}^af(x)dx=2\int_0^a f(x)dx\qquad(f(x)\ \text{even}) \\
  \int_{-a}^af(x)dx=0\qquad(f(x)\ \text{odd}) \\
\end{gather*}

\end{document}
