\documentclass[letterpaper,12pt,fleqn]{article}
\usepackage{matharticle}
\pagestyle{empty}
\renewcommand{\o}{\theta}
\allowdisplaybreaks
\begin{document}
\section*{Reduction Formulas}
\begin{theorem}
Let $n\in\N$:
\begin{enumerate}
\item $\cos^{2n+1}\o=\frac{1}{2^{2n}}\sum_{k=0}^n\binom{2n+1}{k}\cos[(2n+1-2k)\o]$
\item $\cos^{2n}\o=\frac{1}{2^{2n}}\binom{2n}{n}+
    \frac{1}{2^{2n-1}}\sum_{k=0}^{n-1}\binom{2n}{k}\cos[2(n-k)\o]$
\item $\sin^{2n+1}\o=\frac{(-1)^n}{2^{2n}}
    \sum_{k=0}^n\binom{2n+1}{k}(-1)^k\sin[(2n+1-2k)\o]$
\item $\sin^{2n}\o=\frac{1}{2^{2n}}\binom{2n}{n}+
    \frac{(-1)^n}{2^{2n-1}}\sum_{k=0}^{n-1}\binom{2n}{k}(-1)^k\cos[2(n-k)\o]$
\end{enumerate}
\end{theorem}

\begin{theproof}
Assume $m\in\N-\{1\}$.

There exists $n\in\N$ such that:
\[m=\begin{cases}
    2n+1, & m\ \mbox{odd} \\
    2n, & m\ \mbox{even} \\
\end{cases}\]

\begin{eqnarray*}
\cos^m\o &=& \left(\frac{e^{i\o}+e^{-i\o}}{2}\right)^m \\
    &=& \frac{1}{2^m}\left(e^{i\o}+e^{-i\o}\right)^m \\
    &=& \frac{1}{2^m}\sum_{k=0}^m\binom{m}{k}e^{i(m-k)\o}e^{-ik\o} \\
    &=& \frac{1}{2^m}\sum_{k=0}^m\binom{m}{k}e^{i(m-2k)\o} \\
\end{eqnarray*}

\begin{description}
\item{\underline{case 1: $m$ odd ($m=2n+1$)}}

Consider the symmetry and the possible signs of the even number of binomial
coefficients:

\begin{tabular}{cccccc}
$\binom{2n+1}{0}$ & $\cdots$ & $\binom{2n+1}{n}$ &
    $\binom{2n+1}{n+1}$ & $\cdots$ & $\binom{2n+1}{2n+1}$ \\
$+$ & & $+$ & $+$ & & $+$ \\
\end{tabular}

The $k$ coefficient is equal to the $2n+1-k$ coefficient and all signs are
positive.

\begin{eqnarray*}
\cos^{2n+1}\o &=& \frac{1}{2^{2n+1}}\sum_{k=0}^n\binom{2n+1}{k}
        \left[e^{i(2n+1-2k)\o}+e^{i[2n+1-2(2n+1-k)]\o}\right] \\
    &=& \frac{1}{2^{2n+1}}\sum_{k=0}^n\binom{2n+1}{k}
        \left[e^{i(2n+1-2k)\o}+e^{i(-2n-1+2k)\o}\right] \\
    &=& \frac{1}{2^{2n+1}}\sum_{k=0}^n\binom{2n+1}{k}
        \left[e^{i(2n+1-2k)\o}+e^{-i(2n+1-2k)\o}\right] \\
    &=& \frac{1}{2^{2n}}\sum_{k=0}^n\binom{2n+1}{k}
        \left[\frac{e^{i(2n+1-2k)\o}+e^{-i(2n+1-2k)\o}}{2}\right] \\
    &=& \frac{1}{2^{2n}}\sum_{k=0}^n\binom{2n+1}{k}\cos[(2n+1-2k)\o] \\
\end{eqnarray*}

\item{\underline{case 2: $m$ even ($m=2n$)}}

Consider the symmetry and the possible signs of the odd number of binomial
coefficients:

\begin{tabular}{ccccccc}
$\binom{2n}{0}$ & $\cdots$ & $\binom{2n}{n-1}$ & $\binom{2n}{n}$ &
    $\binom{2n}{n+1}$ & $\cdots$ & $\binom{2n}{2n}$ \\
$+$ & & $+$ & $+$ & $+$ & & $+$ \\
\end{tabular}

The $k$ coefficient is equal to the $2n-k$ coefficient and all signs are
positive.

\begin{eqnarray*}
\cos^{2n}\o &=& \frac{1}{2^{2n}}\binom{2n}{n}+
        \frac{1}{2^{2n}}\sum_{k=0}^n\binom{2n}{k}
        \left[e^{i(2n-2k)\o}+e^{i[2n-2(2n-k)]\o}\right] \\
    &=& \frac{1}{2^{2n}}\binom{2n}{n}+
        \frac{1}{2^{2n}}\sum_{k=0}^n\binom{2n}{k}
        \left[e^{i(2n-2k)\o}+e^{i(-2n+2k)\o}\right] \\
    &=& \frac{1}{2^{2n}}\binom{2n}{n}+
        \frac{1}{2^{2n}}\sum_{k=0}^n\binom{2n}{k}
        \left[e^{i(2n-2k)\o}+e^{-i(2n-2k)\o}\right] \\
    &=& \frac{1}{2^{2n}}\binom{2n}{n}+
        \frac{1}{2^{2n-1}}\sum_{k=0}^n\binom{2n}{k}
        \left[\frac{e^{i(2n-2k)\o}+e^{-i(2n-2k)\o}}{2}\right] \\
    &=& \frac{1}{2^{2n}}\binom{2n}{n}+
        \frac{1}{2^{2n-1}}\sum_{k=0}^n\binom{2n}{k}\cos[2(n-k)\o] \\
\end{eqnarray*}
\end{description}

Similarly:

\begin{eqnarray*}
\sin^m\o &=& \left(\frac{e^{i\o}-e^{-i\o}}{2i}\right)^m \\
    &=& \frac{1}{(2i)^m}\left(e^{i\o}-e^{-i\o}\right)^m \\
    &=& \frac{1}{(2i)^m}\sum_{k=0}^m\binom{m}{k}
        e^{i(m-k)\o}\left(-e^{-i\o}\right)^k \\
    &=& \frac{1}{(2i)^m}\sum_{k=0}^m\binom{m}{k}(-1)^ke^{i(m-k)\o}e^{-ik\o} \\
    &=& \frac{1}{(2i)^m}\sum_{k=0}^m\binom{m}{k}(-1)^ke^{i(m-2k)\o} \\
\end{eqnarray*}

\begin{description}
\item{\underline{case 1: $m$ odd ($m=2n+1$)}}

Consider the symmetry and the possible signs of the even number of binomial
coefficients:

\begin{tabular}{cccccc}
$\binom{2n+1}{0}$ & $\cdots$ & $\binom{2n+1}{n}$ &
    $\binom{2n+1}{n+1}$ & $\cdots$ & $\binom{2n+1}{2n+1}$ \\
$+$ & & $+$ & $-$ & & $-$ \\
$+$ & & $-$ & $+$ & & $-$ \\
\end{tabular}

The $k$ coefficient is equal to the $2n+1-k$ coefficient and the signs
alternate.

\begin{eqnarray*}
\sin^{2n+1}\o &=& \frac{1}{(2i)^{2n+1}}\sum_{k=0}^n\binom{2n+1}{k}
        \left[(-1)^ke^{i(2n+1-2k)\o}+(-1)^{k+1}e^{i[2n+1-2(2n+1-k)]\o}\right] \\
    &=&  \frac{1}{(2i)^{2n+1}}\sum_{k=0}^n\binom{2n+1}{k}(-1)^k
        \left[e^{i(2n+1-2k)\o}-e^{i(-2n-1+2k)\o}\right] \\
    &=& \frac{1}{(2i)^{2n+1}}\sum_{k=0}^n\binom{2n+1}{k}(-1)^k
        \left[e^{i(2n+1-2k)\o}-e^{-i(2n+1-2k)\o}\right] \\
    &=& \frac{1}{(2i)^{2n}}\sum_{k=0}^n\binom{2n+1}{k}(-1)^k
        \left[\frac{e^{i(2n+1-2k)\o}-e^{-i(2n+1-2k)\o}}{2i}\right] \\
    &=& \frac{1}{2^{2n}}\frac{1}{i^{2n}}\sum_{k=0}^n\binom{2n+1}{k}(-1)^k
        \sin[(2n+1-2k)\o] \\
    &=& \frac{(-1)^n}{2^{2n}}\sum_{k=0}^n\binom{2n+1}{k}(-1)^k
        \sin[(2n+1-2k)\o] \\
\end{eqnarray*}

\item{\underline{case 2: $m$ even ($m=2n$)}}

Consider the symmetry and the possible signs of the odd number of binomial
coefficients:

\begin{tabular}{ccccccc}
$\binom{2n}{0}$ & $\cdots$ & $\binom{2n}{n-1}$ & $\binom{2n}{n}$ &
    $\binom{2n}{n+1}$ & $\cdots$ & $\binom{2n}{2n}$ \\
$+$ & & $+$ & $-$ & $+$ & & $+$ \\
$+$ & & $-$ & $+$ & $-$ & & $+$ \\
\end{tabular}

The $k$ coefficient is equal to the $2n-k$ coefficient and all signs match, but
alternate.

\begin{eqnarray*}
\sin^{2n}\o &=& \frac{1}{2^{2n}}\binom{2n}{n}+
        \frac{1}{(2i)^{2n}}\sum_{k=0}^n\binom{2n}{k}(-1)^k
        \left[e^{i(2n-2k)\o}+e^{i[2n-2(2n-k)]\o}\right] \\
    &=& \frac{1}{2^{2n}}\binom{2n}{n}+
        \frac{1}{(2i)^{2n}}\sum_{k=0}^n\binom{2n}{k}(-1)^k
        \left[e^{i(2n-2k)\o}+e^{i(-2n+2k)\o}\right] \\
    &=& \frac{1}{2^{2n}}\binom{2n}{n}+
        \frac{1}{(2i)^{2n}}\sum_{k=0}^n\binom{2n}{k}(-1)^k
        \left[e^{i(2n-2k)\o}+e^{-i(2n-2k)\o}\right] \\
    &=& \frac{1}{2^{2n}}\binom{2n}{n}+
        \frac{1}{2^{2n-1}}\left(\frac{1}{i^{2n}}\right)\sum_{k=0}^n\binom{2n}{k}
        (-1)^k\left[\frac{e^{i(2n-2k)\o}+e^{-i(2n-2k)\o}}{2}\right] \\
    &=& \frac{1}{2^{2n}}\binom{2n}{n}+
        \frac{(-1)^n}{2^{2n-1}}\sum_{k=0}^n\binom{2n}{k}(-1)^k\cos[2(n-k)\o] \\
\end{eqnarray*}
\end{description}
\end{theproof}

\begin{example}
\begin{eqnarray*}
\cos^2\o &=& \frac{1}{4}\binom{2}{1}+
    \frac{1}{2}\sum_{k=0}^0\binom{2}{k}\cos(2-2k)\o \\
    &=& \frac{1}{4}(2)+\frac{1}{2}\binom{2}{0}\cos2\o \\
    &=& \frac{1}{2}+\frac{1}{2}\cos2\o \\
    &=& \frac{1+\cos2\o}{2} \\
\end{eqnarray*}

\begin{eqnarray*}
\sin^2\o &=& \frac{1}{4}\binom{2}{1}-
    \frac{1}{2}\sum_{k=0}^0\binom{2}{k}\cos(2-2k)\o \\
    &=& \frac{1}{4}(2)-\frac{1}{2}\binom{2}{0}\cos2\o \\
    &=& \frac{1}{2}-\frac{1}{2}\cos2\o \\
    &=& \frac{1-\cos2\o}{2} \\
\end{eqnarray*}

\begin{eqnarray*}
\cos^3\o &=& \frac{1}{4}\sum_{k=0}^1\binom{3}{k}\cos[(3-2k)\o] \\
4\cos^3\o &=& \binom{3}{0}\cos3\o+\binom{3}{1}\cos\o \\
4\cos^3\o &=& \cos3\o+3\cos\o \\
\cos3\o &=& 4\cos^3\o-3\cos\o \\
\end{eqnarray*}

\begin{eqnarray*}
\sin^3\o &=& -\frac{1}{4}\sum_{k=0}^1\binom{3}{k}(-1)^k\sin[(3-2k)\o] \\
-4\sin^3\o &=& \binom{3}{0}\sin3\o-\binom{3}{1}\sin\o \\
-4\sin^3\o &=& \sin3\o-3\sin\o \\
\sin3\o &=& 3\sin\o-4\sin^3\o \\
\end{eqnarray*}
\end{example}
\end{document}
