\documentclass[letterpaper,12pt,fleqn]{article}
\usepackage{matharticle}
\usepackage{esint}
\pagestyle{empty}
\DeclareMathOperator{\Res}{Res}
\begin{document}
\section*{Extended Complex Plane}

\begin{definition}
  The extended complex plane is $C\cup\{\infty\}$.
\end{definition}

\begin{definition}
  Let $C$ be a circle in the clockwise direction containing all of the
  singularities of $f(z)$ in the finite complex plane. The residue of $f(z)$
  at $\infty$ is given by:
  \[\Res[f,\infty]=\frac{1}{2\pi i}\ointclockwise_{C}f(z)dz=
  -\frac{1}{2\pi i}\ointctrclockwise_{C}f(z)dz\]
\end{definition}

\begin{example}
  $f(z)=z$

  To determine the behavior at $\infty$, examine the behavior in the
  neighborhood of infinity: \\
  $\lim_{z\to\infty}f(z)=\lim_{z\to 0}f(\frac{1}{z})=\frac{1}{z}$ \\
  Since the latter has a simple pole at $0$, $f(z)$ has a simple pole at
  $\infty$.

  Note that $f(z)=z$ is entire in the finite complex place, so:
  \[\Res[f,\infty]=-\frac{1}{2\pi i}\int_{C}zdz=0\]
\end{example}

\begin{example}
  $f(z)=\frac{1}{z}$

  $lim_{z\to\infty}f(z)=lim_{z\to0}f(\frac{1}{z})=z$ \\
  Since the latter is analytic at $0$, $f(z)$ is analytic at $\infty$.
  \[\Res[f,\infty]=-\frac{1}{2\pi i}\int_{C}\frac{1}{z}dz=
  -\frac{1}{2\pi i}[2\pi i(1)]=-1\]
\end{example}

\begin{theorem}
  $\Res[f,\infty]$ equals the negative of the coefficient of $z$ in the
  expansion of $f(\frac{1}{z})$.
\end{theorem}

\begin{theorem}
  Let $f(z)$ have a finite number of singularities $\{z_k\mid1\le k\le n\}$,
  all contained within $C$:
  \[\int_{C}f(z)dz=2\pi i\sum_{k=1}^n\Res[f,z_k]=-2\pi i\Res[f,\infty]\]
\end{theorem}

\begin{theorem}
  $Res[f(z),\infty]$ equals the negative of the coefficient of $w$ in the
  expansion of $f(\frac{1}{w})$.
\end{theorem}

\begin{example}
  $G(z)=\frac{b_{n-1}z^{n-1}+\cdots+b_0}{a_nz^n+\cdots+a_0}$
  \begin{eqnarray*}
    G\left(\frac{1}{w}\right) &=& \frac{\frac{b_{n-1}}{w^{n-1}}+\cdots+b_0}
    {\frac{a_n}{w^n}+\cdots+a_0} \\
    &=& \frac{b_{n-1}w+\cdots+b_0w^n}{a_n+\cdots+a_0w^n} \\
    &=& \frac{b_{n-1}}{a_n}w\left[\frac{1+\frac{b_{n-2}}{b_{n-1}}w+\cdots+
        \frac{b_0}{b_{n-1}}w^n}
      {1+\frac{a_{n-1}}{a_n}w+\cdots+\frac{a_0}{a_n}w^n}\right] \\
    &=& \frac{b_{n-1}}{a_n}w\left[\frac{1+\frac{b_{n-2}}{b_{n-1}}w+\cdots+
        \frac{b_0}{b_{n-1}}w^n}{1+a}\right] \\
    &=& \frac{b_{n-1}}{a_n}w\left[1+\frac{b_{n-2}}{b_{n-1}}w+\cdots+
      \frac{b_0}{b_{n-1}}w^n\right]\left[1-a+a^2\cdots\right] \\
  \end{eqnarray*}
  So the coefficient of $w$ is $\frac{b_{n-1}}{a_n}$

  $Res[G(z),\infty]=-\frac{b_{n-1}}{a_n}$
\end{example}

\end{document}
