\documentclass[letterpaper,12pt,fleqn]{article}
\usepackage{matharticle}
\pagestyle{plain}
\DeclareMathOperator{\nul}{Null}
\DeclareMathOperator{\nuly}{nullity}
\DeclareMathOperator{\rank}{rank}
\DeclareMathOperator{\tr}{tr}
\newcommand{\vx}{\vec{x}}
\newcommand{\vy}{\vec{y}}
\newcommand{\vz}{\vec{0}}
\newcommand{\conj}[1]{\overline{#1}}
\begin{document}
Cavallaro, Jeffery \\
Math 229 \\
Homework \#0

\bigskip

\begin{enumerate}
\item Let $A$ be an $m\times n$ matrix:
  \begin{enumerate}
  \item Prove: $\nul(A^*A)=\nul(A)$

    \begin{description}
    \item $\implies$ Assume $\vx\in\nul(A^*A)$

      $A^*A\vx=\vz$ \\
      $\conj{A}^TA\vx=\vz$ \\
      $\conj{\vx}^T\conj{A}^TA\vx=\conj{\vx}^T\vz=\vz$ \\
      $\left(\conj{A\vx}\right)^T(A\vx)=\vz$ \\
      $\|A\vx\|^2=0$ \\
      $A\vx=\vz$
      
      $\therefore\vx\in\nul(A)$

    \item $\impliedby$ Assume $\vx\in\nul(A)$

      $A\vx=\vz$ \\
      $A^*A\vx=A^*\vz=\vz$
      
      $\therefore\vx\in\nul(A^*A)$
    \end{description}

    $\therefore\nul(A^*A)=\nul(A)$

  \item Prove: $\rank(A^*A)=\rank(A)$

    $A$ is $m\times n$ \\
    $A^*$ is $n\times m$ \\
    $A^*A$ is $n\times n$
    
    By the dimension theorem:
    \[\rank(A^*A)+\nuly(A^*A)=n=\rank(A)+\nuly(A)\]
    But from the part (a): $\nul(A^*A)=\nul(A)$

    $\therefore\rank(A^*A)=\rank(A)$

  \item Prove: $\rank(A^*A)=\rank(AA^*)$

    Note that $(A^*)^*=A$, so from the part (b) we get: \\
    $\rank(A^*A)=\rank(A)$\hspace{2ex}and \\
    $\rank(AA^*)=\rank((A^*)^*A^*)=\rank(A^*)$

    Now, consider the null space of $A$: \\
    $A\vx=0\iff(\conj{A})\conj{\vx}=0$ \\
    Thus, there is a one-to-one correspondence between the vectors in $\nul(A)$
    and $\nul(\conj{A})$, and so $\nuly(A)=\nuly(\conj{A})$ \\
    But $A$ and $\conj{A}$ have the same number of columns, so by the
    dimension theorem: \\
    $\rank(A)=\rank(\conj{A})$ \\
    In class we proved that $\rank(A)=\rank(A^T)$, so: \\
    $\rank(A^*)=\rank(\conj{A}^T)=\rank(\conj{A})=\rank(A)$

    $\therefore,\rank(A^*A)=\rank(AA^*)$
    
  \end{enumerate}

\item Let $A$ and $B$ be square ($n\times n$) matrices:
  \begin{enumerate}
  \item Prove: $\tr(AB)=\tr(BA)$
    \begin{eqnarray*}
      tr(AB) &=& \sum_{i=1}^n(AB)_{ii} \\
      &=& \sum_{i=1}^n\sum_{k=1}^na_{ik}b_{ki} \\
      &=& \sum_{k=1}^n\sum_{i=1}^nb_{ki}a_{ik} \\
      &=& \sum_{k=1}^n(BA)_{kk} \\
      &=& \tr(BA)
    \end{eqnarray*}

  \item Prove: $\det(AB)=\det(BA)$
    \begin{eqnarray*}
      \det(AB) &=& \det(A)\det(B) \\
      &=& \det(B)\det(A) \\
      &=& \det(BA)
    \end{eqnarray*}

  \item Is it always true that $\rank(AB)=\rank(BA)$?

    No. Counterexample:

    \newcommand{\ma}{\begin{bmatrix} 1 & -1 \\ 0 & 0 \end{bmatrix}}
    \newcommand{\mb}{\begin{bmatrix} 1 & 0 \\ 1 & 0 \end{bmatrix}}

    $A=\ma, B=\mb$

    $AB=\ma\mb=\begin{bmatrix} 0 & 0 \\ 0 & 0 \end{bmatrix}$

    So $\rank(AB)=0$

    $BA=\mb\ma=\begin{bmatrix} 1 & -1 \\ 1 & -1 \end{bmatrix}$

    So $\rank(BA)=1$

    $\therefore\rank(AB)\ne\rank(BA)$
  \end{enumerate}

  \newcommand{\mm}{\begin{bmatrix}
      A & -\vx \\ \vy^T & 1
  \end{bmatrix}}
  \newcommand{\mn}{\begin{bmatrix}
      I_n & 0_{n\times 1} \\ -\vy^T & 1
  \end{bmatrix}}
  \newcommand{\mo}{\begin{bmatrix}
      A+\vx\vy^T & -\vx \\ 0 & 1
  \end{bmatrix}}

  \newpage
  
\item Let $A$ be an $n\times n$ square matrix and let $\vx$ and $\vy$ be
  two $n\times 1$ column vectors:
  \begin{enumerate}
  \item
    \[\mm\mn=\mo\]

  \item Prove: $\det\mm=\det(A+\vx\vy^T)$

    $\det\mn=\det(I_n)\det(\begin{bmatrix} 1 \end{bmatrix})=1\cdot1=1$

    $\det\mo=\det(A+\vx\vy^T)\det(\begin{bmatrix} 1 \end{bmatrix})=
    \det(A+\vx\vy^T)\cdot1=\det(A+\vx\vy^T)$

    \begin{eqnarray*}
      \det\left(\mm\mn\right) &=& \det\mo \\
      \left(\det\mm\right)\left(\det\mn\right) &=& \det\mo \\
      \left(\det\mm\right)(1) &=& \det(A+\vx\vy^T) \\
      \det\mm &=& \det(A+\vx\vy^T)
    \end{eqnarray*}
    
  \end{enumerate}

\end{enumerate}

\end{document}
