\documentclass[letterpaper,12pt,fleqn]{article}
\usepackage{matharticle}
\pagestyle{empty}
\newcommand{\vx}{\vec{x}}
\newcommand{\vy}{\vec{y}}
\newcommand{\norm}[1]{\left\|#1\right\|}
\newcommand{\inner}[1]{\left<#1\right>}
\begin{document}
\section*{Strong Convergence}

\begin{definition}[Strong Convergence]
  Let $E$ be an inner product space and let $(\vx_n)$ be a sequence of vectors
  in $E$. To say that $(\vx_n)$ converges to $\vx\in E$ \emph{strongly}, denoted
  $\vx_n\to\vx$, means:
  \[\norm{\vx_n-\vx}\to0\]
\end{definition}

\begin{theorem}
  Let $E$ be an inner product space and let $(\vx_n)$ be a sequence of vectors
  in $E$:
  \[\vx_n\to\vx\implies\norm{\vx_n}\to\norm{\vx}\]
\end{theorem}

\begin{theproof}
  Assume $\vx_n\to\vx$.
  
  $0\le\abs{\norm{\vx_n}-\norm{\vx}}\le\norm{\vx_n-\vx}$

  But $\norm{\vx_n-\vx}\to0$.

  $\therefore\abs{\norm{\vx_n}-\norm{\vx}}\to0$ and thus
  $\norm{\vx_n}\to\norm{\vx}$.
\end{theproof}

\begin{theorem}
  Let $E$ be an inner product space and let $(\vx_n)$ and $(\vy_n)$ be
  sequences of vectors in $E$:
  \[\vx_n\to\vx\ \mbox{and}\ \vy_n\to\vy\implies
  \inner{\vx_n,\vy_n}\to\inner{\vx,\vy}\]
\end{theorem}

\begin{theproof}
  Assume $\vx_n\to\vx\ \mbox{and}\ \vy_n\to\vy$.

  This means that $(\vx_y)$ is bounded. \\
  So $\exists\,M>0$ such that $\forall\,n\in\N,\norm{\vy_n}\le M$.
  \begin{eqnarray*}
    \abs{\inner{\vx_n,\vy_n}-\inner{\vx,\vy}} &=&
    \abs{\inner{\vx_n,\vy_n}-\inner{\vx,\vy_n}+\inner{\vx,\vy_n}-
      \inner{\vx,\vy}} \\
    &=& \abs{(\inner{\vx_n,\vy_n}-\inner{\vx,\vy_n})+(\inner{\vx,\vy_n}-
      \inner{\vx,\vy})} \\
    &\le& \abs{\inner{\vx_n,\vy_n}-\inner{\vx,\vy_n}}+
    \abs{\inner{\vx,\vy_n}-\inner{\vx,\vy}} \\
    &=& \abs{\inner{\vx_n-\vx,\vy_n}}-\abs{\inner{\vx,\vy_n-\vy}} \\
    &\le& \norm{\vx_n-\vx}\norm{\vy_n}-\norm{\vx}\norm{\vy_n-\vy} \\
    &\le& \norm{\vx_n-\vx}M-\norm{\vx}\norm{\vy_n-\vy} \\
    &\to& 0
  \end{eqnarray*}
  $\therefore\inner{\vx_n,\vy_n}\to\inner{\vx,\vy}$
\end{theproof}

\end{document}
