\documentclass[letterpaper,12pt,fleqn]{article}
\usepackage{matharticle}
\usepackage{tikz}
\pagestyle{empty}
\begin{document}
\section*{Metric}
$\forall z_1,z_2\in\C,\abs{z_1-z_2}$ is the \emph{distance} between $z_1$ and
$z_2$ in the complex plane:
\begin{figure}[h]
\setlength{\leftskip}{0.5in}
\begin{tikzpicture}
\draw [<->] (-1,0) -- (4,0);
\draw [<->] (0,-1) -- (0,4);
\draw [->] (0,0) -- (3,1);
\draw [->] (0,0) -- (2,3);
\draw [<-,dashed] (3,1) -- (2,3);
\node at (1.8,0.3) {$z_1$};
\node at (0.8,1.8) {$z_2$};
\node at (3.3,2.1) {$z_1-z_2$};
\end{tikzpicture}
\end{figure}
\begin{eqnarray*}
dist(z_1,z_2) &=& \abs{z_1-z_2} \\
    &=& \abs{(x_1+iy_1)-(x_2+iy_2)} \\
    &=& \abs{(x_1-x_2)+i(y_1-y_2)} \\
    &=& \sqrt{(x_1-x_2)^2+(y_1-y_2)^2} \\
\end{eqnarray*}

\begin{theorem}
$dist(z_1,z_2)=\abs{z_1-z_2}$ is a metric for $\C$.
\end{theorem}

\begin{theproof}
\listbreak
\begin{enumerate}
\item{positive-definite}
Assume $z_1,z_2\in\C$
\[\abs{z_1-z_2}=\sqrt{(x_1-x_2)^2+(y_1-y_2)^2}\ge0\]
\begin{eqnarray*}
\abs{z_1-z_2}=0 &\iff& \sqrt{(x_1-x_2)^2+(y_1-y_2)^2}=0 \\
    &\iff& x_1-x_2=0\ \mbox{and}\ y_1-y_2=0 \\
    &\iff& x_1=x_2\ \mbox{and}\ y_1=y_2 \\
    &\iff& z_1=z_2 \\
\end{eqnarray*}

\item{symmetry}
Assume $z_1,z_2\in\C$
\begin{eqnarray*}
\abs{z_1-z_2} &=& \sqrt{(x_1-x_2)^2+(y_1-y_2)^2} \\
    &=& \sqrt{(x_2-x_1)^2+(y_2-y_1)^2} \\
    &=& \abs{z_2-z_1} \\
\end{eqnarray*}

\item{sub-additivity}
Assume $z_1,z_2,z_3\in\C$
\[\abs{z_1-z_3}=\abs{(z_1-z_2)+(z_2-z_3)}\le\abs{z_1-z_2}+\abs{z_2-z_3}\]
\end{enumerate}
\end{theproof}
\end{document}
