\documentclass[letterpaper,12pt,fleqn]{article}
\usepackage{matharticle}
\pagestyle{plain}
\renewcommand{\l}{\lambda}
\begin{document}

\begin{center}
  \large
  Math-71 Sections 9, 11, 12

  \Large
  Exam \#3 Cheat Sheet
\end{center}

\vspace{0.25in}

\begin{minipage}[t]{3in}
  \subsection*{Derivatives}

  \begin{enumerate}[left=0pt]
    \setlength{\itemsep}{5pt}
  \item \(\displaystyle\frac{d}{dx}[c]=0\)
  \item \(\displaystyle\frac{d}{dx}[x^c]=cx^{c-1}\)
  \item \(\displaystyle\frac{d}{dx}[cf(x)]=cf'(x)\)
  \item \(\displaystyle\frac{d}{dx}[f(x)\pm g(x)]=f'(x)\pm g'(x)\)
  \item \(\displaystyle\frac{d}{dx}[f(x)g(x)]=f(x)g'(x)+f'(x)g(x)\)
  \item \(\displaystyle\frac{d}{dx}\left[\frac{f(x)}{g(x)}\right]=\frac{g(x)f'(x)-g'(x)f(x)}{[g(x)]^2}\)
  \item \(\displaystyle\frac{d}{dx}[f(u(x))]=f'(u)u'(x)\)
  \item \(\displaystyle\frac{d}{dx}[e^x]=e^x\)
  \item \(\displaystyle\frac{d}{dx}[\ln(x)]=\frac{1}{x}\)
  \end{enumerate}
\end{minipage}
\begin{minipage}[t]{3.5in}
  \subsection*{Integrals}

  \begin{enumerate}[left=0pt]
    \setlength{\itemsep}{5pt}
  \item \(\displaystyle\int kdx=kx+C\)
  \item \(\displaystyle\int x^kdx=\frac{1}{k+1}x^{k+1}+C\)
  \item \(\displaystyle\int kf(x)dx=k\int f(x)dx\)
  \item \(\displaystyle\int[f(x)\pm g(x)]dx=\int f(x)dx\pm\int g(x)dx\)
  \item \(\displaystyle\int_a^af(x)dx=0\)
  \item \(\displaystyle\int_a^bf(x)dx+\int_b^cf(x)dx=\int_a^cf(x)dx=0\)
  \item \(\displaystyle\int_a^bf(x)dx+-\int_b^af(x)dx\)
  \item \(\displaystyle\int e^xdx=e^x+C\)
  \item \(\displaystyle\int \frac{dx}{x}=\ln(x)+C\)
  \end{enumerate}
\end{minipage}

\vspace{0.5in}

\begin{minipage}[t]{3in}
  \subsection*{Second Partial Derivative Test}

  \[f_x=0\ \text{and}\ f_y=0\]
  \[d=f_{xx}f_{yy}-[f_{xy}]^2\]
  \begin{tabular}{c|c|c}
    \(d\) & \(f_{xx}\) & result \\
    \hline
    \(>0\) & \(>0\) & relative minimum \\
    \(>0\) & \(<0\) & relative maximum \\
    \(<0\) & & saddle point \\
    \(=0\) & & inconclusive
  \end{tabular}
\end{minipage}
\begin{minipage}[t]{3in}
\subsection*{Lagrange Multiplier}

\begin{gather*}
F(x,y,\l)=f(x,y)-\l g(x,y) \\
\\
f_x=\l g_x \\
f_y=\l g_y \\
g(x,y)=0
\end{gather*}
\end{minipage}

\end{document}
