\documentclass[letterpaper,12pt,fleqn]{article}
\usepackage{matharticle}
\pagestyle{empty}
\newcommand{\p}{\phi}
\begin{document}
\section*{Cayley's Theorem}

\begin{definition}
  Let $G$ be a group and $g\in G$. Define $L_g:G\to G$ by:
  \[L_g(x)=gx\]
\end{definition}

\begin{lemma}
  Let $G$ be a group and $g\in G$:
  \[L_g\ \mbox{is a permutation of}\ G\]
\end{lemma}

\begin{theproof}
  Assume $L_g(x)=L_g(y)$ \\
  $gx=gy$ \\
  $x=y$ \\
  $\therefore L_g$ is one-to-one.

  Assume $y\in G$ \\
  $g^{-1}\in G$ \\
  Let $x\in G,g^{-1}x=y$ \\
  $L_g(x)=g(g^{-1}y)=(gg^{-1})y=ey=y$ \\
  $\therefore L_g$ is onto.

  $\therefore L_g$ is a bijection, and thus a permutation of $G$.
\end{theproof}

\begin{lemma} 
  Let $G$ be a group and $G'=\{L_g\mid g\in G\}$:
  \[\forall\,L_{g_1},L_{g_2}\in G',L_{g_1}L_{g_2}=L_{g_1g_2}\]
\end{lemma}

\begin{theproof}
  Assume $L_{g_1},L_{g_2}\in G'$ \\
  Assume $x\in G$ \\
  $(L_{g_1}L_{g_2})(x)=L_{g_1}(L_{g_2}(x))=L_{g_1}(g_2x)=g_1(g_2x)=(g_1g_2)x=
  L_{g_1g_2}(x)$
\end{theproof}

\begin{lemma}
  Let $G$ be a group and $G'=\{L_g\mid g\in G\}$:
  \[G'\ \mbox{is a group}\]
\end{lemma}

\begin{theproof}
  Assume $L_{g_1},L_{g_2}\in G'$ \\
  $g_1,g_2\in G$ \\
  $L_{g_1}L_{g_2}=L_{g_1g_2}$ \\
  But by closure, $g_1g_2\in G$ \\
  $L_{g_1g_2}\in G'$ \\
  $\therefore G'$ is closed under the operation.

  Composition is associative \\
  $\therefore G'$ is associative under the operation.

  Let $e$ be the identity element for $G$ \\
  Assume $g\in G$ \\
  $L_eL_g=L_{eg}=L_g$ \\
  $L_gL_e=L_{ge}=L_g$ \\
  $\therefore L_e$ is an identity for $G'$.

  Assume $g\in G$ \\
  $g^{-1}\in G$ \\
  $L_{g^{-1}}L_g=L_{g^{-1}g}=L_e$ \\
  $L_gL_{g^{-1}}=L_{gg^{-1}}=L_e$ \\
  $\therefore G'$ is closed under inverses.

  $\therefore G'$ is a group.
\end{theproof}

\begin{theorem}[Cayley]
  Every group is isomorphic to a group of permutations.
\end{theorem}

\begin{theproof}
  Let $G$ a group and $G'=\{L_g\mid g\in G\}$
  $G'$ is a group (lemma)

  Let $\p:G\to G$ be defined by $\p(g)=L_g$

  Assume $\p(g_1)=\p(g_2)$ \\
  $L_{g_1}=L_{g_2}$ \\
  Assume $x\in G$ \\
  $L_{g_1}(x)=L_{g_2}(x)$ \\
  $g_1x=g_2x$ \\
  $g_1=g_2$ \\
  $\therefore \p$ is one-to-one.

  Assume $L_g\in G'$ \\
  $g\in G$ \\
  $\p(g)=L_g$ \\
  $\therefore \p$ is onto and thus a bijection.

  Assume $g_1,g_2\in G$ \\
  $\p(g_1g_2)=L_{g_1g_2}=L_{g_1}L_{g_2}=\p(g_1)\p(g_2)$
  $\therefore \p$ is a homomorphism and thus an isomorphism.

  $\therefore G\simeq G'$
\end{theproof}

\end{document}
