\documentclass[letterpaper,12pt,fleqn]{article}
\usepackage{matharticle}
\pagestyle{empty}
\newcommand{\e}{\epsilon}
\renewcommand{\l}{\lambda}
\newcommand{\norm}[1]{\|#1\|}
\newcommand{\vx}{\vec{x}}
\newcommand{\vy}{\vec{y}}
\begin{document}
\section*{Convergence}

\begin{definition}[Convergence]
  Let $(E,\norm{\cdot})$ be a normed space. To say that a sequence $(\vx_n)$ of
  elements in $E$ converges to some $\vx\in E$ means:
  \[\forall\e>0,\exists\,N(\e)>0,n>N\implies\norm{\vx_n-\vx}<\e\]
\end{definition}

\begin{notation}
  Any of the following can be used to indicate convergence:
  \begin{itemize}
  \item $\lim{\vx_n}=\vx$
  \item $\norm{\vx_n-\vx}\to0$
  \item $\vx_n\to\vx$
  \item $d(\vx_n,\vx)\to0$
  \end{itemize}
\end{notation}

\begin{theorem}[Properties]
  Let $(E,\norm{\cdot})$ be a normed space:
  \begin{enumerate}
  \item $(\vx_n)$ converges $\implies$ the limit is unique.
  \item $\vx_n\to\vx$ and $\l_n\to\l\implies\l_n\vx_n\to\l\vx$.
  \item $\vx_n\to\vx$ and $\vy_n\to\vy\implies(\vx_n+\vy_n)\to(\vx+\vy)$.
  \end{enumerate}
\end{theorem}

\begin{theproof}
  \listbreak
  \begin{enumerate}
  \item Assume $\vx_n\to\vx$ and $\vx_n\to\vy$.

    $\forall\,\e_1>0,\exists\,N_1>0,n>N_1\implies\norm{\vx_n-\vx}<\e_1$ \\
    $\forall\,\e_2>0,\exists\,N_2>0,n>N_2\implies\norm{\vx_n-\vy}<\e_2$ \\
    Assume $\e>0$. \\
    Let $\e_1,\e_2=\frac{\e}{2}$. \\
    Let $N=\max\{N_1,N_2\}$. \\
    Assume $n>N$. \\
    \[\norm{\vx-\vy}=\norm{\vx-\vx_n+\vx_n+\vy}\le
    \norm{\vx-\vx_n}+\norm{\vy-\vx_n}<\frac{\e}{2}+\frac{\e}{2}=\e\]

    $\therefore\vx=\vy$

  \item Assume $\vx_n\to\vx$ and $\l_n\to\l$.

    $\forall\,\e_1>0,\exists\,N_1>0,n>N_1\implies\norm{\vx_n-\vx}<\e_1$ \\
    $\forall\,\e_2>0,\exists\,N_2>0,n>N_2\implies\abs{\l_n-\l}<\e_2$ \\
    So $\exists\,N_3>0,n>N_3\implies\abs{\l_n-\l}<1$. \\
    Assume $\e>0$. \\
    Let $N=\max\{N_1,N_2,N_3\}$. \\
    Assume $n>N$. \\
    $\abs{\l_n}=\abs{\l_n-\l+\l}\le\abs{\l_n-\l}+\abs{\l}<1+\abs{\l}$ \\
    Let $\e_1=\frac{\e}{2(1+\abs{\l})}$ and
    $\e_2=\frac{\e}{2\norm{\vx}}$.
    \begin{eqnarray*}
      \norm{\l_n\vx_n-\l\vx} &=& \norm{\l_n\vx_n-\l_n\vx+\l_n\vx-\l\vx} \\
      &\le& \norm{\l_n\vx_n-\l_n\vx}+\norm{\l_n\vx-\l\vx} \\
      &=& \norm{\l_n(\vx_n-\vx)}+\norm{(\l_n-\l)\vx} \\
      &=& \abs{\l_n}\norm{\vx_n-\vx}+\abs{\l_n-\l}\norm{\vx} \\
      &<& (1+\abs{\l})\frac{\e}{2(1+\abs{\l})}+\frac{\e}{2\norm{\vx}}\norm{x} \\
      &=& \frac{\e}{2}+\frac{\e}{2} \\
      &=& \e
    \end{eqnarray*}
    $\therefore\l_n\vx_n\to\l\vx$

  \item Assume $\vx_n\to\vx$ and $\vy_n\to\vy$

    $\forall\,\e_1>0,\exists\,N_1>0,n>N_1\implies\norm{\vx_n-\vx}<\e_1$ \\
    $\forall\,\e_2>0,\exists\,N_2>0,n>N_2\implies\norm{\vy_n-\vy}<\e_2$ \\
    Assume $\e>0$. \\
    Let $\e_1,\e_2=\frac{\e}{2}$. \\
    Let $N=\max\{N_1,N_2\}$. \\
    Assume $n>N$.
    \begin{eqnarray*}
      \norm{(\vx_n+\vy_n)-(\vx+\vy)} &=& \norm{(\vx_n-\vx)+(\vy_n+\vy)} \\
      &\le& \norm{\vx_n-\vx}+\norm{\vy_n+\vy} \\
      &<& \frac{\e}{2}+\frac{\e}{2} \\
      &=& \e
    \end{eqnarray*}
    $\therefore(\vx_n+\vy_n)\to(\vx+\vy)$
  \end{enumerate}
\end{theproof}

\end{document}
