\documentclass[letterpaper,12pt,fleqn]{article}
\usepackage{matharticle}
\pagestyle{empty}
\begin{document}
\section*{Cayley-Hamilton}

\begin{theorem}[Cayley-Hamilton]
  Let $A\in M_n$ and $p_A(t)$ be its characteristic polynomial:
  \[p_A(A)=A^n+a_{n-1}A^{n-1}+\cdots+a_1A+a_0I=0\]
\end{theorem}

\begin{example}
  \newcommand{\A}{\begin{bmatrix} 3 & 1 \\ -2 & 0 \end{bmatrix}}
  $A=\A$

  $p_A(t)=t^2-3t+2$

  $\A^2-3\A+2I=\begin{bmatrix} 7 & 3 \\ -6 & -2 \end{bmatrix} +
  \begin{bmatrix} -9 & -3 \\ 6 & 0 \end{bmatrix} +
  \begin{bmatrix} 2 & 0 \\ 0 & 2 \end{bmatrix}=
  \begin{bmatrix} 0 & 0 \\ 0 & 0 \end{bmatrix}$
\end{example}

\begin{lemma}
  Let $S_1,\ldots,S_m\in UT(n)$ such that $(S_k)_{kk}=0$:
  \[\prod_{k=1}^nS_k=0\]
\end{lemma}

\begin{example}
  $\begin{bmatrix} 0 & 4 & 5 \\ 0 & 1 & 6 \\ 0 & 0 & 2 \end{bmatrix}
  \begin{bmatrix} 3 & 7 & 8 \\ 0 & 0 & 9 \\ 0 & 0 & 4 \end{bmatrix}
  \begin{bmatrix} 1 & 9 & 4 \\ 0 & -1 & 3 \\ 0 & 0 & 0 \end{bmatrix}=
  \begin{bmatrix} 0 & 0 & 46 \\ 0 & 0 & 33 \\ 0 & 0 & 8 \end{bmatrix}
  \begin{bmatrix} 1 & 9 & 4 \\ 0 & -1 & 3 \\ 0 & 0 & 0 \end{bmatrix}=
  \begin{bmatrix} 0 & 0 & 0 \\ 0 & 0 & 0 \\ 0 & 0 & 0\end{bmatrix}$
\end{example}

\begin{theproof}
  Proof by induction on $n$:
  \begin{description}
  \item Base Case: $n=1$:

    $S_1=\begin{bmatrix} 0 \end{bmatrix}$\hspace{2ex} (done).

  \item Assume true for $n-1$

  \item Consider $S_1,\ldots,S_n$

    Let $T_1,\ldots,T_n$ be the corresponding leading principal $(n-1)x(n-1)$
    matrices:
    \begin{eqnarray*}
    \prod_{k=1}^nS_k &=&
    \left[\begin{array}{@{}ccc|c@{}}
        & & & \\
        & T_1 & & * \\
        & & & \\
        \hline
        & 0 & & *
      \end{array}\right]
    \left[\begin{array}{@{}ccc|c@{}}
        & & & \\
        & T_2 & & * \\
        & & & \\
        \hline
        & 0 & & *
      \end{array}\right]
    \cdots
    \left[\begin{array}{@{}ccc|c@{}}
        & & & \\
        & T_{n-1} & & * \\
        & & & \\
        \hline
        & 0 & & *
      \end{array}\right]
    \left[\begin{array}{@{}ccc|c@{}}
        & & & \\
        & T_n & & * \\
        & & & \\
        \hline
        & 0 & & 0
      \end{array}\right] \\
    &=& \left[\begin{array}{@{}ccc|c@{}}
        & & & \\
        & \prod_{k=1}^{n-1}T_k & & * \\
        & & & \\
        \hline
        & 0 & & *
      \end{array}\right]
    \left[\begin{array}{@{}ccc|c@{}}
        & & & \\
        & T_n & & * \\
        & & & \\
        \hline
        & 0 & & 0
      \end{array}\right] \\
    &=& \left[\begin{array}{@{}ccc|c@{}}
        & & & \\
        & 0 & & * \\
        & & & \\
        \hline
        & 0 & & *
      \end{array}\right]
    \left[\begin{array}{@{}ccc|c@{}}
        & & & \\
        & T_n & & * \\
        & & & \\
        \hline
        & 0 & & 0
      \end{array}\right]\hspace{2ex}\mbox{by inductive assumption} \\
    &=& \left[\begin{array}{@{}ccc|c@{}}
        & & & \\
        & 0 & & 0 \\
        & & & \\
        \hline
        & 0 & & 0
      \end{array}\right]
    \end{eqnarray*}
  \end{description}
\end{theproof}

\begin{theproof}[Cayley-Hamilton]
  By Schur Triangularization, $\exists\,T\in UT(n)$ such that:
  \[A=UTU^*\]
  for some unitary matrix $U$
  
  Let $T=\begin{bmatrix} t_{11} & & * \\ & \ddots & \\ 0 & & t_{nn}
  \end{bmatrix}$
  
  Now, since characteristic polynomials for similar matrices are the same:
  \[p_A(t)=p_T(t)=\prod_{k=1}^n(t-t_{kk})\]
  \[p_A(A)=p_A(UTU^*)=Up_A(T)U*=U\left[\prod_{k=1}^n(T-t_{kk}I_n)\right]U^*=0
  \hspace{2ex}\mbox{(by lemma)}\]
\end{theproof}

A consequence of Cayley-Hamilton is that given any $A\in M_n$ and any
$k\in\Z^+$, $A^k$ is a polynomial of $A$ of degree atmost $n-1$.
\newpage
For example:

$A=\begin{bmatrix} 3 & 1 \\ -2 & 0 \end{bmatrix}$

$p_A(t)=t^2-3t+2$

$p_A(A)=A^2-3A+2I=0$ so $A^2=3A-2I$

$A^3=3A^2-2A=3(3A-2I)-2A=7A-6I$
\end{document}
