\documentclass[letterpaper,12pt,fleqn]{article}
\usepackage{matharticle}
\pagestyle{empty}
\newcommand{\norm}[1]{\|#1\|}
\newcommand{\vx}{\vec{x}}
\newcommand{\vy}{\vec{y}}
\begin{document}
\section*{Triangle Inequality}

For $\ell_1$:
\begin{eqnarray*}
  \norm{\vx+\vy}_1 &=& \sum_{k=1}^n\abs{x_i+y_i} \\
  &\le& \sum_{k=1}^n(\abs{x_i}+\abs{y_i}) \\
  &=& \sum_{k=1}^n\abs{x_i}+\sum_{k=1}^n\abs{y_i}) \\
  &=& \norm{\vx}_1+\norm{\vy}_1
\end{eqnarray*}

For $\ell_{\infty}$:
\begin{eqnarray*}
  \norm{\vx+\vy}_{\infty} &=& \max_{1\le k\le n}\abs{x_i+y_i} \\
  &\le& \max_{1\le k\le n}(\abs{x_i}+\abs{y_i}) \\
  &\le& \max_{1\le k\le n}\abs{x_i}+\max_{1\le k\le n}\abs{y_i}) \\
  &=& \norm{\vx}_{\infty}+\norm{\vy}_{\infty}
\end{eqnarray*}

For $\ell_2$:

\begin{lemma}
  Let $a,b\in\C$:
  \[2\abs{a}\abs{b}\le\abs{a}^2+\abs{b}^2\]
\end{lemma}

\begin{theproof}
  $(\abs{a}-\abs{b})^2\ge 0$ \\
  $\abs{a}^2-2\abs{a}\abs{b}+\abs{b}^2\ge 0$
  
  $\therefore 2\abs{a}\abs{b}\le\abs{a}^2+\abs{b}^2$
\end{theproof}

\begin{theorem}[Cauchy-Schwarz]
  Let $\vx,\vy\in\C^n$:
  \[\sum_{k=1}^nx_ky_k\le\abs{\sum_{k=1}^nx_ky_k}\le\sum_{k=1}^n\abs{x_ky_k}\le
  \left(\sum_{k=1}^n\abs{x_k}^2\right)^{\frac{1}{2}}
  \left(\sum_{k=1}^n\abs{y_k}^2\right)^{\frac{1}{2}}\]
\end{theorem}

\begin{theproof}
  \listbreak
  \begin{eqnarray*}
    \left(\sum_{k=1}^n\abs{x_k}\abs{y_k}\right)^2 &=&
    \sum_{k=1}^n\abs{x_k}^2\abs{y_k}^2+
    2\sum_{i<j}\abs{x_i}\abs{y_i}\abs{x_j}\abs{y_j} \\
    &=& \sum_{k=1}^n\abs{x_k}^2\abs{y_k}^2+
    2\sum_{i<j}(\abs{x_i}\abs{y_j})(\abs{y_i}\abs{x_j}) \\
    &\le& \sum_{k=1}^n\abs{x_k}^2\abs{y_k}^2+
    \sum_{i<j}(\abs{x_i}^2\abs{y_j}^2+\abs{y_i}^2\abs{x_j}^2) \\
    &=& \sum_{1\le i,j\le n}\abs{x_i}^2\abs{y_j}^2 \\
    &=& \left(\sum_{k=1}^n\abs{x_k}^2\right)
    \left(\sum_{k=1}^n\abs{y_k}^2\right) \\
    \therefore \sum_{k=1}^n\abs{x_ky_k} &\le&
    \left(\sum_{k=1}^n\abs{x_k}^2\right)^{\frac{1}{2}}
    \left(\sum_{k=1}^n\abs{y_k}^2\right)^{\frac{1}{2}}
  \end{eqnarray*}
\end{theproof}

\begin{theorem}
  Let $\vx,\vy\in\C^n$:
  \[\norm{\vx+\vy}_2\le\norm{\vx}_2+\norm{\vy}_2\]
\end{theorem}

\begin{theproof}
  \listbreak
  \begin{eqnarray*}
    \sum_{k=1}^n\abs{x_k+y_k}^2 &=& \sum_{k=1}^n\abs{x_k^2+2x_ky_k+y_k^2} \\
    &\le& \sum_{k=1}^n(\abs{x_k}^2+\abs{2x_ky_k}+\abs{y_k}^2) \\
    &=& \sum_{k=1}^n\abs{x_k}^2+2\sum_{k=1}^n\abs{x_ky_k}+
    \sum_{k=1}^n\abs{y_k}^2 \\
    &\le& \sum_{k=1}^n\abs{x_k}^2+
    2\left(\sum_{k=1}^n\abs{x_k}^2\right)^{\frac{1}{2}}
    \left(\sum_{k=1}^n\abs{y_k}^2\right)^{\frac{1}{2}}+
    \sum_{k=1}^n\abs{y_k}^2 \\
    &=&\left[\left(\sum_{k=1}^n\abs{x_k}^2\right)^{\frac{1}{2}}+
      \left(\sum_{k=1}^n\abs{y_k}^2\right)^{\frac{1}{2}}\right]^2 \\
    \left(\sum_{k=1}^n\abs{x_k+y_k}^2\right)^{\frac{1}{2}} &=&
    \left(\sum_{k=1}^n\abs{x_k}^2\right)^{\frac{1}{2}}+
    \left(\sum_{k=1}^n\abs{y_k}^2\right)^{\frac{1}{2}} \\
    \therefore \norm{\vx+\vy}_2 &\le& \norm{\vx}_2+\norm{\vy}_2
  \end{eqnarray*}
\end{theproof}

\end{document}
