\documentclass[letterpaper,12pt,fleqn]{article}
\usepackage{matharticle}
\pagestyle{empty}
\newcommand{\p}{\phi}
\begin{document}
\section*{Kernel}

\begin{definition}
  Let $\p:G\to G'$ be a homomorphism of groups. The $\emph{kernel}$ of $\p$,
  denoted $\ker(\p)$, is given by:
  \[\ker(\p)=\{g\in G\mid\p(g)=e'\}\]
  The kernel contains all elements that map to the identity.
\end{definition}

\begin{theorem}
  Let $\p:G\to G'$ be a homomorphism of groups:
  \[\ker(\p)\le G\]
\end{theorem}

\begin{theproof}
  Assume $a,b\in\ker(\p)$ \\
  $a,b\in G$ \\
  By closure, $ab\in G$ \\
  $\p(ab)=\p(a)\p(b)=e'e'=e'$ \\
  So $ab\in\ker(\p)$ \\
  $\therefore\ker(\p)$ is closed under the operation.

  $\p(e)=e'$ \\
  So $e\in\ker(\p)$ \\
  $\therefore\ker(\p)$ has an identity.

  Assume $a\in\ker(\p)$ \\
  $a\in G$ \\
  $a^{-1}\in G$ \\
  $\p(a^{-1})=\p(a)^{-1}=(e')^{-1}=e'$ \\
  So $a^{-1}\in\ker(\p)$ \\
  $\therefore\ker(\p)$ is closed under inverses.

  $\therefore\ker(\p)\le G$
\end{theproof}

\begin{theorem}
  Let $\p:G\to G'$ be a homomorphism of groups:
  \[\p\ \mbox{is one-to-one}\iff\ker(\p)=e\]
\end{theorem}
\newpage
\begin{theproof}
  \begin{minipage}[t]{3in}
    Assume $\p$ is one-to-one \\
    $\p(e)=e'$ \\
    Assume $\exists\,a\in G,\p(a)=e'$ \\
    $\p(e)=\p(a)$ \\
    $e=a$ \\
    $\therefore\ker(\p)=\{e\}$
  \end{minipage}
  \begin{minipage}[t]{3in}
    Assume $\ker(\p)=\{e\}$ \\
    Assume $a,b\in G,\p(a)=\p(b)$ \\
    $\p(a)\p(b)^{-1}=\p(a)\p(b^{-1})=\p(ab^{-1})=e'$ \\
    $ab^{-1}=e$ \\
    $a=b$ \\
    $\therefore\p$ is one-to-one
  \end{minipage}
\end{theproof}

\begin{theorem}
  Let $\p:G\to G'$ be a homomorphism of groups and $K=\ker(\p)$:
  \[\forall\,a\in G,aK=\{x\in G\mid\p(x)=\p(a)\}\]
  A homomorphism collapses all of the elements in the coset to the same
  element in $G'$.
\end{theorem}

\begin{figure}[h]
  \setlength{\leftskip}{0.5in}
  \begin{tikzpicture}
    \node at (0,0) {
      $\left.\begin{array}{c}a\\x_1\\x_2\\\vdots\\x_n\end{array}\right|$};
    \draw [->] (0.5,0) -- node [above] {$\p$} (3,0) node [right] {$\p(a)$};
    \draw (-0.5,-1.25) -- (-0.5,-1.5) -- node [below] {$aK$} (0.5,-1.5) --
    (0.5,-1.25);
  \end{tikzpicture}
\end{figure}

\begin{theproof}
  Assume $a\in G$
  
  Assume $y\in aK$ \\
  $\exists\,k\in K,y=ak$ \\
  $\p(y)=\p(ak)=\p(a)\p(k)=\p(a)e'=\p(a)$ \\
  $\therefore y\in\{x\in G\mid\p(x)=\p(a)\}$

  Assume $y\in\{x\in G\mid\p(x)=\p(a)\}$ \\
  $\p(y)=\p(a)$ \\
  $\p(a)^{-1}\p(y)=\p(a^{-1})\p(y)=\p(a^{-1}y)=e'$ \\
  So $a^{-1}y\in K$ and thus $\exists\,k\in K,a^{-1}y=k$ \\
  $y=ak$ \\
  $\therefore y\in aK$

  $\therefore aK=\{x\in G\mid\p(x)=\p(a)\}$
\end{theproof}

\begin{theorem}
  Let $\p:G\to G'$ be a homomorphism of groups and $K=\ker(\p)$:
  \[\forall\,a\in G,Ka=\{x\in G\mid\p(x)=\p(a)\}\]
\end{theorem}

\begin{theproof}
  Assume $a\in G$
  
  Assume $y\in Ka$ \\
  $\exists\,k\in K,y=ka$ \\
  $\p(y)=\p(ka)=\p(k)\p(a)=e'\p(a)=\p(a)$ \\
  $\therefore y\in\{x\in G\mid\p(x)=\p(a)\}$

  Assume $y\in\{x\in G\mid\p(x)=\p(a)\}$ \\
  $\p(y)=\p(a)$ \\
  $\p(y)\p(a)^{-1}=\p(y)\p(a^{-1})=\p(ya^{-1})=e'$ \\
  So $ya^{-1}\in K$ and thus $\exists\,k\in K,ya^{-1}=k$ \\
  $y=ka$ \\
  $\therefore y\in Ka$

  $\therefore Ka=\{x\in G\mid\p(x)=\p(a)\}$
\end{theproof}

\begin{corollary}
  Let $\p:G\to G'$ be a homomorphism of groups and $\ker(\p)=K$:
  \[\forall\,a\in G,aK=Ka\]
\end{corollary}

\begin{theorem}
  Let $\p:G\to G'$ be a homomorphism of groups and $\ker(\p)=K$:
  \[\forall\,g_1,g_2\in G,\phi[g_1Kg_2]=\{\phi(g_1g_2)\}\]
\end{theorem}

\begin{theproof}
  Assume $g_1,g_2\in G$ \\
  Assume $k\in K$ \\
  $\p(g_1kg_2)=\p(g_1)\p(k)\p(g_2)=\p(g_1)e'\p(g_2)=\p(g_1)\p(g_2)=\p(g_1g_2)$
\end{theproof}

\end{document}
