\documentclass[letterpaper,12pt,fleqn]{article}
\usepackage{matharticle}
\pagestyle{empty}
\begin{document}
\section*{Units}

\begin{definition}
  Let $R$ be a ring with unity $1\ne0$ and $a\in R$. To say that $a^{-1}\in R$
  is a \emph{multiplicative inverse} of $a$ means:
  \[aa^{-1}=a^{-1}a=1\]
\end{definition}

\begin{theorem}
  Let $R$ be a ring with unity $1\ne0$. $0\in R$ does not have a multiplicative
  inverse.
\end{theorem}

\begin{theproof}
  ABC: $0^{-1}\in R$ \\
  $00^{-1}=1$ \\
  But $00^{-1}=0$ \\
  $0=1$ \\
  CONTRADICTION! \\
  $\therefore 0$ has no multiplicative inverse.
\end{theproof}

\begin{definition}
  Let $R$ be a ring with unity $1\ne0$. To say that $a\in R$ is a \emph{unit}
  means that $a$ has a multiplicative inverse $a^{-1}\in R$.
\end{definition}

\begin{theorem}
  Let $R$ be a ring with unity $1\ne0$. $\forall\,a\in R, a$ is a unit
  $\implies a^{-1}$ is unique.
\end{theorem}

\begin{theproof}
  Assume $a$ is a unit in $R$ \\
  Let $b$ and $b'$ be multiplicative inverses of $a$ in $R$ \\
  $ab=ba=1$ \\
  $ab'=b'a=1$ \\
  $ab=ab'$ \\
  $b(ab)=b(ab')$ \\
  $(ba)b=(ba)b'$ \\
  $1b=1b'$ \\
  $b=b'$
\end{theproof}

\begin{theorem}
  Let $R$ be a ring with unity $1\ne0$ and let
  $R^*=\{a\in R\mid a\ \mbox{is a unit}\}$. $\left<R,\cdot\right>$ is a group.
\end{theorem}
\newpage
\begin{theproof}
  $(1)(1)=1$, so $1\in R^*$ and $R^*\ne\emptyset$

  Assume $a,b\in R^*$ \\
  $\exists\,a^{-1},b^{-1}\in R^*$ \\
  $(b^{-1}a^{-1})(ab)=b^{-1}(a^{-1}a)b=b^{-1}1b=b^{-1}b=1$ \\
  $(ab)(b^{-1}a^{-1})=a(bb^{-1})a^{-1}=a1a^{-1}=aa^{-1}=1$ \\
  $b^{-1}a^{-1}=(ab)^{-1}$ \\
  $ab\in R^*$ \\
  $\therefore R^*$ is closed under the operation.

  Assume $a\in R^*$ \\
  By definition, $a^{-1}\in R^*$ \\
  $\therefore R^*$ is closed under inverses.

  $\therefore R^*$ is a group.
\end{theproof}

\begin{example}
  $R=M_n(\R)$ \\
  $R^*=LR_n(\R)$

  $R=\Z$ \\
  $R^*=\{-1,1\}$

  $R=\Z_n$ \\
  $R^*=\{a\in\Z_n\mid(a,n)=1\}$
\end{example}

\begin{theorem}
  $u\in\Z_n$ is a unit $\iff (u,n)=1$
\end{theorem}

\begin{theproof}
  \listbreak
  \begin{description}
    \begin{minipage}[t]{3in}
    \item $\implies$ Assume $u\in\Z_n$ is a unit

      $\exists\,v\in\Z_n,uv=1$ \\
      $\exists\,k\in\Z,uv=kn+1$ \\
      $uv-kn=1$ \\
      Let $d=(u,n)$ \\
      $d\mid u$ and $d\mid n$ \\
      So $d\mid uv-kn$ \\
      Thus $d\mid 1$ \\
      $d=1$ \\
      $\therefore (u,n)=1$.
    \end{minipage}
    \begin{minipage}[t]{3in}
    \item $\impliedby$ Assume $(u,n)=1$

      $uv-kn=1$ has solutions in $R$ \\
      $uv=kn+1$ \\
      $uv=1$ \\
      But $Z_n$ is commutative, \\
      So $vu=1$ \\
      Thus, $u$ has multiplicative inverse $v$ \\
      $\therefore u$ is a unit.
    \end{minipage}
  \end{description}
\end{theproof}

\end{document}
