\documentclass[letterpaper,12pt,fleqn]{article}
\usepackage{matharticle}
\usepackage{siunitx}
\pagestyle{plain}
\begin{document}

\begin{center}
  \large
  Math-13 Sections 01 and 02

  \Large
  Homework \#8 Solutions
\end{center}

\vspace{0.5in}

Consider the function:
\[f(x)=(2x^2+1)\sqrt{3x-5}\]
Determine \(f'(x)\) and simplify.

Note that \(f(x)=g(x)h(x)\) where:
\begin{gather*}
  g(x)=2x^2+1 \\
  h(x)=\sqrt{3x-5}=(3x-5)^{\frac{1}{2}}
\end{gather*}
So we are going to use the product rule.  We will need the derivatives of the two parts:
\begin{gather*}
  g'(x)=4x \\
  h'(x)=\frac{1}{2}(3x-5)^{-\frac{1}{2}}(3)=\frac{3}{2}(3x-5)^{-\frac{1}{2}}
\end{gather*}
Note that we used the chain rule for \(h'(x)\).  Now, putting the parts together and simplifying:
\begin{align*}
  f'(x) &= g'(x)h(x)+g(x)h'(x) \\
  &= 4x(3x-5)^{\frac{1}{2}}+(2x^2+1)\frac{3}{2}(3x-5)^{-\frac{1}{2}} \\
  &= (3x-5)^{-\frac{1}{2}}\left[4x(3x-5)+\frac{3}{2}(2x^2+1)\right] \\
  &= (3x-5)^{-\frac{1}{2}}\left[12x^2-20x+3x^2+\frac{3}{2}\right] \\
  &= (3x-5)^{-\frac{1}{2}}\left[15x^2-20x+\frac{3}{2}\right] \\
  &= \frac{1}{2}(3x-5)^{-\frac{1}{2}}(30x^2-40x+3) \\
  &= \frac{30x^2-40x+3}{2\sqrt{3x-5}}
\end{align*}

\end{document}
