\documentclass[letterpaper,12pt,fleqn]{article}
\usepackage{matharticle}
\newcommand{\inner}[2]{\left<#1,#2\right>}
\newcommand{\conj}[1]{\overline{#1}}
\newcommand{\vx}{\vec{x}}
\newcommand{\vxct}{\vx^{\,*}}
\newcommand{\ve}{\vec{e}}
\newcommand{\vect}{\ve^{\,*}}
\newcommand{\vf}{\vec{f}}
\newcommand{\vu}{\vec{u}}
\pagestyle{empty}
\begin{document}
\section*{Gram Matrix}

\begin{theorem}
  Let $\inner{\cdot}{\cdot}$ be an inner product on a vector space $V$ with
  basis $\{\vf_1,\ldots,\vf_2\}$ and let $G=\left[\inner{\vf_j}{\vf_i}\right]$,
  which is called the \emph{Gram matrix}:

  $G$ is positive definite.
\end{theorem}

\begin{theproof}
  Assume $\vx\in\C^n$:
  \begin{eqnarray*}
    \vxct G\vx &=& \left(\sum_{i=1}^nx_i\ve_i\right)^*G
    \left(\sum_{j=1}^nx_j\ve_j\right) \\
    &=& \sum_{i=1}^n\sum_{j=1}^n\conj{x_i}(\vect_iG\ve_j)x_j \\
    &=& \sum_{i=1}^n\sum_{j=1}^n\conj{x_i}x_ja_{ij} \\
    &=& \sum_{i=1}^n\sum_{j=1}^n\conj{x_i}x_j\inner{\vf_j}{\vf_i} \\
    &=& \sum_{i=1}^n\sum_{j=1}^n\inner{x_j\vf_j}{x_i\vf_i} \\
    &=& \inner{\sum_{j=1}^nx_j\vf_j}{\sum_{i=1}^nx_i\vf_i} \\
  \end{eqnarray*}
  Let $\vu=\sum_{i=1}^nx_i\vf_i\in V$:
  \[\vxct G\vx = \inner{\vu}{\vu}\ge 0\]
  Equality only holds when $\vu=0$, which means that all the $x_i=0$ because the
  $\vf_i$ are linearly independent, which means $\vx=0$

  $\therefore G$ is positive definite.
\end{theproof}

\begin{example}
  \listbreak
  \begin{enumerate}
  \item $V=\C^n$ and $\inner{x}{y}=\sum_{k=1}^n\conj{y_i}x_i=y^*x$ and
    $\vf_i=\ve_i$

    $\inner{\vf_i}{\vf_j}=\begin{cases}
    1, & i=j \\
    0, & i\ne j
    \end{cases}$

    So $G=I_n$, which is positive definite.

  \item Same as above, except use basis
    $\left\{\begin{bmatrix} 1 \\ 0 \\ 0 \end{bmatrix},
    \begin{bmatrix} 1 \\ 1 \\ 0 \end{bmatrix},
    \begin{bmatrix} 1 \\ 1 \\ 1 \end{bmatrix}\right\}$

    $G=\begin{bmatrix}
    1 & 1 & 1 \\
    1 & 2 & 2 \\
    1 & 2 & 3
    \end{bmatrix}$

  \item $V$ consists of polynomials of degree at most $n$

    $\inner{p(x)}{q(x)}=\int_0^1p(x)\conj{q(x)}dx$

    Use basis $\{1,x,x^2,\ldots,x^n\}$

    $\inner{x^{j-1}}{x^{i-1}}=\int_0^1x^{i+j-2}dx=
    \left.\frac{1}{i+j-1}x^{i+j-1}\right\rvert_0^1=\frac{1}{i+j+1}$

    $G=\begin{bmatrix}
    \frac{1}{1} & \frac{1}{2} & \frac{1}{3} & \cdots & \frac{1}{n} \\
    \frac{1}{2} & \frac{1}{3} & \frac{1}{4} & \cdots & \frac{1}{n+1} \\
    \frac{1}{3} & \frac{1}{4} & \frac{1}{5} & \cdots & \frac{1}{n+2} \\
    \vdots & \vdots & \vdots & \vdots & \vdots \\
    \frac{1}{n} & \frac{1}{n+1} & \frac{1}{n+2} & \cdots & \frac{1}{2n-1} \\
    \end{bmatrix}$
  \end{enumerate}
\end{example}

\end{document}
