\documentclass[letterpaper,12pt,fleqn]{article}
\usepackage{matharticle}
\pagestyle{empty}
\renewcommand{\o}{\sigma}
\newcommand{\ms}[1]{\begin{bmatrix} #1 \end{bmatrix}}
\DeclareMathOperator{\sgn}{sgn}
\begin{document}
\section*{Determinants}

\begin{definition}[Determinant]
  Let $A\in M_n$. The \emph{determinant} of $A$ is given by:
  \[\det(A)=\sum_{\o\in S_n}(-1)^{\sgn(\o)}\prod_{k=1}^na_{k,\o(k)}\]
  where:
  \[\sgn(\o)=\begin{cases}
  0, & \o\ \mbox{even} \\
  1, & \o\ \mbox{odd}
  \end{cases}\]
\end{definition}

\begin{definition}[Laplace Expansion]
  Let $A\in M_n$. The \emph{determinant} of $A$ is given by:
  \[\det(A)=
  \sum_{k=1}^n(-1)^{i+j}a_{ij}\det(A_{ij})=
  \sum_{j=1}^n(-1)^{i+j}a_{ij}\det(A_{ij})\]
  where the first expansion is across the $j^{th}$ column and the second
  expansion is across the $i^{th}$ row.
\end{definition}

Recall that $(-1)^{i+j}\det(A_{ij})$ is a cofactor of $A$.

\begin{example}
  $A=\begin{bmatrix} a & b \\ c & d \end{bmatrix}$

  $\det(A)=a\det\ms{d}-b\det\ms{c}=ad-bc$

  $A=\begin{bmatrix}
  a_{11} & a_{12} & a_{13} \\
  a_{21} & a_{22} & a_{23} \\
  a_{31} & a_{32} & a_{33} \\
  \end{bmatrix}$
  \begin{eqnarray*}
    \det(A) &=& a_{11}\det\begin{bmatrix} a_{22} & a_{23} \\ a_{32} & a_{33} \end{bmatrix}-
    a_{12}\det\begin{bmatrix} a_{21} & a_{23} \\ a_{31} & a_{33} \end{bmatrix}+
    a_{13}\det\begin{bmatrix} a_{21} & a_{22} \\ a_{31} & a_{32} \end{bmatrix} \\
    &=& a_{11}(a_{22}a_{33}-a_{23}a_{32})-a_{12}(a_{21}a_{33}-a_{23}a_{31})+
    a_{13}(a_{21}a_{32}-a_{22}a_{31}) \\
    &=& a_{11}a_{22}a_{33}-a_{11}a_{23}a_{32}-a_{12}a_{21}a_{33}+a_{12}a_{23}a_{31}+
    a_{13}a_{21}a_{32}-a_{13}a_{22}a_{31} \\
    &=& a_{11}a_{22}a_{33}+a_{12}a_{23}a_{31}+a_{13}a_{21}a_{32}-
    (a_{11}a_{23}a_{32}+a_{12}a_{21}a_{33}+a_{13}a_{22}a_{31})
  \end{eqnarray*}
\end{example}

\begin{properties}
  \listbreak
  \begin{enumerate}
  \item $\det(A)=\det(A^T)$
    
  \item $\det(\bar{A})=\overline{\det(A)}$
    
  \item Effects of elementary row operations:
    \begin{description}
    \item Scale - scale determinant
    \item Swap - negation (change sign)
    \item Replace - no effect
    \end{description}
    
  \item Let $T$ be an upper-triangular matrix:
    \[\det(T)=\prod_{k=1}^nt_{kk}\]
    Use EROs to put a matrix in upper-triangular form (swap/replace) and then
    calculate by multiplying the diagonal entries.

  \item $\det\begin{bmatrix} A & B \\ 0 & C \end{bmatrix}=\det(A)\det(B)$

    $\det\begin{bmatrix} A & B \\ 0 & C \end{bmatrix}\to
    \det\begin{bmatrix} T_A & * \\ 0 & T_C \end{bmatrix}$

  \item $\det(AB)=\det(A)\det(B)$

    \begin{theproof}
      \listbreak
      \begin{description}
      \item Case 1: $\det(A)=0$

        $A$ is not invertible \\
        ABC: $AB$ is invertible \\
        $\exists\,C,(AB)C=I$ \\
        $A(BC)=I$ \\
        $A^{-1}=BC$ \\
        Contradiction! \\
        Thus, $AB$ is not invertible \\
        Therefore $\det(AB)=0$ \\
        Also $\det(A)\det(B)=0\cdot\det(B)=0$

        $\therefore \det(AB)=\det(A)\det(B)$

      \item Case 2: $\det(A)\ne0$

        $A$ is invertible \\
        There exists a sequence of ERO matrices $E_1E_2\cdot E_k$ such that
        $E_k\cdot E_2E_1A=I$ \\
        But ERO matrices are invertible, so $A=E_1^{-1}E_2^{-1}\cdot E_k^{-1}I$ \\
        $AB=E_1^{-1}E_2^{-1}\cdot E_k^{-1}B$ \\
        But $\det(EB)=\det(E)\det(B)=\pm\det(B)$, so:
        \begin{eqnarray*}
          \det(AB) &=& \det(E_1^{-1})\det(E_2^{-1})\cdot\det(E_k^{-1})\det(B) \\
          &=& \det(E_1^{-1}E_2^{-1}\cdot E_k^{-1})\det(B) \\
          &=& \det(A)\det(B)
        \end{eqnarray*}
      \end{description}
    \end{theproof}
  \end{enumerate}
\end{properties}

\end{document}
