\documentclass[letterpaper,12pt,fleqn]{article}
\usepackage{matharticle}
\pagestyle{empty}
\newcommand{\conj}[1]{\bar{#1}}
\newcommand{\Conj}[1]{\overline{#1}}
\begin{document}
\section*{Milne-Thomson}

\begin{example}
  Let $f(z)$ be entire and $u(x,y)=x^4-6x^2y^2+y^4$. Find $v(x,y)$.

  $u_x=4x^3-12xy^2=v_y$ \\
  $v(x,y)=4x^3y-4xy^3+g(x)$ \\
  $v_x=12x^2y-4y^3+g'(x)=-u_y$ \\
  $u_y=-12x^2y+4y^3$ \\
  $12x^2-4y^3+g'(x)=12x^2y-4y^3$ \\
  $g'(x)=0$ \\
  $g(x)=C$ \\

  $v(x,y)=4x^3y-4xy^3+C$
\end{example}

To find $f(z)$ from $u(x,y)$ and $v(x,y)$, use:
\[x=\frac{z+\bar{z}}{2}\]
\[y=\frac{z-\bar{z}}{2i}\]
This can be very tedious. For the above example, the answer would be:
\[f(x)=z^4+iC\]

As an alternative, use the Milne-Thompson formula:

\begin{theorem}
  Let $f(z)=u(x,y)+iv(x,y)$ be analytic in a domain $D$ such that
  $z_0=x_0+iy_0\in D$:
  \[f(z)=2u\left(\frac{z+\conj{z_0}}{2},\frac{z-\conj{z_0}}{2i}\right)-
  u(x_0,y_0)+iC,\hspace{0.25in}C\in\R\]
\end{theorem}

\begin{theproof}
  $u(x,y)=\frac{1}{2}\left[f(z)+\Conj{f(z)}\right]=
  \frac{1}{2}\left[f(z)+\conj{f}(\conj{z})\right]=
  \frac{1}{2}\left[f(x+iy)+\conj{f}(x-iy)\right]$

  Let $x=\frac{z+\Conj{z_0}}{2}$ and $y=\frac{z-\Conj{z_0}}{2i}$:
  \begin{eqnarray*}
    u\left(\frac{z+\Conj{z_0}}{2},\frac{z-\Conj{z_0}}{2i}\right) &=&
    \frac{1}{2}\left[f(\frac{z+\Conj{z_0}}{2}+i\frac{z-\Conj{z_0}}{2i})+
      \conj{f}(\frac{z+\Conj{z_0}}{2}-i\frac{z-\Conj{z_0}}{2i})\right] \\
    &=& \frac{1}{2}\left[f(z)+\conj{f}(\Conj{z_0})\right] \\
  \end{eqnarray*}
  \begin{eqnarray*}
    2u\left(\frac{z+\Conj{z_0}}{2},\frac{z-\Conj{z_0}}{2i}\right) &=&
    f(z)+\conj{f}\left(\Conj{z_0}\right) \\
    &=& f(z)+\Conj{f(z_0)} \\
    &=& f(z)+u(x_0,y_0)-iv(x_0,y_0) \\
  \end{eqnarray*}
  Let $v(x_0,y_0)=C\in\R$:
  \[f(z)=2u\left(\frac{z+\Conj{z_0}}{2},\frac{z-\Conj{z_0}}{2i}\right)
  -u(x_0,y_0)+iC\]
\end{theproof}

\begin{example}
  Continuing with the above example with $z_0=0$:
  \begin{eqnarray*}
    f(z) &=& 2u\left(\frac{z}{2},\frac{z}{2i}\right)-u(0,0)+iC \\
    &=& 2\left[\left(\frac{z}{2}\right)^4-
      6\left(\frac{z}{2}\right)^2\left(\frac{z}{2i}\right)^2+
      \left(\frac{z}{2i}\right)^4\right]-0+iC \\
    &=& 2\left(\frac{z^4}{16}+\frac{6z^4}{16}+\frac{z^4}{16}\right)+iC \\
    &=& 2\left(\frac{8z^4}{16}\right)+iC \\
    &=& z^4+iC \\
  \end{eqnarray*}
\end{example}

\begin{theorem}
  Let $f(z)=u(x,y)+iv(x,y)$ be analytic in a domain $D$ such that
  $z_0=x_0+iy_0\in D$:
  \[f(z)=2iv\left(\frac{z+\conj{z_0}}{2},\frac{z-\conj{z_0}}{2i}\right)-
  iv(x_0,y_0)+C,\hspace{0.25in}C\in\R\]
\end{theorem}

\begin{theproof}
  Let $f(z)=u+iv$:
  \begin{eqnarray*}
    if(z) &=& -v+iu \\
    if(z) &=& -2v\left(\frac{z+\Conj{z_0}}{2},\frac{z-\Conj{z_0}}{2i}\right)
    +v(x_0,y_0)+iC \\
    f(z) &=& 2iv\left(\frac{z+\Conj{z_0}}{2},\frac{z-\Conj{z_0}}{2i}\right)
    -iv(x_0,y_0)+C \\
  \end{eqnarray*}
\end{theproof}
\newpage
If $u-v$ is known then:
\[(1+i)(u+iv)=u+iv+iu-v=(u-v)+i(u+v)\]
So, perform the following steps:
\begin{enumerate}
\item Let $F(z)=(1+i)f(z)=(u-v)+i(u+v)$
\item Perform M-T on $F(z)$
\item Divide the result by $1+i$
\end{enumerate}

\begin{theorem}
  Let $f(z)=f(x+iy)=u(x,y)+iv(x,y)$ be analytic in $D$ such that $0\in D$:
  \[f(z)=u(z,0)+i(v,0)\]
\end{theorem}

\begin{theproof}
  $u(x,y)=\frac{1}{2}[f(z)+\Conj{f(z)}]=\frac{1}{2}[f(z)+\conj{f}(\conj{z})]=
  \frac{1}{2}[f(x+iy)+\conj{f}(x-iy)]$ \\
  $v(x,y)=\frac{1}{2i}[f(z)-\Conj{f(z)}]=\frac{1}{2i}[f(z)-\conj{f}(\conj{z})]=
  \frac{1}{2i}[f(x+iy)-\conj{f}(x-iy)]$

  Let $x=z$ and $y=0$

  $u(z,0)=\frac{1}{2}[f(z)+\conj{f}(z)]$ \\
  $v(z,0)=\frac{1}{2i}[f(z)-\conj{f}(z)]$

  $\therefore f(z)=u(z,0)+iv(z,0)$
\end{theproof}

\begin{example}
  $f(z)=(x^2-y^2)+i2xy$

  $u(z,0)=z^2$ \\
  $v(z,0)=0$

  $f(z)=z^2+i0=z^2$
\end{example}

\begin{theorem}
  Let $f(z)=f(x+iy)=u(x,y)+iv(x,y)$ be analytic in $D$ such that $0\in D$:
  \[f(z)=\int\left[u_x(z,0)-iu_y(z,0)\right]dz+C\]
\end{theorem}

\begin{theproof}
  $f'(z)=f_x=u_x+iv_x=u_x-iu_y$

  Let $x=z$ and $y=0$

  $f'(z)=u_x(z,0)-iu_y(z,0)$ \\
  $\therefore f(z)=\int\left[u_x(z,0)-iu_y(z,0)\right]dz+C$
\end{theproof}

\begin{example}
  $f(z)=(x^2-y^2)+i2xy$

  $u_x=2x$ \\
  $u_y=-2y$

  $u_x(z,0)=2z$ \\
  $u_y(z,0)=0$

  $f(z)=\int 2zdz=z^2+C$
\end{example}

\end{document}
