\documentclass[letterpaper,12pt,fleqn]{article}
\usepackage{matharticle}
\usepackage{siunitx}
\usepackage{cancel}
\pagestyle{plain}
\begin{document}

\begin{center}
  \large
  Math-13 Sections 01 and 02

  \Large
  Homework \#4 Solutions

  \large
  \textbf{Due: Midnight 9/25}
\end{center}

\begin{enumerate}
\item Determine the following limit:
  \begin{align*}
    \lim_{x\to\frac{1}{2}}\frac{2x^3+9x^2-5x}{4x^2-1} &= \lim_{x\to\frac{1}{2}}\frac{x(2x^2+9x-5)}{(2x+1)(2x-1)} \\
    &= \lim_{x\to\frac{1}{2}}\frac{x\cancel{(2x-1)}(x+5))}{(2x+1)\cancel{(2x-1)}} \\
    &= \lim_{x\to\frac{1}{2}}\frac{x(x+5)}{2x+1} \\
    &= \frac{\frac{1}{2}\left(\frac{1}{2}+5\right)}{2\left(\frac{1}{2}\right)+1} \\
    &= \frac{\frac{1}{2}\left(\frac{11}{2}\right)}{1+1} \\
    &= \frac{\frac{11}{4}}{2} \\
    &= \frac{11}{8}
  \end{align*}

\item Determine the following limit:
  \begin{align*}  
    \lim_{h\to0}\frac{\sqrt{x+h}-\sqrt{x}}{h}
    &= \lim_{h\to0}\left[\left(\frac{\sqrt{x+h}-\sqrt{x}}{h}\right)
      \left(\frac{\sqrt{x+h}+\sqrt{x}}{\sqrt{x+h}+\sqrt{x}}\right)\right] \\
    &= \lim_{h\to0}\frac{(\cancel{x}+h)-\cancel{x}}{h(\sqrt{x+h}+\sqrt{x})} \\
    &= \lim_{h\to0}\frac{\cancel{h}}{\cancel{h}(\sqrt{x+h}+\sqrt{x})} \\
    &= \lim_{h\to0}\frac{1}{\sqrt{x+h}+\sqrt{x}} \\
    &= \frac{1}{\sqrt{x+0}+\sqrt{x}} \\
    &= \frac{1}{\sqrt{x}+\sqrt{x}} \\
    &= \frac{1}{2\sqrt{x}}
  \end{align*}
\end{enumerate}

\end{document}
