\documentclass[letterpaper,12pt,fleqn]{article}
\usepackage{matharticle}
\pagestyle{empty}
\begin{document}
\subsection*{Complex Field}

\begin{theorem}
$\C$ is a field with:
\begin{itemize}
\item additive identity: $0=(0,0)$
\item additive inverse: $-z=(-x,-y)$
\item multiplicative identity: $1=(1,0)$
\item multiplicative inverse:
    $z^{-1}=\left(\frac{x}{x^2+y^2},\frac{-y}{x^2+y^2}\right)$
\end{itemize}
\end{theorem}

\begin{theproof}
\listbreak
\begin{enumerate}
\item Additive Commutivity
\begin{eqnarray*}
z_1+z_2 &=& (x_1+iy_1)+(x_2+iy_2) \\
    &=& (x_1+x_2)+i(y_1+y_2) \\
    &=& (x_2+x_1)+i(y_2+y_1) \\
    &=& (x_2+iy_2)+(x_1+iy_1) \\
    &=& z_2+z_1 \\
\end{eqnarray*}

\item Additive Associativity
\begin{eqnarray*}
(z_1+z_2)+z_3 &=& [(x_1+iy_1)+(x_2+iy_2)]+(x_3+iy_3) \\
    &=& [(x_1+x_2)+i(y_1+y_2)]+(x_3+iy_3) \\
    &=& [(x_1+x_2)+x_3]+i[(y_1+y_2)+y_3] \\
    &=& [x_1+(x_2+x_3)]+i[y_1+(y_2+y_3)] \\
    &=& (x_1+iy_1)+[(x_2+x_3)+i(y_2+y_3)] \\
    &=& (x_1+iy_1)+[(x_2+iy_2)+(x_3+iy_3)] \\
    &=& z_1+(z_2+z_3) \\
\end{eqnarray*}

\item Additive Identity
\begin{eqnarray*}
z+0 &=& (x+iy)+(0+i0) \\
    &=& (x+0)+i(y+0) \\
    &=& x+iy \\
    &=& z \\
\end{eqnarray*}

\item Additive Inverse
\begin{eqnarray*}
z+(-z) &=& 0 \\
(x+iy)+(u+iv) &=& 0+i0 \\
(x+u)+i(y+v) &=& 0+i0 \\
x+u &=& 0 \\
y+v &=& 0 \\
u &=& -x \\
v &=& -y \\
\end{eqnarray*}
\[\therefore\forall z\in\C,\exists(-z)=(-x,-y),z+(-z)=0\]

\item Multiplicative Commutivity
\begin{eqnarray*}
z_1z_2 &=& (x_1+iy_1)(x_2+iy_2) \\
    &=& (x_1x_2-y_1y_2)+i(x_1y_2+x_2y_1) \\
    &=& (x_2x_1-y_2y_1)+i(x_2y_1+x_1y_2) \\
    &=& (x_2+iy_2)(x_1+iy_1) \\
    &=& z_2z_1 \\
\end{eqnarray*}

\item Multiplicative Associativity
\begin{eqnarray*}
(z_1z_2)z_2 &=& [(x_1+iy_1)(x_2+iy_2)](x_3+iy_3) \\
    &=& [(x_1x_2-y_1y_2)+i(x_1y_2+x_2y_1)](x_3+iy_3) \\
    &=& [(x_1x_2-y_1y_2)x_3-(x_1y_2+x_2y_1)y_3]+
        i[(x_1x_2-y_1y_2)y_3+(x_1y_2+x_2y_1)x_3] \\
    &=& (x_1x_2x_3-y_1y_2x_3-x_1y_2y_3-x_2y_1y_3)+
        i(x_1x_2y_3-y_1y_2y_3+x_1y_2x_3+x_2y_1x_3) \\
    &=& [x_1(x_2x_3-y_2y_3)-y_1(x_2y_3+x_3y_2)]+
        i[x_1(x_2y_3+x_3y_2)+y_1(x_2x_3-y_2y_3)] \\
    &=& (x_1+iy_1)[(x_2x_3-y_2y_3)+i(x_2y_3+x_3y_2)] \\
    &=& (x_1+iy_1)[(x_2+iy_2)(x_3+iy_3)] \\
    &=& z_1(z_2z_3) \\
\end{eqnarray*}

\item Multiplicative Identity
\begin{eqnarray*}
1z &=& (1+i0)(x+iy) \\
    &=& (x-0)+i(y+0) \\
    &=& x+iy \\
    &=& z \\
\end{eqnarray*}

\item Multiplicative Inverse
\allowdisplaybreaks
\begin{eqnarray*}
zz^{-1} &=& 1 \\
(x+iy)(u+iv) &=& 1+i0 \\
(xu-yv)+i(xv+yu) &=& 1+i0 \\
xu-yv &=& 1 \\
yu+xv &=& 0 \\
u &=& \frac{\abs{\begin{array}{cc}1 & -y \\ 0 & x\end{array}}}
    {\abs{\begin{array}{cc}x & -y \\ y & x\end{array}}}=\frac{x}{x^2+y^2} \\
v &=& \frac{\abs{\begin{array}{cc}x & 1 \\ y & 0\end{array}}}
    {\abs{\begin{array}{cc}x & -y \\ y & x\end{array}}}=\frac{-y}{x^2+y^2} \\
\end{eqnarray*}
\[\therefore \forall z\in\C-\{0\},
    \exists z^{-1}=\left(\frac{x}{x^2+y^2},\frac{-y}{x^2+y^2}\right),zz^{-1}=1\]

\item Distribution
\begin{eqnarray*}
z_1(z_2+z_3) &=& (x_1+iy_1)[(x_2+iy_2)+(x_3+iy_3)] \\
    &=& (x_1+iy_1)[(x_2+x_3)+i(y_2+y_3)] \\
    &=& [x_1(x_2+x_3)-y_1(y_2+y_3)]+i[x_1(y_2+y_3)+y_1(x_2+x_3)] \\
    &=& (x_1x_2+x_1x_3-y_1y_2-y_1y_3)+i(x_1y_2+x_1y_3+y_1x_2+y_1x_3) \\
    &=& [(x_1x_2-y_1y_2)+i(x_1y_2+y_1x_2)]+[(x_1x_3-y_1y_2)+i(x_1y_2+y_1x_3)] \\
    &=& (x_1+iy_1)(x_2+iy_2)+(x_1+iy_1)(x_3+iy_3) \\
    &=& z_1z_2+z_1z_3 \\
\end{eqnarray*}
\end{enumerate}
\end{theproof}

Since $\C$ is a field, all of the following properties also hold:
\begin{enumerate}
\item Uniqueness
\begin{enumerate}
\item The additive identity ($0$) is unique.
\item Additive inverses ($-z$) are unique.
\item The multiplicative identity ($1$) is unique.
\item Multiplicative inverses ($z^{-1}$) are unique.
\end{enumerate}
\newpage
\item Properties of 0
\begin{enumerate}
\item $0=-0$
\item $z0=0$
\item $z_1z_2=0\iff z_1=0$ or $z_2=0$
\end{enumerate}
\item Properties of Additive Inverses
\begin{enumerate}
\item $-z=(-1)z$
\item $-(-z)=z$
\item $(-z_1)z_2=z_1(-z_2)=-(z_1z_2)$
\item $(-z_1)(-z_2)=z_1z_2$
\item $-(z_1+z_2)=-z_1+(-z_2)$
\end{enumerate}
\end{enumerate}

\end{document}
