\documentclass[letterpaper,12pt,fleqn]{article}
\usepackage{matharticle}
\pagestyle{empty}
\newcommand{\Rd}{\mathbb{R}^d}
\newcommand{\LtwoRd}{L^2(\Rd)}
\newcommand{\abs}[1]{\left|#1\right|}
\newcommand{\norm}[1]{\lVert#1\rVert}
\newcommand{\inner}[2]{\langle#1,#2\rangle}
\newcommand{\conj}[1]{\bar{#1}}
\newcommand{\Conj}[1]{\overline{#1}}
\newcommand{\hilb}{\mathcal{H}}
\begin{document}
\section*{Orthogonality}

\begin{definition}
Let $\hilb$ be a Hilbert space and let $f,g\in\hilb$. To say that $f$ is
orthogonal (perpendicular) to $g$, denoted $f\perp g$, means that
$\inner{f}{g}=0$.
\end{definition}

\begin{lemma}
$f\perp g\iff g\perp f$
\end{lemma}

\begin{theproof}
$f\perp g\iff\inner{f}{g}=0\iff\Conj{\inner{g}{f}}=0\iff\inner{g}{f}=0\iff
    g\perp f$
\end{theproof}

\begin{theorem}
$f\perp g\implies\norm{f+g}^2=\norm{f}^2+\norm{g}^2$
\end{theorem}

\begin{theproof}
Assume $f\perp g$ \\
$\inner{f}{g}=\inner{g}{f}=0$ \\
\begin{eqnarray*}
\norm{f+g}^2 &=& \inner{f+g}{f+g} \\
    &=& \inner{f}{f}+\inner{f}{g}+\inner{g}{f}+\inner{g}{g} \\
    &=& \norm{f}^2+0+0+\norm{g}^2 \\
    &=& \norm{f}^2+\norm{g}^2 \\
\end{eqnarray*}
\end{theproof}

\begin{definition}
Let $\hilb$ be a Hilbert space. To say that $\{e_1,e_2,\ldots\}\subset\hilb$ is
orthonormal means:
\[\inner{e_j}{e_k}=\begin{cases}
1, & j=k \\
0, & j\ne k \\
\end{cases}\]
In other words, every element has a norm of 1 and is orthogonal to every other
element.
\end{definition}

\begin{theorem}
Let $\hilb$ be a Hilbert space, $\{e_k\}_{k=1}^{\infty}\subset\hilb$ be
orthonormal, and $f=\sum a_ke_k\in\hilb$ be a finite sum.
\[\norm{f}^2=\sum\abs{a_k}^2\]
\end{theorem}

\begin{theproof}
$\norm{f}^2=\inner{f}{f}=\inner{\sum a_je_j}{\sum a_ke_k}$ \\

Each term in the linear expansion is one of the following two forms:
\begin{enumerate}
\item{$j=k$}

$\inner{a_ke_k}{a_ke_k}=\abs{a_k}^2\inner{e_k}{e_k}=\abs{a_k}^2\cdot1=\abs{a_k}^2$

\item{$j\ne k$}

$\inner{a_je_j}{a_ke_k}=a_j\Conj{a_k}\inner{e_j}{e_k}=a_j\Conj{a_k}\cdot0=0$
\end{enumerate}

$\therefore \norm{f}^2=\sum\abs{a_k}^2$
\end{theproof}

\end{document}
