\documentclass[letterpaper,12pt,fleqn]{article}
\usepackage{matharticle}
\pagestyle{empty}
\newcommand{\Rd}{\mathbb{R}^d}
\newcommand{\LtwoRd}{L^2(\mathbb{R}^d)}
\newcommand{\abs}[1]{\left|#1\right|}
\newcommand{\norm}[1]{\lVert#1\rVert}
\newcommand{\inner}[2]{\langle#1,#2\rangle}
\newcommand{\conj}[1]{\bar{#1}}
\newcommand{\Conj}[1]{\overline{#1}}
\begin{document}

\section*{L\textsuperscript2 Norm}

\begin{theorem}
$\norm{\cdot}$ is a proper norm for $L^2$
\end{theorem}

\begin{theproof}
\listbreak
\begin{description}
\item{N1:} Assume $f\in L^2$

$\norm{f}=0\iff f=0\;\; a.e.\qquad(property)$ \\
Note that, once again, we are dealing with equivalence classes, where: \\
$f\sim g$ means $f=g\;\;a.e.$

\item{N2:} Assume $f\in L^2$ and $\alpha\in\mathbb{C}$

$\norm{\alpha f}=\left(\int\abs{\alpha f}^2\right)^{\frac{1}{2}}=
    \left(\abs{\alpha}^2\int\abs{f}^2\right)^{\frac{1}{2}}=
    \abs{\alpha}\left(\int\abs{f}^2\right)^{\frac{1}{2}}=
    \abs{\alpha}\norm{f}$

\item{N3:} Assume $f,g\in L^2$
\[\begin{array}{rcl}
\norm{f+g}^2 &=& \int\abs{f+g}^2 \\
    &=& \int(f+g)\Conj{(f+g)} \\
    &=& \int(f+g)(\conj{f}+\conj{g}) \\
    &=& \int(f\conj{f}+g\conj{g}+f\conj{g}+g\conj{f}) \\
    &=& \int\abs{f}^2+\int\abs{g}^2+\int f\conj{g}+\int g\conj{f}) \\
    &=& \norm{f}^2+\norm{g}^2+\inner{f}{g}+\inner{g}{f} \\
    &\le& \norm{f}^2+\norm{g}^2+\norm{f}\norm{g}+\norm{g}\norm{f} \\
    &=& \norm{f}^2+\norm{g}^2+2\norm{f}\norm{g} \\
    &=& \left(\norm{f}+\norm{g}\right)^2 \\
\end{array}\]

$\therefore \norm{f+g}\le\norm{f}+\norm{g}$
\end{description}
\end{theproof}

\end{document}
