\documentclass[letterpaper,12pt,fleqn]{article}
\usepackage{matharticle}
\pagestyle{empty}
\renewcommand{\l}{\lambda}
\newcommand{\m}{\mu}
\renewcommand{\o}{\sigma}
\twocolumn
\begin{document}

\subsubsection*{Derivatives}

\begin{gather*}
  \frac{d}{dx}\left[c\right]=0 \\
  \frac{d}{dx}\left[x^c\right]=cx^{c-1} \\
  \frac{d}{dx}\left[cf(x)\right]=cf'(x) \\
  \frac{d}{dx}\left[f(x)\pm g(x)\right]=f'(x)\pm g'(x) \\
  \frac{d}{dx}\left[f(x)g(x)\right]=f(x)g'(x)+f'(x)g(x) \\
  \frac{d}{dx}\left[\frac{f(x)}{g(x)}\right]=\frac{g(x)f'(x)-g'(x)f(x)}{[g(x)]^2} \\
  \frac{d}{dx}\left[f(u(x))\right]=f'(u)u'(x) \\
  \frac{d}{dx}\left[\frac{1}{x}\right]=-\frac{1}{x^2} \\
  \frac{d}{dx}\left[e^x\right]=e^x \\
  \frac{d}{dx}\left[e^{u(x)}\right]=e^{u(x)}u'(x) \\
  \frac{d}{dx}\left[a^x\right]=a^x\ln(a) \\
  \frac{d}{dx}\left[a^{u(x)}\right]=a^{u(x)}u'(x)\ln(a) \\
  \frac{d}{dx}\left[\ln(x)\right]=\frac{1}{x} \\
  \frac{d}{dx}\left[\ln(u(x))\right]=\frac{u'(x)}{u(x)} \\
  \frac{d}{dx}\left[\log_a(x)\right]=\frac{1}{\ln(a)}\cdot\frac{1}{x} \\
  \frac{d}{dx}\left[\log_a(u(x))\right]=\frac{1}{\ln(a)}\cdot\frac{u'(x)}{u(x)}
\end{gather*}

\subsection*{Probability}

\[p(x)=\frac{1}{\o\sqrt{2\pi}}e^{\frac{-(x-\m)^2}{2\o^2}}\]
68--95--99.7 rule

\subsubsection*{First/Second Derivative Tests}

\begin{tabular}{|l|l|l|}
  \hline
  & \(<0\) & \(>0\) \\
  \hline
  \(f'(x)\) & decreasing & increasing \\
  \hline
  \(f''(x)\) & concave down & concave up \\
  \hline
\end{tabular}

\subsubsection*{Second Partial Derivative Test}

\[f_x=0\ \text{and}\ f_y=0\]
\[d=f_{xx}f_{yy}-[f_{xy}]^2\]
\begin{tabular}{c|c|c}
  \(d\) & \(f_{xx}\) & result \\
  \hline
  \(>0\) & \(>0\) & relative minimum \\
  \(>0\) & \(<0\) & relative maximum \\
  \(<0\) & & saddle point \\
  \(=0\) & & inconclusive
\end{tabular}

\subsubsection*{Lagrange Multiplier}

\begin{gather*}
f_x=\l g_x \\
f_y=\l g_y \\
\vdots \\
g(x,y,\ldots)=0
\end{gather*}

\subsubsection*{Interest}

\begin{tabular}{ll}
  Compound Interest & \(A=P\left(1+\frac{r}{n}\right)^{nt}\) \\
  Population Growth & \(P(t)=P(0)e^{rt}\) \\
  Radioactive Decay & \(m(t)=m(0)e^{-\frac{t\ln(2)}{h_0}}\)
\end{tabular}

\subsubsection*{Logarithms}

\begin{gather*}
  \ln(1)=0 \\
  \ln(e)=1 \\
  e^{\ln(x)}=x \\
  \ln(e^x)=x \\
  e^x=e^y\iff x=y \\
  \ln(x)=\ln(y)\iff x=y \\
  \ln(xy)=\ln(x)+\ln(y) \\
  \ln\left(\frac{x}{y}\right)=\ln(x)-\ln(y) \\
  \ln\left(x^y\right)=y\ln(x)
\end{gather*}

\end{document}
