\documentclass[letterpaper,12pt,fleqn]{article}
\usepackage{matharticle}
\pagestyle{empty}
\newcommand{\inner}[2]{\left<#1,#2\right>}
\newcommand{\vx}{\vec{x}}
\newcommand{\vy}{\vec{y}}
\newcommand{\vz}{\vec{z}}
\newcommand{\vo}{\vec{0}}
\newcommand{\conj}[1]{\overline{#1}}
\begin{document}
\section*{Inner Product}

\begin{definition}[Inner Product]
  Let $V$ be a vector space over a field $F$. To say that a function
  $\inner{\cdot}{\cdot}:V\times V\to F$ is an \emph{inner product} on $V$ means that it
  satisfies the following five properties $\forall\,\vx,\vy\in V$ and $\forall\,c\in F$:
  \begin{enumerate}
  \item Nonnegativity: $\inner{\vx}{\vx}\ge0$
  \item Positivity: $\inner{\vx}{\vx}=0\iff\vx=\vo$
  \item Additivity: $\inner{\vx+\vy}{\vz}=\inner{\vx}{\vz}+\inner{\vy}{\vz}$
  \item Homogeneity: $\inner{c\vx}{\vy}=c\inner{\vx}{\vy}$
  \item Hermitian: $\inner{\vx}{\vy}=\conj{\inner{\vy}{\vx}}$
  \end{enumerate}
\end{definition}

\begin{properties}[Inner Product]
  \listbreak
  \begin{enumerate}
  \item $\inner{\vx}{c\vy}=\conj{c}\inner{\vx}{\vy}$
  \item $\inner{\vx}{\vy+\vz}=\inner{\vx}{\vy}+\inner{\vx}{\vz}$
  \item $\conj{\inner{\vx}{\vx}}=\inner{\vx}{\vx}$
  \end{enumerate}
\end{properties}

\begin{theproof}
  \listbreak
  \begin{enumerate}
  \item $\inner{\vx}{c\vy}=\conj{\inner{c\vy}{\vx}}=\conj{c\inner{\vy}{\vx}}=
    \conj{c}\conj{\inner{\vy}{\vx}}=\conj{c}\inner{\vx}{\vy}$

  \item $\inner{\vx}{\vy+\vz}=\conj{\inner{\vy+\vz}{\vx}}=
    \conj{\inner{\vy}{\vx}+\inner{\vz}{\vx}}=
    \conj{\inner{\vy}{\vx}}+\conj{\inner{\vz}{\vx}}=
    \inner{\vx}{\vy}+\inner{\vx}{\vz}$

  \item Trivial
  \end{enumerate}
\end{theproof}

\begin{theorem}[Cauchy-Schwarz]
  Let $\vx,\vy\in\C^n$:
  \[\abs{\inner{\vx}{\vy}}^2\le\inner{\vx}{\vx}\inner{\vy}{\vy}\]
\end{theorem}

\begin{theproof}
  If $\vx=\vy=\vo$ then there is nothing to prove, so AWLOG: $\vy\ne\vo$ \\
  Let $\vz=\inner{\vy}{\vy}\vx-\inner{\vx}{\vy}\vy$:
  \begin{eqnarray*}
    0 &\le& \inner{\vz}{\vz} \\
    &=& \inner{\inner{\vy}{\vy}\vx-\inner{\vx}{\vy}\vy}
    {\inner{\vy}{\vy}\vx-\inner{\vx}{\vy}\vy} \\
    &=& \inner{\vy}{\vy}\conj{\inner{\vy}{\vy}}\inner{\vx}{\vx}-
    \inner{\vy}{\vy}\conj{\inner{\vx}{\vy}}\inner{\vx}{\vy}-
    \inner{\vx}{\vy}\conj{\inner{\vy}{\vy}}\inner{\vy}{\vx}+
    \inner{\vx}{\vy}\conj{\inner{\vx}{\vy}}\inner{\vy}{\vy} \\
    &=& \inner{\vy}{\vy}\inner{\vy}{\vy}\inner{\vx}{\vx}-
    \inner{\vy}{\vy}\inner{\vx}{\vy}\conj{\inner{\vx}{\vy}}-
    \inner{\vx}{\vy}\conj{\inner{\vx}{\vy}}\inner{\vy}{\vy}+
    \inner{\vx}{\vy}\conj{\inner{\vx}{\vy}}\inner{\vy}{\vy} \\
    &=& \inner{\vy}{\vy}^2\inner{\vx}{\vx}-\inner{\vy}{\vy}\abs{\inner{\vx}{\vy}}^2 \\
    &=& \inner{\vy}{\vy}(\inner{\vy}{\vy}\inner{\vx}{\vx}-\abs{\inner{\vx}{\vy}}^2)
  \end{eqnarray*}
  But, by assumption, $\vy\ne\vo$, and so:
  \[\inner{\vx}{\vx}\inner{\vy}{\vy}-\abs{\inner{\vx}{\vy}}^2\ge0\]
  $\therefore\abs{\inner{\vx}{\vy}}^2\le\inner{\vx}{\vx}\inner{\vy}{\vy}$
\end{theproof}

\begin{example}
  The standard inner product:
  \[\inner{\vx}{\vy}=\vy^{\,*}\vx=\sum_{k=1}^n\conj{y_k}x_k\]
\end{example}

\begin{definition}[Special Matrices]
  To say that a matrix $A\in M_n$ is \emph{Hermitian} means $A=A^*$.

  To say that a matrix $A\in M_n$ is \emph{positive-definite} means:
  \begin{enumerate}
    \item $A$ is Hermitian
    \item $\forall\,\vx\ne0,\vx^{\,*}A\vx>0$
  \end{enumerate}
\end{definition}

\begin{theorem}
  Any inner product on $C^n$ is of the form:
  \[\inner{\vx}{\vy}=\vy^{\,*}A\vx\]
  for some positive-definite matrix $A$.
\end{theorem}

\begin{example}
  \newcommand{\MA}{
    \begin{bmatrix} \pi & 0 & 0 \\ 0 & e & 0 \\ 0 & 0 & \sqrt{2} \end{bmatrix}
  }

  $A=\MA$

  Note that $A$ is real-diagonal and thus Hermitian.

  Assume $\vx\ne0$:
  \[\vx^{\,*}A\vx=\begin{bmatrix} \conj{x_1} & \conj{x_2} & \conj{x_3} \end{bmatrix}\MA
    \begin{bmatrix} x_1 \\ x_2 \\ x_3 \end{bmatrix}=
    \begin{bmatrix} \conj{x_1}\pi & \conj{x_2}e & \conj{x_3}\sqrt{2} \end{bmatrix}=
    \begin{bmatrix} x_1 \\ x_2 \\ x_3 \end{bmatrix}\]
  \[\vx^{\,*}A\vx=\pi\abs{x_1}^2+e\abs{x_2}^2+\sqrt{2}\abs{x_3}^2\ge0\]
  Thus $A$ is positive-definite.

  $\inner{\vx}{\vy}=\pi\conj{y_1}x_1+e\conj{y_2}x_2+\sqrt{2}\conj{y_3}x_3$
\end{example}

\end{document}
