\documentclass[letterpaper]{article}

\setlength{\topmargin}{0in}
\setlength{\headheight}{0in}
\setlength{\headsep}{0in}
\setlength{\footskip}{0.5in}
\setlength{\textheight}{\paperheight}
\addtolength{\textheight}{-2in}
\addtolength{\textheight}{-\footskip}

\setlength{\oddsidemargin}{0in}
\setlength{\evensidemargin}{0in}
\setlength{\textwidth}{\paperwidth}
\addtolength{\textwidth}{-2in}

\pagestyle{empty}

\begin{document}

\begin{center}
\bfseries
San Jos\'{e} State University \\
Fall 2015 \\
Math-8: College Algebra \\
Section 03: MW noon--1:15pm \\
Section 05: MW 4:30pm-5:45pm \\
\bigskip
Homework Week 3 Solutions
\end{center}

\underline{\textbf{Section 0.3}}

\bigskip

2. $3\cdot3^5=3^1\cdot3^5=3^{1+5}=3^6$

\bigskip

4. $\frac{5^7}{5^5}=5^{7-5}=5^2=25$

\bigskip

6. $(2^5)^3=2^{5\cdot3}=2^{15}$

\bigskip

8. $(-3)^4=((-1)3)^4=(-1)^43^4=(1)3^4=3^4=81$

\bigskip

10. $(-3\cdot4^2)^3=(-3)^3(4^2)^3=-3^34^{2\cdot3}=-3^34^6$

\bigskip

12.

\begin{eqnarray*}
\left(\frac{-5}{4}\right)^3\left(\frac{4}{5}\right)^2 &=&
    \left(\frac{(-5)^3}{4^3}\right)\left(\frac{4^2}{5^2}\right) \\
    &=& \left(-\frac{5^3}{4^3}\right)\left(\frac{4^2}{5^2}\right) \\
    &=& -\frac{5^34^2}{4^35^2} \\
    &=& -\frac{5^34^2}{5^24^3} \\
    &=& -\left(\frac{5^3}{5^2}\right)\left(\frac{4^2}{4^3}\right) \\
    &=& -(5^{3-2})(4^{2-3}) \\
    &=& -(5^1)(4^{-1}) \\
    &=& -\frac{5}{4} \\
\end{eqnarray*}

14. $(-2)^0=1$

\bigskip

16. $(-2w)^5=(-2)^5w^5=-32w^5$

\bigskip

18. $5x^4(x^2)=5(x^4x^2)=5x^{4+2}=5x^6$

\bigskip

20. $2(4x^4)^3=2(4^3)((x^4)^3)=2(64)(x^{4\cdot3})=128x^{12}$

\bigskip

22. $(6y^2)(2y^3)^3=(6y^2)(2^3(y^3)^3)=(6y^2)(8y^{3\cdot3})=(6y^2)(8y^9)=
    (6\cdot8)y^{2+9}=48y^{11}$

\bigskip

24. $\frac{10x^9}{4x^6}=\frac{2\cdot5x^9}{2^2x^6}=\frac{5x^3}{2}=\frac{5}{2}x^3$

\bigskip

26. $\left(\frac{5}{z}\right)^2\left(\frac{2}{z}\right)^3=
     \left(\frac{5^2}{z^2}\right)\left(\frac{2^3}{z^3}\right)=
     \frac{5^22^3}{z^2z^3}=
     \frac{25\cdot8}{z^{2+3}}=
     \frac{200}{z^5}$

\bigskip

28. $\frac{5z^5}{z^7}=\frac{5}{z^2}$

\bigskip

30. $\frac{x^n\cdot x^{2n}}{x^{3n}}=\frac{x^{n+2n}}{x^{3n}}=\frac{x^{3n}}{x^{3n}}=
     x^{3n-3n}=x^0=1$

\bigskip

32. $2^m\cdot2^{3m}=2^{m+3m}=2^{4m}=(2^4)^m=16^m$

\bigskip

34. $\frac{24(x-2)^5}{8(x-2)^4}=\frac{8\cdot3(x-2)^5}{8(x-2)^4}=3(x-2)$

\bigskip

36. $(x+5)^0=1\hspace{0.5in}(x\ne-5)$

\bigskip

38. $6\cdot2^{-3}\cdot3^{-1}=\frac{6}{2^3\cdot3}=\frac{2\cdot3}{2^3\cdot3}=
     \left(\frac{2}{2^3}\right)\left(\frac{3}{3}\right)=\frac{1}{2^2}\cdot1=
     \frac{1}{4}$

\bigskip

40. $\left(\frac{2}{3}\right)^{-3}=\left(\frac{3}{2}\right)^3=\frac{3^3}{2^3}=
     \frac{27}{8}$

\bigskip

42. $4^{-1}-2^{-2}=\frac{1}{4}-\frac{1}{2^2}=\frac{1}{4}-\frac{1}{4}= 0$

\bigskip

44. $-7x^{-1}=-\frac{7}{x}$

\bigskip

46. $\frac{10x^4y^{-4}}{5x^2y^{-2}}=
     \left(\frac{10}{5}\right)\left(\frac{x^4}{x^2}\right)
         \left(\frac{y^{-4}}{y^{-2}}\right)=
     \left(\frac{5\cdot2}{5}\right)x^2y^{-2}=
     \left(2\right)x^2\left(\frac{1}{y^2}\right)=
     \frac{2x^2}{y^2}$

\bigskip

48. $\left(\frac{y}{5}\right)^{-2}=\left(\frac{5}{y}\right)^2=
    \frac{5^2}{y^2}=\frac{25}{y}$

\bigskip

50. $\left(\frac{2z^2}{y}\right)^{-2}=\left(\frac{y}{2z^2}\right)^2=
    \frac{y^2}{(2z^2)^2}=\frac{y^2}{2^2(z^2)^2}=\frac{y^2}{4z^4}$

\bigskip

71. $P=\$10,000$, $r=3.95\%/yr=0.0395/yr$, $n=12yr$

\bigskip

A quick note about units.  Something like ``$12yr$'' means 12 years and
something like ``$0.0395/yr$'' means 0.0395 per year, also sometimes written
$0.0395 yr^{-1}$.  So note that as long as we keep the time units consistent,
the time units will ``cancel'', leaving only the dollar units.  This is often
called unit analysis.

\bigskip

a. $n=365/yr$

\bigskip

$A=\$10,000\left(1+\frac{0.0375/yr}{365/yr}\right)^{12yr\cdot365/yr}=\$15,682.76$

\bigskip

b. $n=52/yr$

\bigskip

$A=\$10,000\left(1+\frac{0.0375/yr}{52/yr}\right)^{12yr\cdot52/yr}=\$15,680.58$

\bigskip

c. $n=12/yr$

\bigskip

$A=\$10,000\left(1+\frac{0.0375/yr}{12/yr}\right)^{12yr\cdot12/yr}=\$15,672.12$

\bigskip

d. $n=4/yr$

\bigskip

$A=\$10,000\left(1+\frac{0.0375/yr}{4/yr}\right)^{12yr\cdot4/yr}=\$15650.28$

\bigskip

Note that the final amount gets smaller as the number of times the interest
compounds in one year decreases.

\bigskip

84. $A=\$1,000,000$, $r=4.5\%/yr=0.045/yr$, $t=21yr$, $n=4/yr$

\bigskip

$P=\frac{\$1,000,000}{\left(1+\frac{0.045/yr}{4/yr}\right)^{21yr\cdot4/yr}}=
    \$390,735.70$

\end{document}
