\documentclass[letterpaper,12pt,fleqn]{article}
\usepackage{matharticle}
\pagestyle{empty}
\newcommand{\vx}{\vec{x}}
\newcommand{\vxct}{\vx^{\,*}}
\newcommand{\ve}{\vec{e}}
\newcommand{\vz}{\vec{0}}
\newcommand{\vu}{\vec{u}}
\newcommand{\conj}[1]{\overline{#1}}
\renewcommand{\o}{\sigma}
\renewcommand{\l}{\lambda}
\DeclareMathOperator{\Imag}{Im}
\DeclareMathOperator{\Real}{Re}
\DeclareMathOperator{\Sp}{Sp}
\begin{document}
\section*{Hermitian Matrices}

\begin{definition}[Hermitian]
  To say that a matrix $A\in M_n$ is \emph{Hermitian (self-adjoint)} means:
  \[A^*=A\]
  To say that $A$ is \emph{skew-Hermitian} means:
  \[A^*=-A\]
\end{definition}

\begin{properties}[Hermitian]
  \listbreak
  \begin{enumerate}
  \item $A,B$ Hermitian $\implies \forall\,a,b\in\R,aA+bB$ Hermitian
  \item $A,B$ skew-Hermitian $\implies \forall\,a,b\in\R,aA+bB$ Hermitian
  \item $A$ Hermitian $\implies iA$ skew-Hermitian
  \item $A$ skew-Hermitian $\implies iA$ Hermitian
  \item $A=[a_{ij}]$ Hermitian $\implies a_{ii}\in\R$
  \item $A=[a_{ij}]$ skew-Hermitian $\implies a_{ii}\in i\R$
  \end{enumerate}
\end{properties}

\begin{theorem}
  Let $A,B\in M_n$ be Hermitian:
  \[AB\ \mbox{Hermitian} \iff AB=BA\]
\end{theorem}

\begin{theproof}
  $A=A^*$ and $B=B^*$ \\
  $AB$ Hermitian $\iff AB=(AB)^* \iff AB=B^*A^* \iff AB=BA$
\end{theproof}

\begin{theorem}
  $A\in M_n$ Hermitian $\iff \forall\,\vx\in\C^n,\vxct A\vx\in\R$
\end{theorem}

\begin{theproof}
  \listbreak
  \begin{description}
  \item $\implies$ Assume $A\in M_n$ is Hermitian

    Note that $\vxct A\vx\in M_1$:
    \[\conj{\vxct A\vx}=(\vxct A\vx)^*=\vxct A^*\vx=\vxct A\vx\]
    $\therefore\vxct A\vx\in\R$

  \item $\impliedby$ Assume $\forall\,\vx\in\C^n,\vxct A\vx\in\R$

    Let $A=[a_{ij}]$ and $A^*=[\conj{a_{ji}}]$
    \begin{description}
    \item Case 1: $i=j$

      Let $\vx=\ve_i$ \\
      $e_i^*Ae_i=a_{ii}\in\R$

      $\therefore a_{ii}=\conj{a_{ii}}$

    \item Case 2: $i\ne j$

      Let $\vx=\ve_i+\ve_j$ \\
      $(\ve_i+\ve_j)^*A(\ve_i+\ve_j)=
      \ve_i^*A\ve_i+\ve_i^*A\ve_j+\ve_j^*A\ve_i+\ve_j^*A\ve_j=
      a_{ii}+a_{ij}+a_{ji}+a_{jj}\in\R$ \\
      But $a_{ii},a_{jj}\in\R$, so $a_{ij}+a_{ji}\in\R$

      $\therefore\Imag(a_{ij})=-\Imag(a_{ji})$

      Now let $\vx=i\ve_i+\ve_j$
      $(i\ve_i+\ve_j)^*A(i\ve_i+\ve_j)=
      \ve_i^*A\ve_i-i\ve_i^*A\ve_j+i\ve_j^*A\ve_i+\ve_j^*A\ve_j=
      a_{ii}+i(-a_{ij}+a_{ji})+a_{jj}\in\R$ \\
      But $a_{ii},a_{jj}\in\R$, so $i(-a_{ij}+a_{ji})\in\R$ \\
      $-a_{ij}+a_{ji}\in i\R$

      $\therefore\Real(a_{ij})=\Real(a_{ji})$
    \end{description}
    Thus, $a_{ij}=\conj{a_{ji}}$ and so $A=A^*$

    Therefore, $A$ is Hermitian.
  \end{description}
\end{theproof}

\begin{theorem}
  Let $A\in M_n$:
  \begin{itemize}
  \item $A$ Hermitian $\implies \o(A)\subseteq\R$
  \item $A$ skew-Hermitian $\implies \o(A)\subseteq i\R$
  \end{itemize}
\end{theorem}

\begin{theproof}
  Assume $A$ is Hermitian \\
  Assume $\l\in\o(A)$ \\
  $\exists\,\vx\ne\vx,A\vx=\l\vx$ \\
  $\l=\vx^*A\vx\in\R$

  $\therefore\o(A)\subseteq\R$

  Assume $A$ is skew-Hermitian \\
  $iA$ is Hermitian \\
  $\o(iA)\subseteq\R$ \\
  $i\o(A)\subseteq\R$ \\
  $-\o(A)\subseteq i\R$ \\

  $\therefore\o(A)\subseteq i\R$
\end{theproof}
\newpage
\begin{theorem}[Spectral Theorem for Hermitian Matrices]
  Let $A\in M_n$ be Hermitian. $A$ is unitary diagonalizable with diagonal
  entries $\{\l_1,\ldots\l_n\}=\Sp(A)\subseteq\R$.
\end{theorem}

\begin{theproof}
  $A$ is Hermitian $\implies A$ is normal $\implies A$ is unitary
  diagonalizable with $\o(A)\subseteq\R$

  Indeed, since $A=U\begin{bmatrix}
  \l_1 & & 0 \\
  & \ddots & \\
  0 & & \l_n
  \end{bmatrix}U^*$

  $AU=U\begin{bmatrix}
  \l_1 & & 0 \\
  & \ddots & \\
  0 & & \l_n
  \end{bmatrix}U^*$

  $A\vu_i=\l_i\vu_i$, so the $\vu_i$ are the eigenvectors of $A$.
\end{theproof}

\end{document}
