\documentclass[letterpaper,12pt,fleqn]{article}
\usepackage{matharticle}
\pagestyle{empty}
\begin{document}
\section*{Polynomials}
\begin{definition}
A \emph{polynomial} in a complex variable $z$ of degree $n\in\N\bigcup\{0\}$ is
given by:
\[p(z)=\sum_{k=0}^{n}a_kz^k, a_k\in\C, a_n\ne0\]
The special case $p(z)=0$ is called the \emph{zero polynomial}.
\end{definition}
Note that for $\abs{z}<R$, $p(z)$ is bounded.
\begin{example}
Let $p(z)=3+z+z^2$ and $\abs{z}<2$.
\begin{eqnarray*}
\abs{p(z)} &=& \abs{3+z+z^2} \\
    &\le& \abs{3}+\abs{z}+\abs{z^2} \\
    &=& 3+\abs{z}+\abs{z}^2 \\
    &<& 3+2+2^2 \\
    &=& 9 \\
\end{eqnarray*}
\end{example}
\begin{theorem}
Let $p(z)$ be a complex polynomial. There exists $R>0$ such that
$\forall \abs{z}<R$:
\[\abs{p(z)}>\frac{\abs{a_n}R^n}{2}\]
and thus:
\[\abs{\frac{1}{p(z)}}<\frac{2}{\abs{a_n}R^n}\]
Thus, $\frac{1}{p(z)}$ is bounded for all $z$ outside the circle
$\abs{z}=R$ for R sufficiently big.
\end{theorem}
\begin{theproof}
Let $w=\sum_{k=0}^{n-1}\frac{a_k}{z^{n-k}}$. \\
$\abs{w}=\abs{\sum_{k=0}^{n-1}\frac{a_k}{z^{n-k}}}\le
    \sum_{k=0}^{n-1}\abs{\frac{a_k}{z^{n-k}}}=
    \sum_{k=0}^{n-1}\frac{\abs{a_k}}{\abs{z^{n-k}}}=
    \sum_{k=0}^{n-1}\frac{\abs{a_k}}{\abs{z}^{n-k}}$ \\
Let $\abs{a_m}=max\{\abs{a_k}\mid0\le k\le n\}$ \\
$\exists c\in\R,\abs{a_n}=c\abs{a_m}$ \\
Let $R=max\left\{1,\frac{2n}{c}\right\}$ \\
Assume $\abs{z}>R\ge1$ \\
\begin{eqnarray*}
\abs{w} &\le& \sum_{k=0}^{n-1}\frac{\abs{a_k}}{\abs{z}^{n-k}} \\
    &\le& \sum_{k=0}^{n-1}\frac{\abs{a_m}}{\abs{z}} \\
    &\le& \sum_{k=0}^{n-1}\frac{\abs{a_n}}{c\abs{z}} \\
    &<& \sum_{k=0}^{n-1}\frac{\abs{a_n}}{c\frac{2n}{c}} \\
    &<& \sum_{k=0}^{n-1}\frac{\abs{a_n}}{2n} \\
    &=& n\frac{\abs{a_n}}{2n} \\
    &=& \frac{\abs{a_n}}{2} \\
\end{eqnarray*}
$\abs{a_n+w}\ge\abs{\abs{a_n}-\abs{w}}=\abs{\abs{a_n}-\frac{\abs{a_n}}{2}}=
    \abs{\frac{\abs{a_n}}{2}}=\frac{\abs{a_n}}{2}$ \\
$p(z)=a_nz^n+wz^n=(a_n+w)z^n$ \\
$\abs{p(z)}=\abs{(a_n+w)z^n}=\abs{a_n+w}\abs{z^n}\ge
    \frac{\abs{a_n}}{2}\abs{z}^n>\frac{\abs{a_n}R^n}{2}$ \\
$\therefore \abs{\frac{1}{p(z)}}<\frac{2}{\abs{a_n}R^n}$
\end{theproof}
\end{document}
