\documentclass[letterpaper,12pt,fleqn]{article}
\usepackage{matharticle}
\pagestyle{empty}
\newcommand{\vx}{\vec{x}}
\newcommand{\e}{\epsilon}
\newcommand{\norm}[1]{\left\|#1\right\|}
\renewcommand{\mp}{\mathcal{P}}
\newcommand{\mc}{\mathcal{C}}
\begin{document}
\section*{Cauchy Sequences}

\begin{definition}[Cauchy]
  Let $E$ be a normed space and $(\vx_n)$ be a sequence in $E$. To say that
  $(\vx_n)$ is \emph{Cauchy} means:
  \[\forall\,\e>0,\exists\,N>0,m,n>N\implies\norm{\vx_n-\vx_m}<\e\]
  In other words, $\norm{\vx_n-\vx_m}\to0$.
\end{definition}

\begin{theorem}
  Let $E$ be a normed space and let $(\vx_n)$ be a sequence in $E$. TFAE:
  \begin{enumerate}
  \item $(\vx_n)$ is Cauchy sequence.
  \item For every pair of increasing sequences $(p_n)$ and $(q_n)$ in $\N$,
    $\norm{\vx_{p_n}-\vx_{q_n}}\to0$.
  \item For every increasing sequence $(p_n)$ in $\N$,
    $\norm{\vx_{p_{n+1}}-\vx_{p_n}}\to0$.
  \end{enumerate}
\end{theorem}

\begin{theproof}
  \listbreak
  \begin{description}
  \item $1\implies2$: Assume $(\vx_n)$ is Cauchy.

    Assume $\e>0$. \\
    $\exists\,N>0,m,n>N\implies\norm{\vx_n-\vx_m}<\e$

    Assume $(p_n)$ and $(q_n)$ are increasing sequences in $\N$. \\
    Assume $p_n,q_n>N$. \\
    $\norm{\vx_{p_n}-\vx_{q_n}}<\e$

    $\therefore\norm{\vx_{p_n}-\vx_{q_n}}\to0$

  \item $2\implies3$: Assume for every pair of increasing sequences $(p_n)$ and
    $(q_n)$ in $\N$, $\norm{\vx_{p_n}-\vx_{q_n}}\to0$.

    Let $p_n=n+1$ and $q_n=n$.

    $\norm{\vx_{p_n}-\vx_{q_n}}=\norm{\vx_{n+1}-\vx_n}\to0$.

  \item $3\implies1$: Assume $(\vx_n)$ is not Cauchy.

    $\exists\,\e>0,\forall\,N>0,\exists\,n,m>N,\norm{\vx_n-\vx_m}\ge\e$ \\
    Let $\e$ be such an $\e$. \\
    Assume $N>0$. \\
    $\exists\,n>N,\norm{\vx_{n+1}-\vx_n}\ge\e$

    WTS: $\exists\,(p_n),\exists\,\e>0,\forall\,N>0,\exists\,p_n>N,
    \norm{\vx_{p_{n+1}}-\vx_{p_n}}\ge\e$

    Let $p_k=k$.

    $\norm{\vx_{p_{n+1}}-\vx_{p_n}}=\norm{\vx_{n+1}-\vx_n}\ge\e$
  \end{description}
\end{theproof}

\newpage

\begin{examples}
  \listbreak
  \begin{enumerate}
  \item $E=\R$ and $\norm{x}=\abs{x}$

    $(x_n)=\{3, 3.1, 3.14, 3.141, \ldots\}$

    $(x_n)$ is a Cauchy sequence in $\Q$; however, it converges to
    $\pi\notin\Q$.

  \item $E=\mp[0,1]$ and the sup norm.

    $f_n=\sum_{k=1}^n\frac{t^k}{k!}$

    $f_n$ is a Cauchy sequence in $\mp[0,1]$; however, it converges to
    $e^t\notin\mp[0,1]$.
  \end{enumerate}
\end{examples}

\begin{theorem}
  Let $E$ be a normed space and let $(\vx_n)$ be a sequence in $E$:
  \[\vx_n\to\vx\in E\implies(\vx_n)\ \mbox{is Cauchy}\]
\end{theorem}

\begin{theproof}
  Assume $\vx_n\to\vx\in E$. \\
  $\norm{\vx_n-\vx_m}=\norm{(\vx_n-\vx)+(\vx-\vx_m)}\le
  \norm{\vx_n-\vx}+\norm{\vx_m-\vx}\to0+0=0$

  Therefore $(\vx_n)$ is Cauchy.
\end{theproof}

Note that the converse holds in finite-dimensional spaces, but does not always
hold in infinite=dimensional spaces.

\begin{theorem}
  Let $E$ be a normed space and let $(\vx_n)$ be a sequence in $E$:
  \[(\vx_n)\ \mbox{Cauchy}\implies(\norm{\vx_n})\ \mbox{converges}\]
\end{theorem}

\begin{theproof}
  Assume $(\vx_n)$ is Cauchy.

  $\abs{\norm{\vx_n}-\norm{\vx_m}}\le\norm{\vx_n-\vx_m}\to0$

  $\therefore(\norm{\vx_n})$ converges.
\end{theproof}

\begin{corollary}
  Let $E$ be a normed space and let $(\vx_n)$ be a sequence in $E$:
  \[(\vx_n)\ \mbox{Cauchy}\implies(\vx_n)\ \mbox{bounded}\]
\end{corollary}

\newpage

\begin{theproof}
  Assume $(\vx_n)$ is Cauchy.

  Thus $(\norm{\vx_n})$ converges in $\R$, and therefore is bounded.
\end{theproof}

\begin{theorem}
  Let $E$ be a normed space and let $(\vx_n)$ be Cauchy in $E$:

  \qquad $(\vx_n)$ has a convergent subsequence $\implies(\vx_n)$ converges to
  the same limit.
\end{theorem}

\begin{theproof}
  Assume $(\vx_n)$ has a convergent subsequence $(\vx_{n_k})\to\vx\in E$.

  $\norm{\vx_n-\vx}=\norm{(\vx_n-\vx_{n_k})+(\vx_{n_k}-\vx)}\le
  \norm{\vx_n-\vx_{n_k}}+\norm{\vx_{n_k}-\vx}$

  But $(\vx_n)$ is Cauchy and so $\norm{\vx_n-\vx_{n_k}}\to0$. \\
  Furthermore, $\vx_{n_k}\to\vx$ and so $\norm{\vx_{n_k}-\vx}\to0$. \\
  And so $\norm{\vx_n-\vx}\to0$.

  Therefore $(\vx_n)$ converges to the same limit.
\end{theproof}

\end{document}
