\documentclass[letterpaper,12pt,fleqn]{article}
\usepackage{matharticle}
\pagestyle{empty}
\begin{document}
\section*{Natural Numbers}

\begin{definition}
The set of \emph{Natural Numbers}, denoted $\mathbb{N}$, are the whole numbers
starting from 1 and continuing to infinity:
\[\mathbb{N}=\{1, 2, 3, \ldots\}\]
\end{definition}

\begin{notation}{}
$[n]=\{1, 2, 3, \ldots, n\}$
\end{notation}

\theoremstyle{mathitem}
\newtheorem*{peano}{Peano Axioms}
\begin{peano}
\listbreak
\begin{description}
\item{N1: } $1\in\mathbb{N}$.
\item{N2: } $n\in\mathbb{N}\implies(n+1)\in\mathbb{N}$.
\item{N3: } 1 is not the successor of any $n\in\mathbb{N}$.
\item{N4: } $n,m\in\mathbb{N}$ have the same successor $\implies n=m$.
\item{N5: } $S\subseteq\mathbb{N}$ and $1\in S$ and
$(n\in S\implies (n+1)\in S)\implies S=\mathbb{N}$.
\end{description}
\end{peano}

Note that N5 is the basis for mathematical induction.

\newtheorem*{closure}{Closure Property}
\begin{closure}
$\forall n,m\in\mathbb{N}$:
\begin{enumerate}
\item $n+m\in\mathbb{N}$
\item $nm\in\mathbb{N}$
\end{enumerate}
\end{closure}

\begin{theorem}
$\sum_{k=1}^n(2k-1)=n^2$
\end{theorem}

\begin{theproof}
By induction:
\subsubsection*{Base: $n=1$}
\[\sum_{k=1}^n(2k-1)=2(1)-1=2-1=1\]
\[1^2=1\]

\subsubsection*{Inductive Assumption}
Assume $\sum_{k=1}^n(2k-1)=n^2$.
\begin{eqnarray*}
\sum_{k=1}^{n+1}(2k-1) &=& 2(n+1)-1+\sum_{k=1}^n(2k-1) \\
    &=& 2n+2-1+n^2 \\
    &=& n^2+2n+1 \\
    &=& (n+1)^2 \\
\end{eqnarray*}

\end{theproof}

\end{document}
