
\documentclass[letterpaper,12pt,fleqn]{article}
\usepackage{matharticle}
\pagestyle{plain}
\renewcommand{\implies}{\rightarrow}
\begin{document}

\begin{center}
  \large
  Math-42 Sections 01, 02, 05

  \Large
  Homework \#3 Solutions
\end{center}

\subsection*{Problem}

Prove the following logical equivalence using the definition of implication and the rules in Table 6 on page 29 in
the text:
\[(p\implies r)\lor(q\implies r)\equiv(p\land q)\implies r\]

Indicate the name of the rule that you use in each step.  Do NOT skip any steps.  In particular, if you need to
rearrange order or precedence then include commutative or associative steps as necessary.  In order words, each
step must exactly match a rule from Table 6.

\begin{tabular}{ll}
  \((p\implies r)\lor(q\implies r)\) & \\
  \((\bar{p}\lor r)\lor(\bar{q}\lor r)\) & Equivalence of implication \\
  \(\bar{p}\lor(r\lor(\bar{q}\lor r))\) & Associativity \\
  \(\bar{p}\lor(r\lor(r\lor\bar{q}))\) & Commutativity \\
  \(\bar{p}\lor((r\lor r)\lor\bar{q})\) & Associativity \\
  \(\bar{p}\lor(r\lor\bar{q})\) & Idempotence \\
  \(\bar{p}\lor(\bar{q}\lor r)\) & Commutativity \\
  \((\bar{p}\lor\bar{q})\lor r\) & Associativity \\
  \(\overline{p\land q}\lor r\) & DeMorgan \\
  \((p\land q)\implies r\) & Equivalence of implication
\end{tabular}

\end{document}
