\documentclass[letterpaper,12pt,fleqn]{article}
\usepackage{matharticle}
\pagestyle{plain}
\newcommand{\son}{\sum_{k=1}^n}
\begin{document}

\begin{center}
  \large
  Math-42 Sections 01, 02, 05

  \Large
  Homework \#9 Solutions
\end{center}

\subsection*{Problems}

Prove the following using the telescoping sum method discussed in class:
\[\sum_{k=1}^nk^2=\frac{n(n+1)(2n+1)}{6}\]

\bigskip

First, start with a telescoping sum:
\begin{align*}
  \son [(k+1)^3-k^3] &= (n+1)^3-1^3 \\
  &= n^3+3n^2+3n+1-1 \\
  &= n^3+3n^2+3n
\end{align*}
Next, evaluate the sum directly:
\begin{align*}
  \son [(k+1)^3-k^3] &= \son(k^3+3k^2+3k+1-k^3) \\
  &= \son(3k^2+3k+1) \\
  &= 3\son k^2+3\son k+\son 1 \\
  &= 3\son k^2+3\left[\frac{n(n+1)}{2}\right]+n
\end{align*}
Finally, equate the two and do some algebra:
\begin{gather*}
  3\son k^2+3\left[\frac{n(n+1)}{2}\right]+n=n^3+3n^2+3n \\
  3\son k^2=n^3+3n^2+3n-3\left[\frac{n(n+1)}{2}\right]-n \\
  3\son k^2=n^3+3n^2+2n-\frac{3}{2}n^2-\frac{3}{2}n \\
  3\son k^2=n^3+\frac{3}{2}n^2+\frac{1}{2}n \\
  3\son k^2=\frac{1}{2}n(2n^2+3n+1) \\
  3\son k^2=\frac{n(n+1)(2n+1)}{2} \\
  \son k^2=\frac{n(n+1)(2n+1)}{6}
\end{gather*}

\end{document}
