\documentclass[letterpaper,12pt,fleqn]{article}
\usepackage{matharticle}
\pagestyle{empty}
\renewcommand{\o}{\theta}
\begin{document}
\section*{DeMoivre's Formula}
\begin{theorem}
Let $n\in\Z$:
\[(\cos\o+i\sin\o)^n=\cos(n\o)+i\sin(n\o)\]
\end{theorem}

\begin{theproof}
\[(\cos\o+i\sin\o)^n=\left(e^{i\o}\right)^n=e^{i(n\o)}=\cos(n\o)+i\sin(n\o)\]
\end{theproof}

\begin{theorem}
Let $n\in\N$ and:
\[m=\begin{cases}
    \frac{n-1}{2}, & n\ \mbox{odd} \\
    \frac{n}{2}, & n\ \mbox{even} \\
\end{cases}\]
\[\cos(n\o)=\sum_{k=0}^m\binom{n}{2k}(-1)^k\cos^{n-2k}\o\sin^{2k}\o\]
\[\sin(n\o)=\sum_{k=0}^m\binom{n}{2k+1}(-1)^k\cos^{n-(2k+1)}\o\sin^{2k+1}\o\]
\end{theorem}

\begin{theproof}
\listbreak
\begin{eqnarray*}
\cos(n\o)+i\sin(n\o) &=& (\cos\o+i\sin\o)^n \\
    &=& \sum_{k=0}^n\binom{n}{k}\cos^{n-k}\o(i\sin\o)^k \\
    &=& \sum_{k=0}^n\binom{n}{k}i^k\cos^{n-k}\o\sin^k\o \\
\end{eqnarray*}

Note that $\cos(n\o)$ is the real terms, occurring at even $k$:

\[\cos(n\o)=\sum_{k=0}^m\binom{n}{2k}(-1)^k\cos^{n-2k}\o\sin^{2k}\o\]

Similarly, $\sin(n\o)$ is the imaginary terms, occurring at odd $k$:

\[\sin(n\o)=\sum_{k=0}^m\binom{n}{2k+1}(-1)^k\cos^{n-(2k+1)}\o\sin^{2k+1}\o\]
\end{theproof}

\begin{example}
\begin{eqnarray*}
\cos(2\o) &=& \sum_{k=0}^1\binom{2}{2k}(-1)^k\cos^{2-2k}\o\sin^{2k}\o \\
    &=& \binom{2}{0}\cos^2\o-\binom{2}{1}\sin^2\o \\
    &=& \cos^2\o-\sin^2\o
\end{eqnarray*}

\begin{eqnarray*}
\sin(2\o) &=& \sum_{k=0}^1\binom{2}{2k+1}(-1)^k\cos^{2-(2k+1)}\o\sin^{2k+1}\o \\
    &=& \binom{2}{1}\cos\o\sin\o-0 \\
    &=& 2\sin\o\cos\o \\
\end{eqnarray*}

\begin{eqnarray*}
\cos(3\o) &=& \sum_{k=0}^1\binom{3}{2k}(-1)^k\cos^{3-2k}\o\sin^{2k}\o \\
    &=& \binom{3}{0}\cos^3\o-\binom{3}{2}\cos\o\sin^2\o \\
    &=& \cos^3\o-3\cos\o\sin^2\o \\
\end{eqnarray*}

\begin{eqnarray*}
\sin(3\o) &=& \sum_{k=0}^1\binom{3}{2k+1}(-1)^k\cos^{3-(2k+1)}\o\sin^{2k+1}\o \\
    &=& \binom{3}{1}\cos^2\o\sin\o-\binom{3}{3}\sin^3\o \\
    &=& 3\cos^2\o\sin\o-\sin^3\o \\
\end{eqnarray*}
\end{example}
\end{document}
