\documentclass[letterpaper,12pt,fleqn]{article}
\usepackage{matharticle}
\pagestyle{empty}
\renewcommand{\c}[1]{\overline{#1}}
\begin{document}
\section*{Cauchy-Schwarz Inequality}

\begin{theorem}
  $\forall\,a,b\in\C$:
  \[\abs{\sum{a_kb_k}}^2\le
  \left(\sum{\abs{a_k}^2}\right)\left(\sum{\abs{b_k}^2}\right)\]
\end{theorem}

\begin{theproof}
  If $\forall\,a_k=0$ or $\forall\,b_k=0$ then trivial, so \\
  AWLOG: $\exists\,a_k\ne0$ and $\exists\,b_k\ne0$ \\
  Assume $c\in\C$
  \begin{eqnarray*}
    \sum{\abs{a_k-c\c{b_k}}^2} &=& \sum{(a_k-c\c{b_k})(\c{a_k-c\c{b_k}})} \\
    &=& \sum{(a_k-c\c{b_k})(\c{a_k}-\c{c}b_k)} \\
    &=& \sum{\left(a_k\c{a_k}+c\c{b_k}\c{c}b_k-a_k\c{c}b_k-c\c{b_k}\c{a_k}
      \right)} \\
    &=& \sum{\left[\abs{a_k}^2+\abs{c}^2\abs{b_k}^2-
        (a_kb_k\c{c}+\c{a_kb_c\c{c}})\right]} \\
    &=& \sum{\left[\abs{a_k}^2+\abs{c}^2\abs{b_k}^2-2Re(a_kb_k\c{c})\right]} \\
    &=& \sum{\abs{a_k}^2}+\abs{c}^2\sum{\abs{b_k}^2}-
    2Re\left(\c{c}\sum{a_kb_k}\right) \\
    &\ge& 0 \\
  \end{eqnarray*}
  Let $c=\frac{\sum{a_kb_k}}{\sum{\abs{b_k}^2}}$
  \[\sum{\abs{a_k}^2}+\abs{c}^2\sum{\abs{b_k}^2}-    
  2Re\left(\c{c}\sum{a_kb_k}\right)\ge0\]
  \[\sum{\abs{a_k}^2}+
  \abs{\frac{\sum{a_kb_k}}{\sum{\abs{b_k}^2}}}^2\sum{\abs{b_k}^2}-    
  2Re\left(\c{\frac{\sum{a_kb_k}}{\sum{\abs{b_k}^2}}}\sum{a_kb_k}\right)\ge0\]
  \[\sum{\abs{a_k}^2}+\frac{\abs{\sum{a_kb_k}}^2}{\sum{\abs{b_k}^2}}-
  2Re\left(\frac{\abs{\sum{a_kb_k}}^2}{\sum{\abs{b_k}^2}}\right)\ge0\]
  \[\sum{\abs{a_k}^2}+\frac{\abs{\sum{a_kb_k}}^2}{\sum{\abs{b_k}^2}}-
  2\frac{\abs{\sum{a_kb_k}}^2}{\sum{\abs{b_k}^2}}\ge0\]
  \[\sum{\abs{a_k}^2}-\frac{\abs{\sum{a_kb_k}}^2}{\sum{\abs{b_k}^2}}\ge0\]
  \[\left(\sum{\abs{a_k}^2}\right)\left(\sum{\abs{b_k}^2}\right)-
  \abs{\sum{a_kb_k}}^2\ge0\]
  \[\abs{\sum{a_kb_k}}^2\le
  \left(\sum{\abs{a_k}^2}\right)\left(\sum{\abs{b_k}^2}\right)\]
\end{theproof}

\end{document}
