\documentclass[letterpaper,12pt,fleqn]{article}
\usepackage{matharticle}
\usepackage{cancel}
\pagestyle{plain}
\begin{document}

\begin{center}
  \large
  Math-71 Sections 02, 03, 60

  \Large
  Homework \#3 Solutions
\end{center}

\subsection*{Problem}

Consider the function: \(f(x)=\sqrt{x}\).
\begin{enumerate}
\item Calculate \(f'(x)\) using the definition of the derivative.
  \begin{align*}
    f'(t) &= \lim_{h\to0}\frac{f(x+h)-f(x)}{h} \\
    &= \lim_{h\to0}\frac{\sqrt{x+h}-\sqrt{x}}{h} \\
    &= \lim_{h\to0}\left(\frac{\sqrt{x+h}-\sqrt{x}}{h}\right)
    \left(\frac{\sqrt{x+h}+\sqrt{x}}{\sqrt{x+h}+\sqrt{x}}\right) \\
    &= \lim_{h\to0}\frac{(\cancel{x}+h)-(\cancel{x})}{h(\sqrt{x+h}+\sqrt{x})} \\
    &= \lim_{h\to0}\frac{\cancel{h}}{\cancel{h}(\sqrt{x+h}+\sqrt{x})} \\
    &= \lim_{h\to0}\frac{1}{\sqrt{x+h}+\sqrt{x}} \\
    &= \frac{1}{\sqrt{x+0}+\sqrt{x}} \\
    &= \frac{1}{\sqrt{x}+\sqrt{x}} \\
    &= \frac{1}{2\sqrt{x}}
  \end{align*}
  
\item Calculate \(f'(x)\) using some other method.

  Make sure that your two final answers match exactly.
  \begin{gather*}
    f(x)=\sqrt{x}=x^{\frac{1}{2}} \\
    \\
    f'(x)=\frac{1}{2}x^{-\frac{1}{2}}=\frac{1}{2x^{\frac{1}{2}}}=\frac{1}{2\sqrt{x}}
  \end{gather*}
\end{enumerate}

\end{document}
