\documentclass[letterpaper,12pt,fleqn]{article}
\usepackage{matharticle}
\pagestyle{empty}
\begin{document}
\section*{Center}

\begin{definition}
  Let $G$ be a group:
  \begin{enumerate}
  \item Let $a\in G$. $G_a$ is the subset of $G$ consisting of all elements in
    $G$ that commute with $a$:
    \[G_a=\{g\in G\mid ga=ag\}\]

  \item Let $S\subseteq G,S\ne\emptyset$. $G_S$ is the subset of $G$ consisting
    of all elements in $G$ that commute with all elements in $S$:
    \[G_S=\{g\in G\mid\forall\,s\in S,gs=sg\}\]
  \end{enumerate}
\end{definition}

\begin{theorem}
  Let $G$ be a group and $a\in G$:
  \[G_a\le G\]
\end{theorem}

\begin{theproof}
  Assume $x,y\in G_a$ \\
  $G_a\subseteq G$, so $x,y\in G$ \\
  $G$ is a group, so $y^{-1}\in G$ \\
  Assume $g\in G$ \\
  $xgy=gxy=gyx=ygx$ \\
  $y^{-1}xgy=y^{-1}ygx$ \\
  $xy^{-1}gy=gx$ \\
  $xy^{-1}gyy^{-1}=gxy^{-1}$ \\
  $xy^{-1}g=gxy^{-1}$ \\
  $xy^{-1}\in G_a$ \\
  $\therefore$ by the subgroup test, $G_a\le G$.
\end{theproof}

\begin{theorem}
  Let $G$ be a group and $S\subseteq G,S\ne\emptyset$:
  \[G_S\le G\]
\end{theorem}

\begin{theproof}
  Assume $x,y\in G_S$ \\
  $G_S\subseteq G$, so $x,y\in G$ \\
  $G$ is a group, so $y^{-1}\in G$ \\
  Assume $s\in S$ \\
  $xsy=sxy=syx=ysx$ \\
  $y^{-1}xsy=y^{-1}ysx$ \\
  $xy^{-1}sy=sx$ \\
  $xy^{-1}syy^{-1}=sxy^{-1}$ \\
  $xy^{-1}s=sxy^{-1}$ \\
  $xy^{-1}\in G_S$ \\
  $\therefore$ by the subgroup test, $G_S\le G$.
\end{theproof}

\begin{definition}
  The \emph{center} of a group $G$, denoted $Z(G)$, is the subgroup of G
  whose elements commute with all elements in $G$:
  \[Z(G)=G_G\]
\end{definition}

\begin{theorem}
  Let $G$ be a group. $Z(G)$ is abelian.
\end{theorem}

\begin{theproof}
  Assume $a,b\in Z(G)$ \\
  $Z(G)\subseteq G$, so $a,b\in G$ \\
  $ab=ba$ \\
  $\therefore Z(G)$ is abelian.
\end{theproof}

\end{document}
