\documentclass[letterpaper,12pt,fleqn]{article}
\usepackage{matharticle}
\pagestyle{empty}
\newcommand{\p}{\varphi}
\newcommand{\s}{\psi}
\renewcommand{\a}{\alpha}
\renewcommand{\b}{\beta}
\newcommand{\n}{\trianglelefteq}
\newcommand{\rest}[2]{\left.#1\right|_{#2}}
\DeclareMathOperator{\Aut}{Aut}
\begin{document}
\section*{Stable}

\begin{definition}[Stable]
  Let $F\subseteq L\subseteq K$ be an inclusion of fields. To say that $L$ is
  \emph{stable} with respect to $K/F$ means:
  \[\forall\p\in\Aut(K/F),\p[L]\subseteq L\]
\end{definition}

\begin{theorem}
  Let $F\subseteq L\subseteq K$ be an inclusion of fields such that $L$ is stable with
  respect to $K/F$:
  \[\forall\p\in\Aut(K/F),\p[L]=L\]
  Thus $\rest{\p}{L}\in\Aut(L/F)$.
\end{theorem}

\begin{theproof}
  Assume $\p\in G$ \\
  Since $L$ is stable, $\p[L]\subseteq L$ \\
  But $\p$ is bijective, so $\rest{\p}{L}$ is surjective

  $\therefore\p[L]=L$
\end{theproof}

\begin{theorem}
  Let $F\subseteq L\subseteq K$ be an inclusion of fields such that $K/F$ is Galois and
  $L$ is stable with respect to $K/F$:
  \[L/F\ \mbox{is Galois}\]
\end{theorem}

\begin{theorem}
  Assume $\a\in L\setminus F$ \\
  $\exists\p\in\Aut(K/F),\p(\a)\ne\a$ \\
  But $L$ is stable, so $\rest{\p}{L}\in\Aut(L/F)$ and $\rest{\p}{L}(\a)\ne\a$

  Therefore $L/F$ is Galois.
\end{theorem}

\begin{theorem}
  Let $F\subseteq L\subseteq K$ be an inclusion of fields:
  \begin{enumerate}
  \item $L$ stable $\implies G(L)\n G$
  \item $H\n G \implies F(H)$ stable.
  \end{enumerate}
\end{theorem}

\newpage

\begin{theproof}
  \listbreak
  \begin{enumerate}
  \item Assume $L$ is stable

    Assume $\p\in G(L)$ \\
    Assume $\a\in L$ \\
    $\p(\a)=\a$

    Assume $\s\in G$ \\
    Since $\s$ is bijective and $L$ is stable, $\exists\,\b\in L,\s(b)=\a$ and
    $\s^{-1}(\a)=\b$ \\
    Also, since $\b\in L$, $\p(\b)=\b$

    $(\s\p\s^{-1})(\a)=\s(\p(\s^{-1}(\a)))=\s(\p(\b))=\s(\b)=\a$ \\
    Thus, $\s\p\s^{-1}\in G(L)$

    $\therefore G(L)\n G$.

  \item Assume $H\n G$

    Assume $\p\in H$ \\
    Assume $\s\in G$ \\
    Since $H\n G$, $\s^{-1}\p\s\in H$

    Assume $\a\in F(H)$ \\
    $(\s^{-1}\p\s)(\a)=\a$ \\
    $(\p\s)(\a)=\s(\a)$ \\
    $\p(\s(\a))=\s(\a)$ \\
    Thus, $\s(\a)\in F(H)$

    Therefore, $F(H)$ is stable.
  \end{enumerate}
\end{theproof}

\end{document}
