\documentclass[letterpaper,12pt,fleqn]{article}
\usepackage{matharticle}
\pagestyle{empty}
\newcommand{\vx}{\vec{x}}
\newcommand{\vy}{\vec{y}}
\newcommand{\vz}{\vec{0}}
\newcommand{\norm}[1]{\|#1\|}
\begin{document}
\section*{Vector Norm}

\begin{definition}[Vector Norm]
  Let $V$ be a vector space over a field $F$. To say that a function
  $\norm{\cdot}:V\to\R$ is a \emph{vector norm} means that it satifies the
  following four properties $\forall\,\vx,\vy\in V$ and $\forall\,c\in F$:
  \begin{enumerate}
  \item Nonnegativity: $\norm{\vx}\ge0$
  \item Positivity: $\norm{\vx}=0\iff\vx=0$
  \item Homogeneity: $\norm{c\vx}=\abs{c}\norm{\vx}$
  \item Subadditivity: $\norm{\vx+\vy}\le\norm{\vx}+\norm{\vy}$
    (triangle inequality)
  \end{enumerate}
\end{definition}

\begin{theorem}
  Let $V$ be a vector space and let $\vx\in V$:
  \[\norm{-\vx}=\norm{\vx}\]
\end{theorem}

\begin{theproof}
  $\norm{-\vx}=\norm{(-1)\vx}=\abs{-1}\norm{\vx}=1\cdot\norm{\vx}=\norm{\vx}$
\end{theproof}

\begin{theorem}
  The nonnegativity property of the norm can be derived from the other three
  properties.
\end{theorem}

\begin{theproof}
  Assume $V$ be a vector space over a field $F$ \\
  Assume $\vx\in V$
  \begin{eqnarray*}
    \norm{\vx-\vx} &\le& \norm{\vx}+\norm{-\vx} \\
    \norm{\vz} &\le& \norm{\vx}+\norm{\vx} \\
    0 &\le& 2\norm{\vx} \\
    \therefore\norm{\vx} &\ge& 0
  \end{eqnarray*}
\end{theproof}

\begin{theorem}
  Let $V$ be a vector space over a field $F$. $\forall\,\vx,\vy\in V$:
  \[\abs{\norm{x}-\norm{y}}\le\norm{\vx-\vy}\le\norm{\vx}+\norm{\vy}\]
\end{theorem}

\begin{theproof}
  $\norm{\vy}=\norm{\vx+(\vy-\vx)}\le\norm{\vx}+\norm{\vy-\vx}=
  \norm{\vx}+\norm{\vx-\vy}$ \\
  $\norm{\vy}-\norm{\vx}\le\norm{\vx-\vy}$ \\
  $-(\norm{\vx}-\norm{\vy})\le\norm{\vx-\vy}$

  $\norm{\vx}=\norm{\vy+(\vx-\vy)}\le\norm{\vy}+\norm{\vx-\vy}$ \\
  $\norm{\vx}-\norm{\vy}\le\norm{\vx-\vy}$

  $\pm(\norm{\vx}-\norm{\vy})\le\norm{\vx-\vy}$ \\
  $\abs{\norm{\vx}-\norm{\vy}}\le\norm{\vx-\vy}$

  $\norm{\vx-\vy}\le\norm{\vx}+\norm{-\vy}=\norm{\vx}+\norm{\vy}$

  $\therefore\abs{\norm{x}-\norm{y}}\le\norm{\vx-\vy}\le\norm{\vx}+\norm{\vy}$
\end{theproof}

\begin{example}
  Let $V=\C^n$:
  \begin{enumerate}
  \item $\ell_2$ (Euclidean) Norm

    $\norm{\vx}_2=\left(\sum_{k=1}^n\abs{x_k}^2\right)^{\frac{1}{2}}=
    \vx^{\,*}\vx$\hspace{2ex}(standard norm)

  \item $\ell_1$ Norm

    $\norm{\vx}_1=\sum_{k=1}^n\abs{x_k}$

  \item $\ell_{\infty}$ Norm
    
    $\norm{\vx}_1=\max\{\abs{x_k}\mid 1\le k\le n\}$

  \item $\ell_p$ Norm ($1\le p\le \infty$)

    $\norm{\vx}_p=\left(\sum_{k=1}^n\abs{x_k}^p\right)^{\frac{1}{p}}$

  \item $k$-norm ($k\in\Z^+$

    $\norm{\vx}_{[k]}=\sum_{i=1}^k\abs{x_{j_i}}$ where the components have been
    permuted such that $\abs{x_{j_i}}\ge\abs{x_{j_{i+1}}}$
  \end{enumerate}
\end{example}

\end{document}
