\documentclass[letterpaper,12pt,fleqn]{article}
\usepackage{matharticle}
\pagestyle{empty}
\renewcommand{\a}{\alpha}
\newcommand{\vp}{\varphi}
\DeclareMathOperator{\id}{id}
\DeclareMathOperator{\Aut}{Aut}
\begin{document}
\section*{Closure}

\begin{definition}[Closure]
  Let $F\subseteq L\subseteq K$ be an inclusion of fields and let $H\le G(L)$:
  \begin{itemize}
  \item The \emph{closure} of $L$ is $F(G(L))$.
  \item The \emph{closure} of $H$ is $G(F(H))$.
  \end{itemize}

  To say that $L$ and $G$ are called $\emph{closed}$ means:
  \begin{itemize}
  \item $F(G(L))=L$
  \item $G(F(H))=H$
  \end{itemize}

  Thus, $K/F$ is closed iff $K/F$ is Galois.
\end{definition}

\begin{theorem}
  Let $F\subseteq E\subseteq L\subseteq K$ be an inclusion of fields and
  subgroups $\{\id\}=I\le J\le H\le G=\Aut(K/F)$:
  \begin{enumerate}
  \item $G(L)\le G(E)$
  \item $F(H)\subseteq F(J)$
  \item $H\le G(F(H))$
  \item $L\subseteq F(G(L))$
  \item $G(L)$ is closed
  \item $F(H)$ is closed
  \end{enumerate}
\end{theorem}

\begin{theproof}
  \listbreak
  \begin{enumerate}
  \item Assume $\vp\in G(L)$

    Since it has already been proven that $G(L),G(E)\le G$, it suffices to show inclusion:

    $\forall\,\a\in L,\vp(\a)=\a$ \\
    Since $E\subseteq L$, $\forall\,\a\in E,\vp(\a)=\a$ \\
    $\vp\in G(E)$
    
    $\therefore G(L)\le G(E)$

  \item Assume $\a\in F(H)$

    $\forall\,\vp\in H,\vp(\a)=\a$ \\
    Since $J\subseteq H$, $\forall\,\vp\in J,\vp(\a)=\a$ \\
    So $\a\in F(J)$

    $\therefore F(H)\subseteq F(J)$

  \item Assume $\vp\in H$

    Since it has already been proven that $H,G(F(H))\le G$, it suffices to show inclusion.
    
    By definition, $\vp$ fixes everything in $F(H)$ \\
    So, by definition, $\vp\in G(F(H))$.

    $\therefore H\le G(F(H))$

  \item Assume $\a\in L$

    By definition, $\a$ is fixed by everything in $G(L)$ \\
    So, by definition, $\a\in F(G(L))$.

    $\therefore L\subseteq F(G(L))$

  \item It has already been proven that $G(L)\subseteq G(F(G(L)))$

    Assume $\vp\in G(F(G(L)))$ \\
    $\vp$ fixes everything in $F(G(L))$ \\
    $L\subseteq F(G(L))$ \\
    So $\vp$ fixes everything in $L$ \\
    Thus, $\vp\in G(L)$
    
    $\therefore G(L)=G(F(G(L)))$ and so $G(L)$ is closed.

  \item It has already been proven that $F(H)\subseteq F(G(F(H)))$

    Assume $\a\in F(G(F(H)))$ \\
    $\a$ is fixed by everything in $G(F(H))$ \\
    $H\subseteq G(F(H))$ \\
    So $\a$ is fixed by everything in $H$ \\
    Thus, $\a\in F(H)$

    $\therefore F(H)=F(G(F(H)))$.
  \end{enumerate}
\end{theproof}

\end{document}
