\documentclass[letterpaper,12pt,fleqn]{article}
\usepackage{matharticle}
\pagestyle{empty}
\renewcommand{\o}{\theta}
\allowdisplaybreaks
\begin{document}
\section*{Lagrange's Identity}
\begin{theorem}
\[\sum_{k=0}^n\cos k\o=
    \frac{1}{2}+
        \frac{\sin\left[(2n+1)\frac{\o}{2}\right]}
        {2\sin\left(\frac{\o}{2}\right)}=
    \frac{\sin\left[(n+1)\frac{\o}{2}\right]\cos\left(n\frac{\o}{2}\right)}
        {\sin\left(\frac{\o}{2}\right)}\]
\[\sum_{k=0}^n\sin k\o=
    \frac{\cot\left(\frac{\o}{2}\right)}{2}-
        \frac{\cos\left[(2n+1)\frac{\o}{2}\right]}
        {2\sin\left(\frac{\o}{2}\right)}=
    \frac{\sin\left[(n+1)\frac{\o}{2}\right]\sin\left(n\frac{\o}{2}\right)}
        {\sin\left(\frac{\o}{2}\right)}\]
\end{theorem}

\begin{theproof}
Let $R=\sum_{k=0}^n\cos k\o$ \\
Let $I=\sum_{k=0}^n\sin k\o$ \\
\begin{eqnarray*}
R+iI &=& \sum_{k=0}^n\cos k\o+i\sum_{k=0}^n\sin k\o \\
    &=& \sum_{k=0}^n(\cos k\o+i\sin k\o) \\
    &=& \sum_{k=0}^n\left(e^{i\o}\right)^k \\
    &=& \frac{e^{i(n+1)\o}-1}{e^{i\o}-1} \\
    &=& \frac{e^{-i\frac{\o}{2}}\left[e^{i(n+1)\o}-1\right]}
        {e^{-i\frac{\o}{2}}\left(e^{i\o}-1\right)} \\
    &=& \frac{\left[e^{i(n\o+\o-\frac{\o}{2})}-e^{-i\frac{\o}{2}}\right]}
        {e^{i\frac{\o}{2}}-e^{-i\frac{\o}{2}}} \\
    &=& \frac{\left[e^{i(n\o+\frac{\o}{2})}-e^{-i\frac{\o}{2}}\right]}
        {2i\sin\left(\frac{\o}{2}\right)} \\
    &=& \frac{\left[\cos\left(n\o+\frac{\o}{2}\right)+
            i\sin\left(n\o+\frac{\o}{2}\right)\right]-
            \left(\cos\frac{\o}{2}-i\sin\frac{\o}{2}\right)}
            {2i\sin\left(\frac{\o}{2}\right)} \\
    &=& \frac{\left[\cos\left(n\o+\frac{\o}{2}\right)-\cos\frac{\o}{2}\right]+
            i\left[\sin\left(n\o+\frac{\o}{2}\right)+\sin\frac{\o}{2}\right]}
            {2i\sin\left(\frac{\o}{2}\right)} \\
    &=& \frac{\left[\sin\left(n\o+\frac{\o}{2}\right)+\sin\frac{\o}{2}\right]-
            i\left[\cos\left(n\o+\frac{\o}{2}\right)-\cos\frac{\o}{2}\right]}
            {2\sin\left(\frac{\o}{2}\right)} \\
\end{eqnarray*}

\[\sum_{k=0}^n\cos(k\o)=Re(R+iI)=
    \frac{\sin\frac{\o}{2}+\sin\left(n\o+\frac{\o}{2}\right)}
    {2\sin\left(\frac{\o}{2}\right)}=
    \frac{1}{2}+\frac{\sin\left[(2n+1)\frac{\o}{2}\right]}
    {2\sin\left(\frac{\o}{2}\right)}\]

\[\sum_{k=0}^n\sin(k\o)=Im(R+iI)=
    \frac{\cos\frac{\o}{2}-\cos\left(n\o+\frac{\o}{2}\right)}
    {2\sin\left(\frac{\o}{2}\right)}=
    \frac{\cot\left(\frac{\o}{2}\right)}{2}-
    \frac{\cos\left[(2n+1)\frac{\o}{2}\right]}
    {2\sin\left(\frac{\o}{2}\right)}\]

Continuing:

\begin{eqnarray*}
R+iI &=& \frac{\left[\sin\left(n\o+\frac{\o}{2}\right)+\sin\frac{\o}{2}\right]-
            i\left[\cos\left(n\o+\frac{\o}{2}\right)-\cos\frac{\o}{2}\right]}
            {2\sin\left(\frac{\o}{2}\right)} \\
     &=& \frac{2\sin\left(\frac{n\o+\frac{\o}{2}+\frac{\o}{2}}{2}\right)
            \cos\left(\frac{n\o+\frac{\o}{2}-\frac{\o}{2}}{2}\right)+
            i2\sin\left(\frac{n\o+\frac{\o}{2}+\frac{\o}{2}}{2}\right)
            \sin\left(\frac{n\o+\frac{\o}{2}-\frac{\o}{2}}{2}\right)}
            {2\sin\left(\frac{\o}{2}\right)} \\
     &=& \frac{\sin\left(\frac{n\o+\frac{\o}{2}+\frac{\o}{2}}{2}\right)
            \cos\left(\frac{n\o+\frac{\o}{2}-\frac{\o}{2}}{2}\right)+
            i\sin\left(\frac{n\o+\frac{\o}{2}+\frac{\o}{2}}{2}\right)
            \sin\left(\frac{n\o+\frac{\o}{2}-\frac{\o}{2}}{2}\right)}
            {\sin\left(\frac{\o}{2}\right)} \\
     &=& \frac{\sin\left(\frac{n\o+\o}{2}\right)
            \cos\left(\frac{n\o}{2}\right)+
            i\sin\left(\frac{n\o+\o}{2}\right)
            \sin\left(\frac{n\o}{2}\right)}
            {\sin\left(\frac{\o}{2}\right)} \\
\end{eqnarray*}

\[\sum_{k=0}^n\cos k\o=Re(R+iI)=
    \frac{\sin\left(\frac{n\o+\o}{2}\right)\cos\left(\frac{n\o}{2}\right)}
    {\sin\left(\frac{\o}{2}\right)}=
    \frac{\sin\left[(n+1)\frac{\o}{2}\right]\cos\left(n\frac{\o}{2}\right)}
    {\sin\left(\frac{\o}{2}\right)}\]

\[\sum_{k=0}^n\sin k\o=Im(R+iI)=
    \frac{\sin\left(\frac{n\o+\o}{2}\right)\sin\left(\frac{n\o}{2}\right)}
    {\sin\left(\frac{\o}{2}\right)}=
    \frac{\sin\left[(n+1)\frac{\o}{2}\right]\sin\left(n\frac{\o}{2}\right)}
    {\sin\left(\frac{\o}{2}\right)}\]
\end{theproof}
\end{document}
