\documentclass[letterpaper,12pt,fleqn]{article}
\usepackage{matharticle}
\pagestyle{empty}
\newcommand{\vx}{\vec{x}}
\newcommand{\mb}{\mathcal{B}}
\newcommand{\norm}[1]{\left\|#1\right\|}
\newcommand{\inner}[1]{\left<#1\right>}
\begin{document}
\section*{Normal Operators}

\begin{definition}[Normal]
  Let $E$ be a vector space and let $T$ be a bounded operator on $E$. To say
  that $T$ is a \emph{normal} operator means:
  \[T^*T=TT^*\]
  In other words, $T$ and its adjoint commute.
\end{definition}

Note that if $T$ is self-adjoint then it is clearly normal; however, the
converse is not necessarily true.

\begin{example}
  Let $T\vx=i\vx$. \\
  $T=iI$ \\
  $T^*=(iI)^*=-iI^*=-iI$

  $\therefore T\ne T^*$

  $TT^*=(iI)(-iI)=(-iI)(iI)=T^*T$

  Therefore $T$ and $T^*$ commute.
\end{example}

\begin{theorem}
  Let $H$ be a Hilbert space and let $T\in\mb(H)$:

  \qquad$T$ is normal $\iff\forall\,\vx\in H,\norm{T\vx}=\norm{T^*\vx}$
\end{theorem}

\begin{theproof}
  Assume $\vx\in H$.
  \begin{description}
  \item $\implies$ Assume $T$ is normal.

    $\norm{T\vx}^2=\inner{T\vx,T\vx}={T^*T\vx,\vx}={TT^*\vx,\vx}=
    {T^*\vx,T^*\vx}=\norm{T^*\vx}^2$

    $\therefore\norm{T\vx}=\norm{T^*\vx}$

  \item $\impliedby$ Assume $\norm{T\vx}=\norm{T^*\vx}$.

    $\inner{T\vx,T\vx}=\inner{T^*\vx,T^*\vx}$

    $\inner{T^*T\vx,\vx}=\inner{TT^*\vx,\vx}$

    Therefore $T^*T=TT^*$ and thus $T$ is normal.
  \end{description}
\end{theproof}

\newpage

\begin{theorem}
  Let $H$ be a Hilbert space and let $T,A,B\in\mb(H)$ such that $T=A+iB$:

  \qquad$T$ is normal $\iff AB=BA$.
\end{theorem}

\begin{theproof}
  By previous theorem, $A$ and $B$ are unique and self-adjoint.

  $T^*=(A+iB)^*=A^*+(iB)^*=A^*-iB^*=A-iB$

  $TT^*=(A+iB)(A-iB)=A^2-iAB+iBA=B^2=A^2+B^2+i(BA-AB)$

  $T^*T=(A-iB)(A+iB)=A^2-iBA+iAB=B^2=A^2+B^2-i(BA-AB)$

  \begin{tabular}{lcl}
    $T$ is normal & $\iff$ & $TT^*=T^*T$ \\
    & $\iff$ & $A^2+B^2+i(BA-AB)=A^2+B^2-i(BA-AB)$ \\
    & $\iff$ & $2i(BA-AB)=0$ \\
    & $\iff$ & $BA-BA=0$ \\
    & $\iff$ & $AB=BA$
  \end{tabular}
\end{theproof}

\begin{theorem}
  Let $H$ be a Hilbert space and $T\in\mb(H)$:

  \qquad$T$ is normal $\implies\norm{T^n}=\norm{T}^n$
\end{theorem}

\begin{theproof}
  It is already known that $\norm{T^n}\le\norm{T}^n$.

  For $\norm{T^n}\ge\norm{T}^n$, proof by induction on $n$:
  \begin{description}
  \item Base case: $n=1$: Trivial.

  \item Assume $\norm{T^n}\le\norm{T}^n$

  \item Consider $n+1$.

    Assume $\vx\in H$ such that $\norm{\vx}=1$.
    
    First, note:
    \[\norm{T^2\vx}^2=\inner{T^2\vx,T^2\vx}=\inner{T^*T\vx,T^*T\vx}=
    \norm{T^*T\vx}^4\]
    But, since $\norm{T^*T}=sup_{\norm{\vx}=1}\abs{\inner{T^*T\vx,\vx}}$:
    \[\norm{T^2\vx}=\norm{T^*T\vx}^2\ge\inner{T^*T\vx,\vx}=
    \inner{T\vx,T\vx}=\norm{T\vx}^2\]
    Now:
    \begin{eqnarray*}
      \norm{T^{n+1}\vx} &=& \norm{T^nT\vx} \\
      &=& \norm{T\vx}\norm{\frac{1}{\norm{T\vx}}T^nT\vx} \\
      &=& \norm{T\vx}\norm{T^n\frac{T\vx}{\norm{T\vx}}} \\
      &\ge& \norm{T\vx}\norm{T\frac{T\vx}{\norm{T\vx}}}^n \\
      &=& \norm{T\vx}^{1-n}\norm{T^2\vx}^n \\
      &\ge& \norm{T\vx}^{1-n}\norm{T\vx}^{2n} \\
      &=& \norm{T\vx}^{n+1}
    \end{eqnarray*}
  \end{description}
\end{theproof}

\end{document}
