\documentclass[letterpaper,12pt,fleqn]{article}
\usepackage{matharticle}
\pagestyle{empty}
\newcommand{\p}{\phi}
\begin{document}
\section*{Inverse Properties}

It has already been show that inverses are unique.

\begin{theorem}
  Let $G$ be a group with identity element $e$.
  \[e^{-1}=e\]
\end{theorem}

\begin{theproof}
  $ee=e$ \\
  But inverses are unique, \\
  $\therefore e^{-1}=e$
\end{theproof}

\begin{theorem}
  Let $G$ be a group with identity element $e$.
  \[\forall\,a,b\in G,(ab)^{-1}=b^{-1}a^{-1}\]
\end{theorem}

\begin{theproof}
  Assume $a,b\in G$ \\
  $a^{-1},b^{-1}\in G$ \\
  $ab$ and $b^{-1}a^{-1}\in G$ \\
  $(ab)(b^{-1}a^{-1})=a(bb^{-1})a^{-1}=aea^{-1}=aa^{-1}=e$ \\
  But inverses are unique, \\
  $\therefore (ab)^{-1}=b^{-1}a^{-1}$
\end{theproof}

\begin{theorem}
  Let $G$ be a group with identity element $e$.
  \[\forall\,a\in G,\left(a^{-1}\right)^{-1}=a\]
\end{theorem}

\begin{theproof}
  Assume $a\in G$ \\
  $a^{-1}$ and $\left(a^{-1}\right)^{-1}\in G$ \\
  $a^{-1}\left(a^{-1}\right)^{-1}=\left(a^{-1}a\right)^{-1}=e^{-1}=e$ \\
  But inverses are unique, \\
  $\therefore \left(a^{-1}\right)^{-1}=a$
\end{theproof}

\begin{theorem}
  Let $G,H$ be groups and let $\p:G\to H$ be an isomorphism.
  \[\forall\,a\in G,\p(a^{-1})=\p(a)^{-1}\]
\end{theorem}

\begin{theproof}
  Assume $a\in G$ \\
  $a^{-1}\in G$ \\
  $\p(aa^{-1})=\p(a)\p(a^{-1})$ \\
  $\p(aa^{-1})=\p(e)$ \\
  $\p(a)\p(a^{-1})=\p(e)$ \\
  But $\p(e)$ is an identity for $H$ and inverses are unique, \\
  $\therefore \p(a^{-1})=\p(a)^{-1}$
\end{theproof}

\end{document}
