\documentclass[letterpaper,12pt,fleqn]{article}
\usepackage{matharticle}
\pagestyle{empty}
\newcommand{\D}{\Delta}
\newcommand{\Dx}{\D x}
\newcommand{\Dy}{\D y}
\newcommand{\Dz}{\D z}
\newcommand{\limDx}{\lim_{\Dx\to 0}}
\newcommand{\limDy}{\lim_{i\Dy\to 0}}
\newcommand{\limDz}{\lim_{\Dz\to 0}}
\newcommand{\limDxy}{\lim_{(\Dx,\Dy)\to (0,0)}}
\begin{document}
\section*{Cauchy-Riemann Equations}

\begin{theorem}
  Let $f(z)=u(x,y)+iv(x,y)$ be differentiable on a domain $D$. The first
  partial derivatives ($u_x,u_y,v_x,v_y$) exist in $D$ and satisfy the
  Cauchy-Rieman equations:
  \[u_x=v_y\ \mbox{and}\ u_y=-v_x\]
  so that:
  \[f'(z)=u_x+iv_x=v_y-iu_y\]
\end{theorem}

\begin{theproof}
  Assume $z\in D$
  \[f'(z)=\limDz{\frac{f(z+\Dz)-f(z)}{\Dz}}\]
  \[=\limDxy{\frac{[u(x+\Dx,y+\Dy)+iv(x+\Dx,y+\Dy)]-
      [u(x,y)+iv(x,y)}{\Dx+i\Dy}}\]
  \[=\limDxy{\left[\frac{u(x+\Dx,y+\Dy)-u(x,y)}{\Dx+i\Dy}+
      i\frac{v(x+\Dx,y+\Dy)-v(x,y)}{\Dx+i\Dy}\right]}\]
  
  Consider the path along the $x$-axis: $(\Dx,0)\to(0,0)$:
  \[f'(z)=\limDx{\left[\frac{u(x+\Dx,y)-u(x,y)}{\Dx}+
      i\frac{v(x+\Dx,y)-v(x,y)}{\Dx}\right]}\]
  \[=\limDx{\frac{u(x+\Dx,y)-u(x,y)}{\Dx}}+
  i\limDx{\frac{v(x+\Dx,y)-v(x,y)}{\Dx}}\]
  \[=u_x+iv_x\]
  
  Now, consider the path along the $y$-axis: $(0,i\Dy)\to(0,0)$:
  \[f'(z)=\limDy{\left[\frac{u(x,y+\Dy)-u(x,y)}{i\Dy}+
      i\frac{v(x,y+\Dy)-v(x,y)}{i\Dy}\right]}\]
  \[=\limDy{\left[\frac{v(x,y+\Dy)-v(x,y)}{\Dy}-
      i\frac{u(x,y+\Dy)-u(x,y)}{\Dy}\right]}\]
  \[=\limDy{\frac{v(x,y+\Dy)-v(x,y)}{\Dy}}-
  i\limDy{\frac{u(x,y+\Dy)-u(x,y)}{\Dy}}\]
  \[=v_y-iu_y\]

  Thus, in order for the limit to exist:
  \[f'(z)=u_x+iv_x=v_y-iu_y\]
  $\therefore u_x=u_y$ and $v_x=-u_y$
\end{theproof}

\begin{corollary}
  Let $f(z)=u(x,y)+iv(x,y)$ be differentiable on a domain $D$:
  \[f'(z)=f_x=-if_y\]
\end{corollary}

\begin{theproof}
  The CR equations hold in $D$ \\
  $f'(z)=u_x+iv_x=f_x$ \\
  $f'(z)=v_y-iu_y=-i(u_y+iv_y)=-if_y$
\end{theproof}

\begin{example}
  $f(z)=z^2=(x^2-y^2)+i2xy$ \\
  $f'(z)=2z$ \\
  \begin{minipage}[t]{2in}
    \begin{eqnarray*}
      u &=& x^2-y^2 \\
      u_x &=& 2x \\
      u_y &=& -2y \\
    \end{eqnarray*}
  \end{minipage}
  \begin{minipage}[t]{2in}
    \begin{eqnarray*}
      v &=& 2xy \\
      v_x &=& 2y \\
      v_y &=& 2x \\
    \end{eqnarray*}
  \end{minipage}

  $u_x=v_y=2x$ and $v_x=-u_y=2y$

  $f'(z)=f_x=2x+i2y=2(x+iy)=2z$ \\
  $f'(z)=-if_y=-i(-2y+i2x)=2x+i2y=2(x+iy)=2z$
\end{example}

\end{document}
