\documentclass[letterpaper,12pt,fleqn]{article}
\usepackage{matharticle}
\usepackage{tikz}
\pagestyle{empty}
\begin{document}
\section*{Fields}

\begin{definition}
To say that `*' is a binary operator on a set $S$ means $\forall a,b\in S$, the
operator `*' is:
\begin{enumerate}
\item{Closed: $a*b\in S$}
\item{Well-defined: $a*b=c$ and $a*b=d\implies c=d$}
\end{enumerate}
\end{definition}

\begin{definition}
A field is a mathematical object consisting of a non-empty set of elements $F$
and two binary operators called addition $(a+b)$ and multiplication
$(a\cdot b=ab)$ that satisfy the following nine axioms:
\begin{description}
\item{A1. } Additive Commutivity: $\forall a,b\in F, a+b=b+a$
\item{A2. } Additive Associativity: $\forall a,b,c\in F, (a+b)+c=a+(b+c)$
\item{A3. } Additive Identity: $\exists\, 0\in F,\forall a\in F, a+0=0+a=a$
\item{A4. } Additive Inverse: $\forall a\in F, \exists (-a)\in F,a+(-a)=0$
\\
\item{M1. } Multiplicative Commutivity: $\forall a,b\in F, ab=ba$
\item{M2. } Multiplicative Associativity: $\forall a,b,c\in F, (ab)c=a(bc)$
\item{M3. } Multiplicative Identity: $\exists\, 1\in F,\forall a\in F, a1=1a=a$
\item{M4. } Multiplicative Inverse:
    $\forall a\in F-\{0\}, \exists a^{-1}\in F,aa^{-1}=1$
\\
\item{LD. } Left Distribution: $\forall a,b,c\in F, a(b+c)=ab+ac$
\end{description}
\end{definition}

\begin{theorem}[Right Distribution (RD)]
$\forall a,b,c\in F, (a+b)c=ac+bc$
\end{theorem}

\begin{theproof}
Assume $a,b,c\in F$. \\
\begin{tabular}{ll}
$a+b\in F$ & closure \\
$(a+b)c=c(a+b)$ & M1 \\
$(a+b)c=ca+cb$ & LD \\
$\therefore (a+b)c=ac+bc$ & M1 \\
\end{tabular}
\end{theproof}

\begin{theorem}[Right Cancellation]
\listbreak
\begin{enumerate}
\item{$\forall a,b,c\in F, a+c=b+c\iff a=b$}
\item{$\forall a,b,c\in F, ac=bc$ and $c\ne0\implies a=b$}
\item{$\forall a,b,c\in F, a=b\implies ac=bc$}
\end{enumerate}
\end{theorem}

\begin{theproof}
\listbreak
\begin{enumerate}
\item Assume $a,b,c\in F$.
\begin{description}
\item{$\implies$} Assume $a+c=b+c$.

\begin{tabular}{ll}
$\exists (-c)\in F,c+(-c)=0$ & A4 \\
$(a+c)+(-c)=(b+c)+(-c)$ & WD \\
$a+(c+(-c))=b+(c+(-c))$ & A2 \\
$a+0=b+0$ & A4 \\
$\therefore a=b$ & A3 \\
\end{tabular}

\item{$\impliedby$} Assume $a=b$.

\begin{tabular}{ll}
$\therefore a+c=b+c$ & WD \\
\end{tabular}
\end{description}

\item Assume $a,b\in F$ and $c\in F-\{0\}$.
\\
Assume $ac=bc$.

\begin{tabular}{ll}
$\exists c^{-1}\in F,cc^{-1}=1$ & M4 \\
$(ac)c^{-1}=(bc)c^{-1}$ & WD \\
$a(cc^{-1})=b(cc^{-1})$ & M2 \\
$a1=b1$ & M4 \\
$\therefore a=b$ & M3 \\
\end{tabular}

\item Assume $a,b,c\in F$.
\\
Assume $a=b$.

\begin{tabular}{ll}
$\therefore ac=bc$ & WD \\
\end{tabular}

\end{enumerate}
\end{theproof}

\begin{theorem}[Left Cancellation]
\listbreak
\begin{enumerate}
\item{$\forall a,b,c\in F, c+a=c+b\iff a=b$}
\item{$\forall a,b,c\in F, ca=cb$ and $c\ne0\implies a=b$}
\item{$\forall a,b,c\in F, a=b\implies ca=cb$}
\end{enumerate}
\end{theorem}

\begin{theproof}
\listbreak
\begin{enumerate}
\item{Assume $a,b,c\in F$.}
\begin{eqnarray*}
c+a=c+b &\iff& a+c=b+c\hspace{0.25in}\mbox{(A1)} \\
    &\iff& a=b\hspace{0.25in}\mbox{(RCAN)} \\
\end{eqnarray*}

\item{Assume $a,b\in F$ and $c\in F-\{0\}$.}
\\
Assume $ac=bc$.

\begin{tabular}{ll}
$ac=bc$ & M1 \\
$\therefore a=b$ & RCAN \\
\end{tabular}

\item{Assume $a,b,c\in F$}.
\\
Assume $a=b$.

\begin{tabular}{ll}
$ac=bc$ & WD \\
$\therefore ca=cb$ & M1 \\
\end{tabular}
\end{enumerate}
\end{theproof}

\begin{theorem}[Uniqueness]
\listbreak
\begin{enumerate}
\item{The additive identify is unique}
\item{$\forall a\in F, (-a)$ is unique}
\item{The multiplicative identify is unique}
\item{$\forall a\in F-\{0\}, a^{-1}$ is unique}
\end{enumerate}
\end{theorem}

\begin{theproof}
\listbreak
\begin{enumerate}
\item{Assume that there are two: $0$ and $0'$.}

\begin{tabular}{ll}
$a+0=a$ & A3 \\
$a+0'=a$ & A3 \\
$a+0=a+0'$ & WD \\
$\therefore 0=0'$ & LCAN \\
\end{tabular}

\item{Assume that there are two: $a'$ and $a''$.}

\begin{tabular}{ll}
$a+a'=0$ & A4 \\
$a+a''=0$ & A4 \\
$a+a'=a+a''$ & WD \\
$\therefore a'=a''$ & LCAN \\
\end{tabular}

\item{Assume that there are two: $1$ and $1'$.}

\begin{tabular}{ll}
$a1=a$ & A3 \\
$a1'=a$ & A3 \\
$a1=a1'$ & WD \\
$\therefore 1=1'$ & LCAN \\
\end{tabular}

\item{Assume that there are two: $a'$ and $a''$.}

\begin{tabular}{ll}
$aa'=1$ & M4 \\
$aa''=1$ & M4 \\
$aa'=aa''$ & WD \\
$\therefore a'=a''$ & LCAN \\
\end{tabular}
\end{enumerate}
\end{theproof}

\theoremstyle{mathitem}
\newtheorem*{zero}{Properties of Zero}
\begin{zero}
\listbreak
\begin{enumerate}
\item{$0=-0$}
\item{$\forall a\in F,a0=0a=0$}
\item{$\forall a,b\in F, ab=0\iff a=0$ or $b=0$}
\end{enumerate}
\end{zero}

\begin{theproof}
\listbreak
\begin{enumerate}

\item\mbox{}
\listbreak

\begin{tabular}{ll}
$0+(-0)=0$ & A4 \\
$0+(-0)=-0$ & A3 \\
$\therefore 0=-0$ \\
\end{tabular}

\item{Assume $a\in F$.}

\begin{tabular}{ll}
$a0\in F$ & Closure \\
$a0=a0+0$ & A3 \\
$a(0+0)=a0+0$ & A3 \\
$a0+a0=a0+0$ & LD \\
$\therefore a0=0$ & LCAN \\
$\therefore 0a=0$ & M1 \\
\end{tabular}

\item{Assume $a,b\in F$.}
\begin{description}
\item{$\implies$} Assume $ab=0$.

\begin{tabular}{ll}
AWLOG: $b\ne 0$ & \\
$\exists b^{-1}\in F, bb^{-1}=1$ & M4 \\
$(ab)b^{-1}=0b^{-1}$ & WD \\
$(ab)b^{-1}=0$ & prop of 0 \\
$a(bb^{-1})=0$ & M2 \\
$a1=0$ & M4 \\
$\therefore a=0$ & M3 \\
\end{tabular}

\item{$\impliedby$} AWLOG: $a=0$

\begin{tabular}{ll}
$ab=0a=0$ & prop of 0 \\
\end{tabular}

\end{description}
\end{enumerate}
\end{theproof}

\theoremstyle{mathitem}
\newtheorem*{inverse}{Properties of Negatives}
\begin{inverse}
\listbreak
\begin{enumerate}
\item{$\forall a\in F, (-1)a=-a$}
\item{$\forall a\in F, -(-a)=a$}
\item{$\forall a,b\in F, (-a)b=-ab$}
\item{$\forall a,b\in F, a(-b)=-ab$}
\item{$\forall a,b\in F, (-a)(-b)=ab$}
\end{enumerate}
\end{inverse}

\begin{theproof}
\listbreak
\begin{enumerate}
\item{Assume $a\in F$}

\begin{tabular}{ll}
$a+(-1)a=1a+(-1)a$ & M3 \\
$a+(-1)a=(1+(-1))a$ & RD \\
$a+(-1)a=0a$ & A4 \\
$a+(-1)a=0$ & prop of 0 \\
$\therefore (-1)a=-a$ & uniqueness \\
\end{tabular}

\item{Assume $a\in F$}

\begin{tabular}{ll}
$-(-a)+(-a)=(-1)(-a)+(-a)$ & (1) \\
$-(-a)+(-a)=(-1)(-a)+1(-a)$ & M3 \\
$-(-a)+(-a)=((-1)+1)(-a)$ & RD \\
$-(-a)+(-a)=0(-a)$ & A4 \\
$-(-a)+(-a)=0$ & prop of 0 \\
$\therefore -(-a)=a$ & uniqueness \\
\end{tabular}

\item{Assume $a,b\in F$}

\begin{tabular}{ll}
$ab+(-a)b=(a+(-a))b$ & RD \\
$ab+(-a)b=0b$ & A4 \\
$ab+(-a)b=0$ & prop of 0 \\
$\therefore (-a)b=-ab$ & uniqueness \\
\end{tabular}

\item{Assume $a,b\in F$}

\begin{tabular}{ll}
$ab+a(-b)=a(b+(-b))$ & LD \\
$ab+a(-b)=a0$ & A4 \\
$ab+a(-b)=0$ & prop of 0 \\
$\therefore a(-b)=-ab$ & uniqueness \\
\end{tabular}

\item{Assume $a,b\in F$}

\begin{tabular}{ll}
$(-a)(-b)+(-ab)=(-a)(-b)+(-a)b$ & (3) \\
$(-a)(-b)+(-ab)=(-a)(-b+b)$ & LD \\
$(-a)(-b)+(-ab)=(-a)0$ & A4 \\
$(-a)(-b)+(-ab)=0$ & A3 \\
$\therefore (-a)(-b)=ab$ & uniqueness \\
\end{tabular}
\end{enumerate}
\end{theproof}
\end{document}
