\documentclass[letterpaper,12pt,fleqn]{article}
\usepackage{matharticle}
\pagestyle{empty}
\begin{document}
\section*{Relatively Prime}

\begin{definition}
  $\forall\,a,b\in\Z$, to say that $a$ and $b$ are \emph{relatively prime}
  means $(a,b)=1$.
\end{definition}

\begin{corollary}[To B\'ezout]
  \listbreak
  \[\forall\,a,b\in\Z,(a,b)=1\iff\exists\,m,n\in\Z,ma+nb=1\]
\end{corollary}

\begin{theproof}
  Assume $a,b\in\Z$ \\
  $(a,b)=1\iff1=\min\{ma+nb\in\Z^+\mid m,n\in\Z\}\iff\exists\,m,n\in\Z,ma+nb=1$
\end{theproof}

\begin{theorem}
  Let $a,b,c\in\Z$ and $a\ne0$:
  \[a\mid bc\ \mbox{and}\ (a,b)=1\implies a\mid c\]
\end{theorem}

\begin{theproof}
  Assume $a\mid bc$ and $(a,b)=1$ \\
  $\exists\,m,n\in\Z,ma+nb=1$ \\
  $(cm)a+n(bc)=c$ \\
  But $a\mid a$ and $a\mid bc$ \\
  So $a\mid(cm)a+n(bc)$ \\
  $\therefore a\mid c$
\end{theproof}

\begin{theorem}
  Let $p$ be a prime number:
  \[\forall\,a\in\Z,(p,a)=1\iff p\nmid a\]
\end{theorem}

\begin{theproof}
  Assume $a\in\Z$

  \begin{description}
  \item $\implies$ Assume $p\mid a$

    $p\mid p$ \\
    $p\in D_p\cap D_a$ \\
    $p>1$ \\
    $\therefore (p,a)\ge p>1$

  \item $\impliedby$ Assume $p\nmid a$

    $D_p=\{\pm1,\pm p\}$ \\
    $D_p\cap D_a=\{\pm1\}$ \\
    $\therefore (p,a)=1$
  \end{description}
\end{theproof}

\begin{corollary}
  Let $p$ be a prime number:
  \[\forall\,a,b\in\Z,p\mid ab\implies p\mid a\ \mbox{or}\ p\mid b\]
\end{corollary}

\begin{theproof}
  Assume $a,b\in\Z$ \\
  Assume $p\mid ab$ \\
  \begin{description}
  \item{Case 1: $p\mid a$}

    Done.
    
  \item{Case 2: $p\nmid a$}

    (p,a)=1 \\
    $\therefore p\mid b$
  \end{description}
\end{theproof}

\begin{corollary}
  Let $a,b\in\Z$ such that $a\ne0$ or $b\ne0$ and $d=(a,b)$:
  \[(\frac{a}{d},\frac{b}{d})=1\]
\end{corollary}

\begin{theproof}
  \[(\frac{a}{d},\frac{b}{d})=\frac{d}{d}=1\]
\end{theproof}

\begin{corollary}
  Let $\frac{a}{b}\in\Q$:
  \[\exists\,\frac{p}{q}\in\Q,\frac{a}{b}=\frac{p}{q}\ \mbox{and}\ (p,q)=1\]
\end{corollary}

\begin{theproof}
  Let $d=(a,b)$ \\
  Let $p=\frac{a}{d}$ and $q=\frac{b}{d}$ \\
  $(p,q)=1$ \\
  $\frac{p}{q}=\frac{\frac{a}{d}}{\frac{b}{d}}=\frac{a}{b}$
\end{theproof}

\end{document}
