\documentclass[letterpaper,12pt,fleqn]{article}
\usepackage{matharticle}
\pagestyle{empty}
\DeclareMathOperator{\tr}{tr}
\newcommand{\conj}[1]{\overline{#1}}
\begin{document}
\section*{Unitary Similarity}

\begin{definition}[Unitary Similarity]
  Let $A,B\in M_n$. To say that $A$ is \emph{unitary similar} to $B$ means
  there exists a unitary matrix $U$ such that:
  \[B=UAU^*\]
\end{definition}

\begin{theorem}
  Let $A,B\in M_n$ be unitary similar:
  \[\tr(AA^*)=\tr(BB^*)\]
\end{theorem}

\begin{theproof}
  There exists unitary matrix $U$ such that $B=UAU^*$ \\
  $BB^*=(UAU^*)(UAU^*)^*=UAU^*UA^*U^*=(UA)(A^*U^*)$ \\
  $\tr(BB^*)=\tr((UA)(A^*U^*))=\tr((A^*U^*)(UA))=\tr(A^*A)=\tr(AA^*)$
\end{theproof}

Thus, we can rule out unitary similarity if $\tr(AA^*)\ne\tr(BB^*)$.

\begin{theorem}[Frobenius Norm]
  Let $A\in M_n$:
  \[\tr(AA^*)=\sum_{1\le i,j\le n}\abs{A_{ij}}^2\]
\end{theorem}

\begin{theproof}
  $A=[a_{ij}]$ \\
  $A^*=[\conj{a_{ji}}]$ \\
  $(A^*A)_{ij}=\sum_{k=1}^n(A^*)_{ik}A_{kj}=\sum_{k=1}^n\conj{a_{ki}}a_{kj}$ \\
  $(A^*A)_{ii}=\sum_{k=1}^n\conj{a_{ki}}a_{ki}=\sum_{k=1}^n\abs{a_{ki}}^2$ \\
  $\therefore\tr(A^*A)=\sum_{i=1}^n\sum_{k=1}^n\abs{a_{ki}}^2=
  \sum_{i,j=1}^n\abs{a_{ij}}^2$ \\
\end{theproof}

\begin{example}
  Let $A=\begin{bmatrix} 3 & 1 \\ -2 & 0 \end{bmatrix}$ and
  $B=\begin{bmatrix} 1 & 1 \\ 0 & 2 \end{bmatrix}$

  These matrices are similar; however:

  $\tr(AA^*)=3^2+1^2+(-2)^2+0^2=14$

  $\tr(BB^*)=1^2+1^2+0^2+2^2=6$

  Thus, $A$ and $B$ are not unitary similar.
\end{example}

\end{document}
