\documentclass[letterpaper]{article}

\setlength{\topmargin}{0in}
\setlength{\headheight}{0in}
\setlength{\headsep}{0in}
\setlength{\footskip}{0.5in}
\setlength{\textheight}{\paperheight}
\addtolength{\textheight}{-2in}
\addtolength{\textheight}{-\footskip}

\setlength{\oddsidemargin}{0in}
\setlength{\evensidemargin}{0in}
\setlength{\textwidth}{\paperwidth}
\addtolength{\textwidth}{-2in}

\pagestyle{empty}

\begin{document}

\begin{center}
\bfseries
San Jos\'{e} State University \\
Fall 2015 \\
Math-8: College Algebra \\
Section 03: MW noon--1:15pm \\
Section 05: MW 4:30pm-5:45pm \\
\bigskip
Homework Week 4 Solutions
\end{center}

\underline{\textbf{Section 0.5}}

\bigskip

7. $-3x^3+2x+8$, degree=3

\bigskip

8. Not a polynomial because of the $-3x^{-1}$ term.

\bigskip

9. Not a polynomial, because if we divide by $x$ we get $3+4x^{-1}$, which is
not a polynomial because of the $4x^{-1}$ term.

\bigskip

10. $\frac{2}{3}x^2+\frac{5}{3}x-1$, degree=2

\bigskip

11. $-w^4+2w^3+w^2$, degree=4

\bigskip

12. Not a polynomial because of the square root.

\bigskip

16. $x^3-4x^2+x$

\bigskip

a. $x=-1$

\[(-1)^3-4(-1)^2+(-1)=-1-4(1)-1=-1-4-1=-6\]

b. $x=0$

\[(0)^3-4(0)^2+(0)=0-4(0)+0=0\]

c. $x=1$

\[(1)^3-4(1)^2+(1)=1-4(1)+1=1-4+1=-2\]

d. $x=2$

\[(2)^3-4(2)^2+(2)=8-4(4)+2=8-16+2=-6\]

18.
\begin{eqnarray*}
(3x^2+1)-(2x^2-2x+3) &=& 3x^2+1-2x^2+2x-3 \\
                    &=& (3x^2-2x^2)+2x+(1-3) \\
                    &=& x^2+2x-2 \\
\end{eqnarray*}

20.
\begin{eqnarray*}
-(5x^2-1)+(-3x^2+5) &=& -5x^2+1-3x^2+5 \\
                   &=& (-5x^2-3x^2)+(1+5) \\
                   &=& -8x^2+6 \\
\end{eqnarray*}

22.
\begin{eqnarray*}
(15x^4-18x-19)-(13x^4-5x+15) &=& 15x^4-18x-19-13x^4+5x-15 \\
                            &=& (15x^4-13x^4)+(-18x+5x)+(-19-15) \\
                            &=& 2x^4-13x-34 \\
\end{eqnarray*}

24. $z^2(2z^2+3z+1)=2z^4+6z^3+z^2$

\bigskip

26. $(2-x^2)(-2x)(4x)=-8x^2(2-x^2)=-16x^2+8x^4=8x^4-16^2$

\bigskip

28. $(x-5)(x+10)=x^2+10x-5x-50=x^2+5x-50$

\bigskip

30. $(7x-2)(4x-3)=28x^2-21x-8x+6=28x^2-29x+6$

\bigskip

32. $(3x-4)(x^2-2x+1)=$
\begin{tabular}{cccc}
$3x^3$ & $-6x^2$ & $+3x$ & \\
     & $-4x^2$ & $+8x$ & $-4$ \\
\hline
$3x^3$ & $-10x^2$ & $+11x$ & $-4$ \\
\end{tabular}

\bigskip

34. $(x^2+3x+2)(2x^2-x+4)=$
\begin{tabular}{ccccc}
$2x^4$ & $-x^3$ & $+4x^2$ & & \\
       & $+6x^3$ & $-3x^2$ & $+12x$ & \\
       &         & $+4x^2$ & $-2x$ & $+8$ \\
\hline
$2x^4$ & $+5x^3$ & $+5x^2$ & $+10x$ & $+8$ \\
\end{tabular}

\bigskip

36. $(3x+2)(3x-2)=9x^2-4$

\bigskip

38. $(3x-2)^2=9x^2-12x+4$

\bigskip

40. $(5-8x)^2=25-80x+64x^2=64x^2-80x+25$

\bigskip

42. $[(x+1)-y]^2=(x+1)^2-2(x+1)y+y^2$

\bigskip

44. $(x-2)^3=x^3-3x^2(2)+3x(2^2)-x^3=x^3-6x^2+12x-8$

\bigskip

46.
\begin{eqnarray*}
(3x+2y)^3 &=& (3x)^3+3(3x)^2(2y)+3(3x)(2y)^2+(2y)^3 \\
          &=& 27x^3+(3\cdot9\cdot2)x^2y+(3\cdot3\cdot4)xy^2+8y^3 \\
          &=& 27x^3+54x^2y+36xy^2+3y^3 \\
\end{eqnarray*}

48. $(3x^2-4y^2)(3x^2+4y^2)=9x^4-16y^2$

\bigskip

62. $920(1.04)^5+1000(1.04)^4+780(1.04)^3+1310(1.04)^2+1020(1.04)+1200=6844.27$

Not quite \$7000, so you would be a little short on the deposit.

\bigskip

64. $20(x+x+12)=20(2x+12)=40x+240$

\bigskip

\underline{\textbf{Section 0.6}}

\bigskip

34. $x^2+6x+8=(x+4)(x+2)$

\bigskip

36. $z^2-z-6=(z-3)(z+2)$

\bigskip

38. $z^2-4z-21=(z-7)(z+3)$

\bigskip

40. $x^2-5x-150=(x-15)(x+10)$

\bigskip

42. $2x^2-x-1=(2x+1)(x-1)$

\bigskip

44. $12y^2+7y+1=(4y+1)(3y+1)$

\bigskip

46. $5u^2+13u-6=(5u-2)(u+3)$

\bigskip

52. $z^5+2z^3+z^2+2=z^3(z^2+2)+(z^2+2)=(z^3+1)(z^2+2)$

\bigskip

54. $3x^2+5x-2=3x^2+6x-x-2=3x(x+2)-(x+2)=(3x-1)(x+2)$

\bigskip

58. $12x^3-48x=12x(x^2-4)=12x(x+2)(x-2)$

\bigskip

60. $x^3-\frac{1}{4}x=\frac{1}{4}x(4x^2-1)=\frac{1}{4}x(2x+1)(2x-1)$

\bigskip

62. $7y^2-63=7(y^2-9)=7(y+3)(y-3)$

\bigskip

64. $9x^2-6x+1=(3x-1)^2$

\bigskip

66. $16+6x-x^2=-(x^2-6x-16)=-(x-8)(x+2)$

\bigskip

68. $3x^4+x^3-10x^2=x^2(3x^2+x-10)=x^2(3x-5)(x+2)$

\bigskip

70. Irreducible

\bigskip

72. $5-x+5x^2-x^3=(5-x)+x^2(5-x)=(1+x^2)(5-x)$

\bigskip

74. $3u-2u^2+6-u^3=(3u+6)-(2u^2+u^3)=3(u+2)-u^2(u+2)=(3-u^2)(u+2)$

\bigskip

76. $(t-1)^2-49=[(t-1)+7][(t-1)-7]=(t+6)(t-8)$

\bigskip

78. $(x^2+8)^2-36x^2=[(x^2+8)+6x][(x^2+8)-6x]=(x^2+6x+8)(x^2-6x+8)$

\bigskip

80. $3x^3+81=3(x^3+27)=3(x+3)(x^2-3x+9)$

\bigskip

86. $3x^2+8x+4=(3x+2)(x+2)$, so if the width is $x+2$ then the length must be
$3x+2$.

\bigskip

\underline{\textbf{Section 1.3}}

\bigskip

12.
\begin{eqnarray*}
x^2-10x+9 &=& 0 \\
(x-1)(x-9) &=& 0 \\
x &=& 1,9 \\
\end{eqnarray*}

14.
\begin{eqnarray*}
9x^2-1 &=& 0 \\
(3x-1)(3x+1) &=& 0 \\
x &=& \pm\frac{1}{3} \\
\end{eqnarray*}

16.
\begin{eqnarray*}
16x^2+56x+49 &=& 0 \\
(4x+7)^2 &=& 0 \\
x &=& -\frac{7}{4} \\
\end{eqnarray*}

18.
\begin{eqnarray*}
2x^2 &=& 19x+33 \\
2x^2-19x-33 &=& 0 \\
(2x+3)(x-11) &=& 0 \\
x &=& -\frac{3}{2},11 \\
\end{eqnarray*}

20.
\begin{eqnarray*}
x^2+4x &=& 21 \\
x^2+4x-21 &=& 0 \\
(x+7)(x-3) &=& 0 \\
x &=& -7,3 \\
\end{eqnarray*}

66.
\begin{eqnarray*}
w(w+10) &=& 336 \\
w^2+10w-336=0 \\
(w+28)(w-14) &=& 0 \\
w &=& 14 \\
l &=& 14+10=24 \\
\end{eqnarray*}

70.
\begin{eqnarray*}
(2x+40)(2x+30) &=& 3000 \\
2(x+20)\cdot2(x+15) &=& 3000 \\
4(x+20)(x+15) &=& 3000 \\
(x+20)(x+15) &=& 750 \\
x^2+35x+300 &=& 750 \\
x^2+35x-450 &=& 0 \\
(x+45)(x-10) &=& 0 \\
x &=& 10 \\
w &=& 2(10)+30=50\mbox{ft} \\
\end{eqnarray*}

72.
\begin{eqnarray*}
-16t^2+1053 &=& 0 \\
-16t^2 &=& -1053 \\
t^2 &=& \frac{1053}{16} \\
t &=& \sqrt{\frac{1053}{16}} \\
t &\approx& 8\ \mbox{seconds} \\
\end{eqnarray*}

74.
\begin{eqnarray*}
-16t^2+100 &=& 0 \\
16t^2-100 &=& 0 \\
4t^2-25 &=& 0 \\
(2t+5)(2t-5) &=& 0 \\
t &=& 2.5\ \mbox{seconds} \\
\end{eqnarray*}

\end{document}
