\documentclass[letterpaper,12pt,fleqn]{article}
\usepackage{matharticle}
\pagestyle{empty}
\newcommand{\dz}[1]{\operatorname{\frac{d}{dz}}\left[#1\right]}
\newcommand{\e}{\epsilon}
\renewcommand{\d}{\delta}
\newcommand{\D}{\Delta}
\newcommand{\Dz}{\D z}
\newcommand{\limz}{\lim_{z\to z_0}}
\newcommand{\limdz}{\lim_{\D z\to0}}
\newcommand{\limw}{\lim_{w\to w_0}}
\newcommand{\p}{\phi}
\begin{document}
\section*{Derivative Laws}

\begin{lemma}
  $f(z)$ continuous at $z_0\implies \limdz{f(z_0+\Dz)}=f(z_0)$
\end{lemma}

\begin{theproof}
  Assume $f(z)$ is continuous at $z_0$:
  \[\limdz{f(z_0+\Dz)}=\limz{f(z_0+(z-z_0))}=\limz{f(z)}=f(z_0)\]
\end{theproof}

\begin{theorem}
  Assume $f(z)$ and $g(z)$ be differentiable (and thus continuous):
  \begin{enumerate}
  \item $\dz{c}=0$

  \item $\dz{z}=1$

  \item $\dz{f(z)+g(z)}=f'(z)+g'(z)$

  \item $\dz{f(z)g(z)}=f'(z)g(z)+f(z)f'(z)$

  \item $g(z)\ne0\implies
    \dz{\frac{f(z)}{g(z)}}=\frac{f'(z)g(z)-f(z)g'(z)}{g(z)^2}$

  \item $\dz{cf(z)}=cf'(z)$

  \item $\forall\,n\in\Z,(n>0\ \mbox{or}\ z\ne0)\implies\dz{z^n}=nz^{n-1}$

  \item $\dz{g(f(z))}=g'[f(z)]f'(z)$
  \end{enumerate}
\end{theorem}

\begin{theproof}
  \listbreak
  \begin{enumerate}
  \item
    \[\limdz{\frac{c-c}{\Dz}}=\limdz\frac{0}{\Dz}=\limdz0=0\]

  \item
    \[\limdz{\frac{(z+\Dz)-z}{\Dz}}=\limdz\frac{\Dz}{\Dz}=\limdz1=1\]

  \item
    \[\limdz{\frac{[f(z+\Dz)+g(z+\Dz)]-[f(z)+g(z)]}{\Dz}}\]
    \[=\limdz{\frac{[f(z+\Dz)-f(z)]+[g(z+\Dz)-g(z)]}{\Dz}}\]
    \[=\limdz{\left[\frac{f(z+\Dz)-f(z)}{\Dz}+\frac{g(z+\Dz)-g(z)}{\Dz}
        \right]}\]
    \[=f'(z)+g'(z)\]

  \item
    \[\limdz{\frac{f(z+\Dz)g(z+\Dz)-f(z)g(z)}{\Dz}}\]
    \[=\limdz{\frac{f(z+\Dz)g(z+\Dz)-f(z)g(z+\Dz)+f(z)g(z+\Dz)-
        f(z)g(z)}{\Dz}}\]
    \[=\limdz{\frac{[f(z+\Dz)-f(z)]g(z+\Dz)+f(z)[g(z+\Dz)-g(z)]}{\Dz}}\]
    \[=\limdz{\left[\frac{f(z+\Dz)-f(z)}{\Dz}g(z+\Dz)+
        f(z)\frac{g(z+\Dz)-g(z)}{\Dz}\right]}\]
    \[=f'(z)g(z)+f(z)g'(z)\]

  \item
    \[\limdz{\frac{\frac{f(z+\Dz)}{g(z+\Dz)}-\frac{f(z)}{g(z)}}{\Dz}}\]
    \[=\limdz{\frac{f(z+\Dz)g(z)-f(z)g(z+\Dz)}{g(z+\Dz)g(z)\Dz}}\]
    \[=\limdz{\frac{f(z+\Dz)g(z)-f(z)g(z)+f(z)g(z)-f(z)g(z+\Dz)}
      {g(z+\Dz)g(z)\Dz}}\]
    \[=\limdz{\frac{[f(z+\Dz)-f(z)]g(z)-f(z)[g(z+\Dz)-g(z)]}{g(z+\Dz)g(z)\Dz}}\]
    \[=\limdz{\frac{\frac{f(z+\Dz)-f(z)}{\Dz}g(z)-
        f(z)\frac{g(z+\Dz)-g(z)}{\Dz}}{g(z+\Dz)g(z)}}\]
    \[=\frac{f'(z)g(z)-f(z)g'(z)}{g(z)^2}\]

  \item
    \[\dz{cf(z)}=\dz{c}f(z)+c\dz{f(z)}=0+cf'(z)=cf'(z)\]

  \item Assume $n\in\Z$

    Assume $n>0$ or $z\ne0$

    \begin{description}
    \item Case 1: $n>0$

      Proof by induction on $n$:

      \begin{description}
      \item Base: $z=1$

        $\dz{z^1}=\dz{z}=1$ \\
        $1z^{1-1}=z^0=1$

      \item Assume $\dz{z^n}=nz^{n-1}$

      \item Consider $\dz{z^{n+1}}$
        \begin{eqnarray*}
          \dz{z^{n+1}} &=& \dz{z^nz} \\
          &=& \dz{z^n}z+z^n\dz{z} \\
          &=& nz^{n-1}z+z^n(1) \\
          &=& nz^n+z^n \\
          &=& (n+1)z^n \\
          &=& (n+1)z^{(n+1)-1} \\
          \end{eqnarray*}
      \end{description}
      
    \item Case 2: $n=0$

      $\dz{z^0}=\dz{1}=0$ \\
      Since $n\not>0$, $z\ne0$ \\
      $0z^{0-1}=0z^{-1}=\frac{0}{z}=0$
      
    \item Case 3: $n<0$

      Let $m=-n>0$ \\
      $\dz{z^n}=\dz{z^{-m}}=\dz{\frac{1}{z^m}}=\frac{z^m(0)-(1)mz^{m-1}}{z^{2m}}
      =-mz^{-m-1}=nz^{n-1}$
    \end{description}

  \item Assume $f(z)$ is differentiable at $z_0$

    Let $w_0=f(z_0)$ \\
    Assume $g(z)$ is differentiable at $w_0$ \\
    Define the following function at $w_0$ and in some neighborhood
    $\abs{w-w_0}<\e$:
    \[\p(w)=\begin{cases}
    0, & w=w_0 \\
    \frac{g(w)-g(w_0)}{w-w_0}-g'(w_0), & \abs{w-w_0}<\e \\
    \end{cases}\]
    $\limw{\p(w)}=0=\p(w_0)$ \\
    Thus, $\p$ is continuous at $w_0$ \\
    $g(w)-g(w_0)=[g'(w_o)+\p(w)](w-w_0)$ \\
    $f$ is continuous at $z_0$ \\
    $\exists\,\d>0,0<\abs{z-z_0}<\d\implies\abs{w-w_0}<\e$ \\
    \newpage
    Assume $0<\abs{z-z_0}<\d$ \\
    \[g[f(z)]-g[f(z_0)]=[g'(f(z_0))+\p(f(z))](f(z)-f(z_0))\]
    \[\frac{g[f(z)]-g[f(z_0)]}{z-z_0}=[g'(f(z_0))+\p(f(z))]
    \frac{f(z)-f(z_0)}{z-z_0}\]
    Since $\p$ is continuous at $w_0$ and $f$ is continuous at $z_0$,
    $\p[f(z)]$ is continuous at $z_0$ and:
    \[\limz{\p[f(z)]}=\p[f(z_0)]=\p(w_0)=0\]
    \begin{eqnarray*}
      \dz{g(f(z))} &=& \limz{\frac{g[f(z)]-g[f(z_0)]}{z-z_0}} \\
      &=& \limz{[g'(f(z_0))+\p(f(z))]\frac{f(z)-f(z_0)}{z-z_0}} \\
      &=& [g'(f(z_0))+0]f'(z_0) \\
      &=& g'[f(z_0)]f'(z_0) \\
    \end{eqnarray*}
  \end{enumerate}
\end{theproof}

\end{document}
