\documentclass[letterpaper,12pt,fleqn]{article}
\usepackage{matharticle}
\pagestyle{empty}
\newcommand{\F}{\mathbb{F}}
\newcommand{\Mn}{M_n(\F)}
\begin{document}
\section*{Transpose}

\begin{definition}[Transpose]
  Let $A$ be an $m\times n$ matrix. The \emph{transpose} of $A$, denoted $A^T$,
  is the $n\times m$ matrix with entries:
  \[(A^T)_{ij}=A_{ji}\]
  Thus, the $i^{th}$ row becomes the $i^{th}$ column and the $j^{th}$ column
  becomes the $j^{th}$ row.
\end{definition}

\begin{theorem}
  \listbreak
  \begin{enumerate}
  \item $(A^T)^T=A^T$
  \item $(cA)^T=cA^T$
  \item $(A+B)^T=A^T+B^T$
  \item $(cA+dB)^T=cA^T+dB^T$
  \end{enumerate}
\end{theorem}

\begin{theproof}
  \listbreak
  \begin{enumerate}
  \item

    $((A^T)^T)_{ij}=(A^T)_{ji}=A_{ij}$

    $\therefore (A^T)^T=A^T$

  \item

    $((cA)^T)_{ij}=(cA)_{ji}=cA_{ji}=c(A^T)_{ij}$

    $\therefore (cA)^T=cA^T$

  \item

    $((A+B)^T)_{ij}=(A+B)_{ji}=A_{ji}+B_{ji}=(A^T)_{ij}+(B^T)_{ij}=(A^T+B^T)_{ij}$

    $\therefore (A+B)^T=A^T+B^T$

  \item

    $(cA+dB)^T=(cA)^T+(dB)^T=cA^T+dB^T$
  \end{enumerate}
\end{theproof}

\begin{definition}[Symmetric]
  To say that a matrix $A$ is symmetry means $A=A^T$.

  Thus, all symmetry matrices must be square matrices.
\end{definition}

\begin{theorem}
  Let $S$ be the set of all symmetric $n\times n$ matrices over a field $\F$:

  $S$ is a subspace of $\Mn$
\end{theorem}

\begin{theproof}
  Clearly, $0^T=0$, so the zero matrix is in $S$.

  Assume $A,B\in S$ \\
  $(A+B)^T=A^T+B^T=A+B$ \\
  Thus, $A+B\in S$

  Therefore $S$ is closed under matrix addition.

  Assume $c\in\F$ \\
  $(cA)^T=cA^T=cA$ \\
  Thus, $cA\in S$

  Therefore $S$ is closed under scalar multiplication.

  Therefore, by the subspace test, $S$ is a subspace of $\Mn$.
\end{theproof}

\end{document}
