\documentclass[letterpaper,12pt,fleqn]{article}
\usepackage{matharticle}
\usepackage{tikz}
\pagestyle{empty}
\newcommand{\conj}[1]{\bar{#1}}
\newcommand{\Conj}[1]{\overline{#1}}
\begin{document}
\section*{Triangle Inequality}
Since complex numbers are vector-like, we can add complex numbers graphically
in vector-like style:

\begin{figure}[h]
\begin{tikzpicture}
\draw (-1,0) -- (4,0);
\draw (0,-1) -- (0,4);
\draw [->] (0,0) -- (3,1);
\draw [->] (0,0) -- (1,2);
\draw [dashed] (3,1) -- (4,3);
\draw [dashed] (1,2) -- (4,3);
\draw [->] (0,0) -- (4,3);
\node [below] at (1.8,0.6) {$z_1$};
\node [above,rotate=75] at (0.6,1.1) {$z_2$};
\node [above,rotate=43] at (2,1.5) {$z_1+z_2$};
\node [rotate=75] at (3.6,1.7) {$z_2$};
\node at (7,2) {$\abs{z_1+z_1}\le\abs{z_1}+\abs{z_2}$};
\end{tikzpicture}
\end{figure}

Note that the triangle inequality is evident from the diagram; however, it can
also be proved analytically:

\begin{theorem}
$\forall z_1,z_2\in\C$:
\[\abs{\abs{a}-\abs{b}}\le\abs{z_1+z_2}\le\abs{z_1}+\abs{z_2}\]
\end{theorem}

\begin{theproof}
  Assume $z_1,z_2\in\C$ \\
  \begin{minipage}[t]{3.25in}
    \begin{eqnarray*}
      \abs{z_1+z_2}^2 &=& (z_1+z_2)\Conj{(z_1+z_2)} \\
      &=& (z_1+z_2)(\conj{z}_1+\conj{z}_2) \\
      &=& z_1\conj{z}_1+z_2\conj{z}_2+z_1\conj{z}_2+\conj{z}_1z_2 \\
      &=& \abs{z_1}^2+\abs{z_2}^2+z_1\conj{z}_2+\Conj{z_1\conj{z}_2} \\
      &=& \abs{z_1}^2+\abs{z_2}^2+2Re(z_1\conj{z}_2) \\
      &\le& \abs{z_1}^2+\abs{z_2}^2+2\abs{z_1\conj{z}_2} \\
      &=& \abs{z_1}^2+\abs{z_2}^2+2\abs{z_1}\abs{\conj{z}_2} \\
      &=& \abs{z_1}^2+\abs{z_2}^2+2\abs{z_1}\abs{z_2} \\
      &=& (\abs{z_1}+\abs{z_2})^2 \\
      \abs{z_1+z_2} &\le& \abs{z_1}+\abs{z_2} \\
    \end{eqnarray*}
  \end{minipage}
  \begin{minipage}[t]{3.25in}
    \begin{eqnarray*}
      \abs{z_1-z_2}^2 &=& (z_1-z_2)\Conj{(z_1-z_2)} \\
      &=& (z_1-z_2)(\conj{z}_1-\conj{z}_2) \\
      &=& z_1\conj{z}_1+z_2\conj{z}_2-z_1\conj{z}_2-\conj{z}_1z_2 \\
      &=& \abs{z_1}^2+\abs{z_2}^2-(z_1\conj{z}_2+\Conj{z_1\conj{z}_2}) \\
      &=& \abs{z_1}^2+\abs{z_2}^2-2Re(z_1\conj{z}_2) \\
      &\ge& \abs{z_1}^2+\abs{z_2}^2-2\abs{z_1\conj{z}_2} \\
      &=& \abs{z_1}^2+\abs{z_2}^2-2\abs{z_1}\abs{\conj{z}_2} \\
      &=& \abs{z_1}^2+\abs{z_2}^2-2\abs{z_1}\abs{z_2} \\
      &=& (\abs{z_1}-\abs{z_2})^2 \\
      \abs{z_1-z_2} &\ge& \abs{\abs{z_1}+\abs{z_2}} \\
      \abs{z_1-(-z_2)} &\ge& \abs{\abs{z_1}+\abs{-z_2}} \\
      \abs{z_1+z_2} &\ge& \abs{\abs{z_1}+\abs{z_2}} \\
    \end{eqnarray*}
  \end{minipage}

  $\therefore\abs{\abs{a}-\abs{b}}\le\abs{z_1+z_2}\le\abs{z_1}+\abs{z_2}$
\end{theproof}

\begin{theproof}[alternate]
  Assume $z_1,z_2\in\C$ \\
  \[\abs{z_1}=\abs{z_1+z_2-z_2}\le\abs{z_1+z_2}+\abs{z_2}\]
  \[\abs{z_1}-\abs{z_2}\le\abs{z_1+z_2}\]
  \[\abs{z_2}=\abs{z_2+z_1-z_1}\le\abs{z_2+z_1}+\abs{z_1}\]
  \[\abs{z_2}-\abs{z_1}=-(\abs{z_1}-\abs{z_2})\le\abs{z_1+z_2}\]
  \[\therefore\abs{\abs{z_1}-\abs{z_2}}\le\abs{z_1+z_2}\]
\end{theproof}

\begin{corollary}
$\forall z_1,z_2\in\C$:
\[\abs{z_1-z_2}\le\abs{z_1}+\abs{z_2}\]
\end{corollary}

\begin{theproof}
Assume $z_1,z_2\in\C$ \\
\[\abs{z_1-z_2}=\abs{z_1+(-z_2)}\le\abs{z_1}+\abs{-z_2}=\abs{z_1}+\abs{z_2}\]
\end{theproof}

\begin{theorem}
$\forall n\in\N$:
\[\abs{\sum_{k=1}^{n}z_k}\le\sum_{k=1}^{n}\abs{z_k}\]
\end{theorem}

\begin{theproof}
(by induction)
\begin{description}
\item{Base Case: $n=1$} \\
$\abs{\sum_{k=1}^{1}z_k}=\abs{z_1}$ \\
$\sum_{k=1}^{1}\abs{z_k}=\abs{z_1}$

\item{Assume $\abs{\sum_{k=1}^{n}z_k}\le\sum_{k=1}^{n}\abs{z_k}$}

\item Consider $\abs{\sum_{k=1}^{n+1}z_k}$
  \[\abs{\sum_{k=1}^{n+1}z_k}=\abs{\sum_{k=1}^{n}z_k+z_{n+1}}\le
  \abs{\sum_{k=1}^{n}z_k}+\abs{z_{n+1}}\le
  \sum_{k=1}^{n}\abs{z_k}+\abs{z_{n+1}}=
  \sum_{k=1}^{n+1}\abs{z_k}\]
\end{description}
\end{theproof}

\begin{theorem}
  $\forall\,z=x+iy\in\C$:
  \[\frac{\abs{x}+\abs{y}}{\sqrt{2}}\le\abs{z}\le\abs{x}+\abs{y}\]
\end{theorem}

\begin{theproof}
  Assume $z=x+iy\in\C$
  \begin{eqnarray*}
    \left(\abs{x}-\abs{y}\right)^2 &=& \abs{x}^2+\abs{y}^2-2\abs{x}\abs{y} \\
    &=& 2\abs{x}^2+2\abs{y}^2-\abs{x}^2-\abs{y}^2-2\abs{x}\abs{y} \\
    &=& 2(\abs{x}^2+\abs{y}^2)-(\abs{x}^2+\abs{y}^2+2\abs{x}\abs{y}) \\
    &=& 2(\abs{z}^2)-(\abs{x}+\abs{y})^2 \\
    &\ge& 0 \\
  \end{eqnarray*}
  \begin{eqnarray*}
    (\abs{x}+\abs{y})^2 &\le& 2(\abs{z}^2) \\
    \abs{x}+\abs{y} &\le& \sqrt{2}\abs{z} \\
    \frac{\abs{x}+\abs{y}}{\sqrt{2}} &\le& \abs{z} \\
  \end{eqnarray*}
  \[\abs{z}=\abs{x+iy}\le\abs{x}+\abs{iy}=\abs{x}+\abs{i}\abs{y}=
  \abs{x}+(1)\abs{y}=\abs{x}+\abs{y}\]

  $\therefore\frac{\abs{x}+\abs{y}}{\sqrt{2}}\le\abs{z}\le\abs{x}+\abs{y}$
\end{theproof}

Note that equality occurs in the first case when $\abs{x}=\abs{y}$, and in the
second case when $x=0$ or $y=0$.

\end{document}
