\documentclass[letterpaper,12pt,fleqn]{article}
\usepackage{matharticle}
\pagestyle{empty}
\newcommand{\vb}{\vec{b}}
\newcommand{\vx}{\vec{x}}
\newcommand{\vy}{\vec{y}}
\newcommand{\vz}{\vec{z}}
\newcommand{\vo}{\vec{0}}
\newcommand{\norm}[1]{\left\|#1\right\|}
\newcommand{\inner}[1]{\left<#1\right>}
\newcommand{\weak}{\overset{w}{\longrightarrow}}
\renewcommand{\a}{\alpha}
\renewcommand{\b}{\beta}
\newcommand{\e}{\epsilon}
\newcommand{\F}{\mathbb{F}}
\newcommand{\conj}[1]{\overline{#1}}
\DeclareMathOperator{\spn}{span}
\begin{document}
\section*{Weak Convergence}

\begin{definition}[Weak Convergence]
  Let $E$ be an inner product space and let $(\vx_n)$ be a sequence of vectors
  in $E$. To say that $(\vx_n)$ converges to $\vx\in E$ \emph{weakly}, denoted
  $\vx_n\weak\vx$, means $\forall\,\vy\in E$:
  \[\inner{\vx_n,y}\to\inner{\vx,y}\]
\end{definition}

\begin{properties}
  Let $H$ be a Hilbert space over a field $\F$. Let $\vx_n\weak\vx$ and
  $\vy_n\weak\vy$ in $H$ and $\a_n\to\a$ in $\F$:
  \begin{enumerate}
  \item The weak limit is unique - i.e., if $\forall\,n\in\N,\vx_n=\vy_n$
    then $\vx=\vy$.
  \item $\vx_n+\vy_n\weak\vx+\vy$
  \item $\a_n\vx_n\weak\a\vx$
  \end{enumerate}
\end{properties}

\begin{theproof}
  \listbreak
  \begin{enumerate}
    \item Assume $\vz\in H$ such that $\vz\ne\vo$ and $\vz\not\perp(\vx-\vy)$.
      \begin{eqnarray*}
        \inner{\vx-\vy,\vz} &=& \inner{(\vx-\vx_n)+(\vx_n-\vy),\vz} \\
        &=& \inner{\vx-\vx_n,\vz}+\inner{\vx_n-\vy,\vz} \\
        &\to& 0+0 \\
        &=& 0
      \end{eqnarray*}
      And so $\vx-\vy=\vo$.

      $\therefore\vx=\vy$

    \item $\inner{\vx_n+\vy_n,\vz}=\inner{\vx_n,\vz}+\inner{\vy_n,\vz}\to
      \inner{\vx,\vz}+\inner{\vy,\vz}=\inner{\vx+\vy,\vz}$

      $\therefore\vx_n+\vy_n\weak\vx+\vy$

    \item $\inner{\a_n\vx_n,\vz}=\a_n\inner{\vx_n,\vz}\to\a\inner{\vx,\vz}=
      \inner{\a\vx,\vz}$

      $\therefore\a_n\vx_n\weak\a\vx$
  \end{enumerate}
\end{theproof}

\begin{theorem}
  Let $E$ be an inner product space and let $(\vx_n)$ be a sequence of vectors
  in $E$:
  \[\vx_n\to\vx\implies\vx_n\weak\vx\]
\end{theorem}

\begin{theproof}
  Assume $\vx_n\to\vx$.

  $\norm{\vx_n-\vx}\to0$

  Assume $\vy\in E$.

  $\abs{\inner{\vx_n,\vy}-\inner{\vx,\vy}}=
  \abs{\inner{\vx_n-\vx,\vy}}\le\norm{\vx_n-\vx}\norm{\vy}\to0$

  $\therefore\vx_n\weak\vx$
\end{theproof}

\begin{theorem}
  Let $E$ be an inner product space and let $(\vx_n)$ be a sequence of vectors
  in $E$:
  \[\vx_n\weak\vx\ \mbox{and}\ \norm{\vx_n}\to\norm{\vx}\implies\vx_n\to\vx\]
\end{theorem}

\begin{theproof}
  Assume $\vx_n\weak\vx\ \mbox{and}\ \norm{\vx_n}\to\norm{\vx}$.
  \begin{eqnarray*}
    \norm{\vx_n-\vx}^2 &=& \inner{\vx_n-\vx,\vx_n-\vx} \\
    &=& \inner{\vx_n,\vx_n}-\inner{\vx_n,\vx}-\inner{\vx,\vx_n}+
    \inner{\vx,\vx} \\
    &=& \norm{\vx_n}^2-\inner{\vx_n,\vx}-\inner{\vx,\vx_n}+\norm{\vx}^2 \\
    &\to& \norm{\vx}^2 -\inner{\vx,\vx}-\inner{\vx,\vx}+\norm{\vx}^2 \\
    &=& 2\norm{\vx}^2-2\norm{\vx}^2 \\
    &=& 0
  \end{eqnarray*}
  $\therefore\vx_n\to\vx$
\end{theproof}

\begin{theorem}
  Let $H$ be a finite dimensional Hilbert space over a field $\F$. For all
  sequences $(\vx_n)$ in $H$:
  \[\vx_n\to\vx\iff\vx_n\weak\vx\]
  Thus, weak convergence implies strong convergence in a finite dimensional
  Hilber space.
\end{theorem}

\begin{theproof}
  Assume $(\vx_n)$ is a sequence in $H$.
  \begin{description}
  \item $\implies$ Assume $\vx_n\to\vx$.

    But strong convergence implies weak convergence in any inner product space.

    $\therefore\vx_n\weak\vx$

  \item $\impliedby$ Assume $\vx_n\weak\vx$.

    Assume $B=\{\vb_1,\ldots,\vb_N\}$ is a basis for $H$. \\
    AWLOG: $B$ is an orthonormal basis (otherwise, use Graham-Schmitt). \\
    $\forall\,n\in\N,\exists\,x_{n,k}\in\F$ such that
    $\vx_n=\sum_{k=1}^nx_{n,k}\vb_k$. \\
    $\exists\,x_k\in\F$ such that $\vx=\sum_{k=1}^Nx_k\vb_k$. \\
    Assume $\vz\in H$. \\
    $\exists\,z_k\in\F$ such that $\vz=\sum_{k=1}^Nz_k\vb_k$. \\
    Since $\vx_n\weak\vx$:
    \begin{eqnarray*}
      \inner{\vx_n-\vx,\vz} &=&
      \inner{\sum_{k=1}^Nx_{n,k}\vb_k-\sum_{k=1}^Nx_k\vb_k,\sum_{k=1}^Nz_k\vb_k} \\
      &=& \inner{\sum_{k=1}^N(x_{n,k}-x_k)\vb_k,\sum_{k=1}^Nz_k\vb_k} \\
      &=& \sum_{k=1}^N(x_{n,k}-x_k)\conj{z_k} \\
      &\to& 0
    \end{eqnarray*}
    But this is for any $\vz\in E$, and so it must be the case that
    $x_{n,k}-x_n\to0$.

    So $\vx_n$ converges to $\vx$ component-wise. \\
    It has already been shown that $\norm{\cdot}_{\infty}$ with respect to a
    particular basis is a proper norm. \\
    Now, since all norms are equivalent in a finite dimensional vector space:
    \[\norm{\vx_n-\vx}_{\infty}=\sup_{k\in\N}\abs{x_{n,k}-x_k}\to0\]
    $\therefore\vx_n\to\vx$
  \end{description}
\end{theproof}

\begin{theorem}
  Let $E$ be an inner product space and let $S\subseteq E$ such that
  $\spn(S)$ is dense in $E$. Let $(\vx_n)$ be a bounded sequence in $E$.
  \[\vx_n\weak\vx\iff\forall\,\vy\in S,\inner{\vx_n,\vy}\to\inner{\vx,\vy}\]
\end{theorem}

\begin{theproof}
  \listbreak
  \begin{description}
  \item $\implies$ Assume $\vx_n\weak\vx$.

    $\forall\,\vy\in E,\inner{\vx_n,\vy}\to\inner{\vx,\vy}$ \\
    But $X\subseteq E$.
    
    $\therefore\forall\,\vy\in S,\inner{\vx_n,\vy}\to\inner{\vx,\vy}$

  \item $\impliedby$ Assume $\forall\,\vy\in S,\inner{\vx_n,\vy}\to
    \inner{\vx,\vy}$

    Assume $\e>0$. \\
    Assume $\vz\in E$. \\
    Since $(\vx_n)$ is bounded, $\exists\,M>0$ such that
    $\norm{\vx_n},\norm{\vx}\le M$. \\
    Since $\spn(S)$ is dense in $E$, $\exists\,\vy_0\in\spn(S)$ such that:
    \[\norm{\vz-\vy_0}<\frac{\e}{3M}\]
    Furthermore, by assumption, $\exists\,N>0$ such that $\forall\,n>N$:
    \[\abs{\inner{\vx_n,\vy_0}-\inner{\vx,\vy_0}}<\frac{\e}{3}\]
    Assume $n>N$:
    \begin{eqnarray*}
      \abs{\inner{\vx_n,\vz}-\inner{\vx,\vz}} &=&
      \abs{(\inner{\vx_n,\vz}-\inner{\vx_n,\vy_0})+
        (\inner{\vx_n,\vy_0}-\inner{\vx,\vy_0})+
        (\inner{\vx,\vy_0}-\inner{\vx,\vz})} \\
      &\le& \abs{\inner{\vx_n,\vz}-\inner{\vx_n,\vy_0}}+
      \abs{\inner{\vx_n,\vy_0}-\inner{\vx,\vy_0}}+
      \abs{\inner{\vx,\vy_0}-\inner{\vx,\vz}} \\
      &\le& \abs{\inner{\vx_n,\vz-\vy_0}}+\frac{\e}{3}+
      \abs{\inner{\vx,\vy_0-\vz}} \\
      &\le& \norm{\vx_n}\norm{\vz-\vy_0}+\frac{\e}{3}+
      \norm{\vx}\norm{\vy_0-\vz} \\
      &\le& M\frac{\e}{3M}+\frac{\e}{3}+M\frac{\e}{3M} \\
      &=& \frac{\e}{3}+\frac{\e}{3}+\frac{\e}{3} \\
      &=& \e
    \end{eqnarray*}
    $\therefore\vx_n\weak\vx$
  \end{description}
\end{theproof}

\begin{theorem}
  Let $H$ be a Hilbert space and let $(\vx)$ be a sequence in $H$:

  \qquad$\vx_n\weak\vx\implies(\vx_n)$ is bounded.
\end{theorem}

\begin{theproof}
  Assume $\vx_n\weak\vx$. \\
  Define $f_n:H\to\C$ by $f_n(\vy)=\inner{\vy,\vx_n}$, $\forall\,n\in\N$. \\
  $f_n$ is clearly linear (due to sesquilinearity of the inner product).

  Assume $\vy_n\to\vy$, and so $\norm{\vy_n-\vy}\to0$ \\
  Since strong implies weak, $\vy_n\weak\vy$. \\
  So $\inner{\vy_n,\vx_n}\to\inner{\vy,\vx_n}$. \\
  $\norm{f_n(\vy_n)-f_n(\vy)}=\abs{\inner{\vy_n,\vx_n}-\inner{\vy,\vx_n}}
  \to0$ \\
  Therefore $f_n(y)$ is continuous, and thus bounded.

  Now, $\forall\,\vy\in H$ the sequence $(f_n(\vy))=(\inner{\vy,\vx_n})$
  converges to $\inner{\vy,\vx}$, and so it is bounded:
  \[\forall\,\vy\in H,\exists\,M_y>0,\abs{f_n(\vy)}=\inner{\vy,\vx_n}<M_y\]
  And so, by the principle of uniform boundedness:
  \[\exists\,M>0,\forall\,n\in\N,\norm{f_n}\le M\]

  Finally:
  \[\norm{f_n(\vx_n)}=\abs{\inner{\vx_n,\vx_n}}=\norm{\vx_n}^2\le
  \norm{f_n}\norm{\vx_n}\]
  Therefore $\norm{\vx_n}\le\norm{f_n}\le M$ and thus $(\vx_n)$ is bounded.
\end{theproof}

\end{document}
